move semantics_new to semantics and remove semantics_new. try to build and run experiments

src/Semantics.v
@@ -992,7 +992,7 @@ Fixpoint iterate (n : nat) (func : VM.t hvalue -> VM.t hvalue -> VM.t hvalue -> 
             end
   end.
 
-Parameter n : nat. (* TBD *)
+Parameter n : nat. 
 Definition compute_Sem (c : HiF.hfcircuit) (inputs : VM.t hvalue) (reg_init : VM.t hvalue) : option (VM.t hvalue * VM.t hvalue) :=
   (* inputs signal and register should update during a rising edge and keep during the iteration *)
   (* compute the value connected to registers according to the stable state, return it as a new reg_init for the next clock cycle *)
@@ -1259,10 +1259,10 @@ with stmt_tmap' (tmap : PVM.t (fgtyp * fcomponent)) (s : HiFP.hfstmt) : option (
                   end
   | Smem _ _ => None (* Memory not considered*)
   | Sinst _ _ => None
-  | Swhen cond ss_true ss_false =>
-      match type_of_hfexpr cond tmap, stmts_tmap' tmap ss_true with
-      | Some _, Some tmap_true => stmts_tmap' tmap_true ss_false 
-      | _, _ => None
+  | Swhen _ ss_true ss_false =>
+      match stmts_tmap' tmap ss_true with
+      | Some tmap_true => stmts_tmap' tmap_true ss_false 
+      | _ => None
       end
   end.
 
@@ -1359,12 +1359,12 @@ Fixpoint iterate (n : nat) (func : PVM.t bits -> PVM.t bits -> PVM.t bits -> PVM
   | n'.+1 => match func (PVM.empty bits) (PVM.empty bits) s tmap with
             | Some (_, ns) => (* everytime we start with an empty map to record the values to be updated in the next iteration *) 
               let s_upd := update_values ns s in
-              if PVM.equal (fun val1 val2 => val1 == val2) s_upd s (* LFP *) then Some s_upd else iterate n' func s_upd tmap
+              (*if PVM.equal (fun val1 val2 => val1 == val2) s_upd s (* LFP *) then Some s_upd else*) iterate n' func s_upd tmap
             | _ => None
             end
   end.
 
-Parameter n : nat. (* TBD *)
+Parameter n : nat. 
 Definition compute_Sem (c : HiFP.hfcircuit) (inputs reg_init : PVM.t bits) : option (PVM.t bits * PVM.t bits) :=
   match circuit_tmap c, c with
   | Some tmap, Fcircuit _ [::(FInmod _ ps ss)] => 
@@ -1384,6 +1384,13 @@ Definition compute_Sem (c : HiFP.hfcircuit) (inputs reg_init : PVM.t bits) : opt
   | _, _ => None
   end.
 
+Lemma iterate_n_is_LFP n ss init_s tmap s : iterate n (eval_hfstmts ss) init_s tmap = Some s -> 
+  forall rs ns, eval_hfstmts ss (PVM.empty bits) (PVM.empty bits) s tmap = Some (rs, ns) -> 
+  PVM.equal (fun val1 val2 => val1 == val2) (update_values ns s) s.
+Proof.
+(* TBD *)
+Admitted.
+
 Definition indeterminate_cst (gt : fgtyp) : HiFP.hfexpr := 
   let w := sizeof_fgtyp gt in 
   let w_inde := length indeterminate_val in
@@ -1393,7 +1400,6 @@ Definition indeterminate_cst (gt : fgtyp) : HiFP.hfexpr :=
 End Sem_HiFP.
 
 Parameter flat_valmap : (VM.t hvalue) -> (VM.t (ftype * fcomponent)) -> PVM.t bits.
-(* TBD *)
 
 Parameter expandConnects : HiF.hfcircuit -> option HiFP.hfcircuit.
 
@@ -1424,9 +1430,8 @@ Section ExpandWhens.
 
 (* a type to indicate connects *)
 Inductive def_expr : Type :=
-| D_undefined (* declared but not connected, no "is invalid" statement *)
-| D_invalidated : fgtyp -> def_expr (* declared but not connected, there is a "is invalid" statement *)
-| D_fexpr : HiFP.hfexpr -> def_expr (* declared and connected *)
+| D_invalidated : fgtyp -> def_expr (* a "is invalid" statement *)
+| D_fexpr : HiFP.hfexpr -> def_expr (* connected *)
 .
 
 (* equality of def_expr is decidable [because equality of hfexpr is decidable] *)
@@ -1439,7 +1444,6 @@ Qed.
 
 Definition def_expr_eqn (x y : def_expr) : bool :=
 match x, y with
-| D_undefined, D_undefined => true
 | D_invalidated gt1, D_invalidated gt2 => gt1 == gt2
 | D_fexpr expr1, D_fexpr expr2 => expr1 == expr2
 | _, _ => false
@@ -1475,9 +1479,7 @@ Definition combine_when_connections
                       | Some (D_fexpr te), Some (D_fexpr fe) =>
                           if te == fe then true_expr
                           else Some (D_fexpr (Emux cond te fe))
-                      | Some D_undefined, _
-                      | _, Some D_undefined => Some D_undefined
-                      | None, _ => false_expr (* TBD cannot be proved now, 关系到when case的证明 *)
+                      | None, _ => false_expr 
                       | _, None => true_expr
                       | Some (D_invalidated gt), Some (D_fexpr fe) => Some (D_fexpr (Emux cond (Sem_HiFP.indeterminate_cst gt) fe)) 
                       | Some (D_fexpr te), Some (D_invalidated gt) => Some (D_fexpr (Emux cond te (Sem_HiFP.indeterminate_cst gt))) 
@@ -1485,7 +1487,43 @@ Definition combine_when_connections
                           Some (D_fexpr (Emux cond (Sem_HiFP.indeterminate_cst gt0) (Sem_HiFP.indeterminate_cst gt1)))
                       end)
              true_conn_map false_conn_map.
-
+(*
+Definition combine_when_connections
+    (* a helper function that takes two connection maps, generated
+       by the two branches of a when statement, and combines them
+       into one connection map containing suitable multiplexers *)
+    (cond           : HiFP.hfexpr)    (* condition under which to decide whether to take the value from true_conn_map *)
+    (true_conn_map  : PVM.t def_expr) (* connections made before or in the true branch *)
+    (false_conn_map : PVM.t def_expr) (* connections made before or in the false branch *)
+:   PVM.t def_expr
+:=  PVM.map2 (fun true_expr false_expr : option def_expr =>
+                      match true_expr, false_expr with
+                      | Some (D_fexpr te), Some (D_fexpr fe) =>
+                          if te == fe then true_expr
+                          else Some (D_fexpr (Emux cond te fe))
+                      | None, _ => false_expr 
+                      | _, None => true_expr
+                      | Some (D_invalidated gt), Some (D_fexpr fe) => match gt with
+                          | Fuint _ 
+                          | Fsint _ => Some (D_fexpr (Emux cond (Sem_HiFP.indeterminate_cst gt) fe)) 
+                          | _ => None
+                          end
+                      | Some (D_fexpr te), Some (D_invalidated gt) => match gt with
+                          | Fuint _ 
+                          | Fsint _ => Some (D_fexpr (Emux cond te (Sem_HiFP.indeterminate_cst gt))) 
+                          | _ => None
+                          end
+                      | Some (D_invalidated gt0), Some (D_invalidated gt1) => match gt0, gt1 with
+                          | Fuint _, Fuint _  
+                          | Fuint _, Fsint _  
+                          | Fsint _, Fuint _  
+                          | Fsint _, Fsint _ => 
+                          Some (D_fexpr (Emux cond (Sem_HiFP.indeterminate_cst gt0) (Sem_HiFP.indeterminate_cst gt1)))
+                          | _, _ => None
+                          end
+                      end)
+             true_conn_map false_conn_map.
+*)
 Fixpoint ExpandBranches_funs
 (* split a statement sequence (possibly containing when
    statements) into a connection map.  The output does not contain when statements. *)
@@ -1546,7 +1584,6 @@ Definition convert_to_connect_stmt
     (old_ss : HiFP.hfstmt_seq) (* old sequence of connect statements *)
 :   HiFP.hfstmt_seq (* returns old_ss, extended with assigning d to v *)
 :=  match d with
-    | D_undefined => old_ss
     | D_invalidated _ => Qcons (Sinvalid (Eid v)) old_ss
     | D_fexpr e => Qcons (Sfcnct (Eid v) e) old_ss
     end.
@@ -1554,7 +1591,7 @@ Definition convert_to_connect_stmt
 Fixpoint component_stmts_of (ss : HiFP.hfstmt_seq) : HiFP.hfstmt_seq :=
 (* extracts from ss the statements that define components *)
 match ss with
-| Qnil => ss
+| Qnil => ss 
 | Qcons s ss' => Qcat (component_stmt_of s) (component_stmts_of ss')
 end
 with component_stmt_of (s : HiFP.hfstmt) : HiFP.hfstmt_seq :=
@@ -1637,16 +1674,30 @@ Proof.
       * by apply H2.
 Qed.
 
-Lemma component_stmts_of_is_declaration ss : forall s, Qin s (component_stmts_of ss) -> is_declaration s.
+Lemma component_stmts_of_is_declaration ss : forall s, Qin s (component_stmts_of ss) -> is_declaration s
+with component_stmt_of_is_declaration ss : forall s, Qin s (component_stmt_of ss) -> is_declaration s.
 Proof.
   induction ss as [|s ss IH]. simpl; done.
-  simpl; intros. destruct s as [|v0 t|v0 r|v0 m|v0 v1|v0 e0|v0 e0|v0|c s1 s2] eqn : Hstmt; subst s; simpl in *.
-  1,7,8 : apply IH; done.
-  1,2,3,4,5 : case /orP : H => H; destruct s0 eqn : Hs0; try done; apply IH; done.
-  admit. (* when *)
-Admitted.
+  simpl; intros. apply Qin_Qcat in H. destruct H. 
+  move : H; apply component_stmt_of_is_declaration.
+  move : H; apply IH.
+  clear component_stmt_of_is_declaration.
+  intro. destruct ss as [|v0 t|v0 r|v0 m|v0 v1|v0 e0|v0 e0|v0|c s1 s2] eqn : Hstmt; subst ss; simpl; try done; intros.
+  1-5 : destruct s; try done. apply Qin_Qcat in H. destruct H. 
+  1,2 : move : H; apply component_stmts_of_is_declaration.
+Qed.
 
-Lemma stmts_tmap_component_stmts_of_eq ss pmap : Sem_HiFP.stmts_tmap' pmap ss = Sem_HiFP.stmts_tmap' pmap (component_stmts_of ss).
+Lemma stmts_tmap_qcat pmap s1 s2 : match Sem_HiFP.stmts_tmap' pmap s1 with
+  | Some tmap_true => Sem_HiFP.stmts_tmap' tmap_true s2 
+  | _ => None
+  end = Sem_HiFP.stmts_tmap' pmap (Qcat s1 s2).
+Proof. 
+  move : s1 pmap s2. elim; simpl in *; try done.
+  intros hd tl IH pmap s2. destruct (Sem_HiFP.stmt_tmap' pmap hd) as [tmap'|]; try done.
+Qed.
+
+Lemma stmts_tmap_component_stmts_of_eq ss pmap : Sem_HiFP.stmts_tmap' pmap ss = Sem_HiFP.stmts_tmap' pmap (component_stmts_of ss)
+with stmt_tmap_component_stmts_of_eq s pmap : Sem_HiFP.stmt_tmap' pmap s = Sem_HiFP.stmts_tmap' pmap (component_stmt_of s).
 Proof.
   move : ss pmap; elim. simpl; done.
   intros hd tl IH pmap. simpl. destruct hd as [|v0 t|v0 r|v0 m|v0 v1|v0 e0|v0 e0|v0|c s1 s2] eqn : Hstmt; subst hd; simpl in *; try done.
@@ -1654,8 +1705,20 @@ Proof.
   destruct (PVM.find v0 pmap); try done; destruct (Sem_HiFP.type_of_hfexpr (clock r) pmap); try done; destruct r; try done; 
     destruct (HiFirrtl.type {| type := type; clock := clock; reset := reset |}); try done.
   destruct (PVM.find v0 pmap); try done; destruct (Sem_HiFP.type_of_hfexpr e0 pmap); try done.
-  admit. (* when *)
-Admitted.
+  rewrite (stmts_tmap_component_stmts_of_eq s1). rewrite -stmts_tmap_qcat. rewrite -stmts_tmap_qcat.
+  destruct (Sem_HiFP.stmts_tmap' pmap (component_stmts_of s1)) as [tmap_true|]; try done.
+  rewrite (stmts_tmap_component_stmts_of_eq s2). destruct (Sem_HiFP.stmts_tmap' tmap_true (component_stmts_of s2)) as [tmap_false|]; try done.
+
+  clear stmt_tmap_component_stmts_of_eq. destruct s as [|v0 t|v0 r|v0 m|v0 v1|v0 e0|v0 e0|v0|c s1 s2] eqn : Hstmt; subst s; simpl in *; try done.
+  (* wire *)
+  destruct t as [gt|a b|a b]; try done. destruct (PVM.find v0 pmap); try done.
+  (* reg *)
+  destruct (PVM.find v0 pmap); try done. destruct (Sem_HiFP.type_of_hfexpr (clock r) pmap); try done. destruct (type r); try done.
+  (* node *)
+  destruct (PVM.find v0 pmap); destruct (Sem_HiFP.type_of_hfexpr e0 pmap); try done.
+  (* when *)
+  rewrite stmts_tmap_component_stmts_of_eq. rewrite -stmts_tmap_qcat. destruct (Sem_HiFP.stmts_tmap' pmap (component_stmts_of s1)); try done.
+Qed.
 
 Lemma stmts_tmap_qcat_convert_to_connect_stmts_eq ss cncts pmap : (forall s, Qin s cncts -> is_connection s) ->
   Sem_HiFP.stmts_tmap' pmap (Qcat ss cncts) = Sem_HiFP.stmts_tmap' pmap ss.
@@ -1679,17 +1742,31 @@ Proof.
   apply convert_to_connect_stmts_is_connection.
 Qed.
 
-Lemma init_dclrs_component_stmts_of_eq ss valmap tmap : Sem_HiFP.init_dclrs ss valmap tmap = Sem_HiFP.init_dclrs (component_stmts_of ss) valmap tmap.
+Lemma init_dclrs_qcat valmap tmap s1 s2 : match Sem_HiFP.init_dclrs s1 valmap tmap with
+  | Some valmap' => Sem_HiFP.init_dclrs s2 valmap' tmap 
+  | _ => None
+  end = Sem_HiFP.init_dclrs (Qcat s1 s2) valmap tmap.
+Proof. 
+  move : s1 tmap valmap s2. elim; simpl in *; try done.
+  intros hd tl IH tmap valmap s2. destruct (Sem_HiFP.init_dclr hd valmap tmap) as [valmap'|]; try done.
+Qed.
+
+Lemma init_dclrs_component_stmts_of_eq ss valmap tmap : Sem_HiFP.init_dclrs ss valmap tmap = Sem_HiFP.init_dclrs (component_stmts_of ss) valmap tmap
+with init_dclr_component_stmt_of_eq s valmap tmap : Sem_HiFP.init_dclr s valmap tmap = Sem_HiFP.init_dclrs (component_stmt_of s) valmap tmap.
 Proof.
   move : ss valmap; elim. simpl; done.
-  intros hd tl IH valmap. simpl. destruct hd as [|v0 t|v0 r|v0 m|v0 v1|v0 e0|v0 e0|v0|c s1 s2] eqn : Hstmt; subst hd; simpl in *; try done.
+  intros hd tl IH valmap. simpl. rewrite (init_dclr_component_stmt_of_eq hd). rewrite -init_dclrs_qcat.
+  destruct (Sem_HiFP.init_dclrs (component_stmt_of hd) valmap tmap); try done.
+  
+  clear init_dclr_component_stmt_of_eq.
+  destruct s as [|v0 t|v0 r|v0 m|v0 v1|v0 e0|v0 e0|v0|c s1 s2] eqn : Hstmt; subst s; simpl in *; try done.
   destruct t; try done.
-  destruct (Sem_HiFP.eval_hfexpr e0 valmap tmap); try done. 
-  admit. (* when *)
-Admitted.
+  destruct (Sem_HiFP.eval_hfexpr e0 valmap tmap); try done.
+  rewrite (init_dclrs_component_stmts_of_eq s1). rewrite -init_dclrs_qcat. destruct (Sem_HiFP.init_dclrs (component_stmts_of s1) valmap tmap); try done.
+Qed.
 
 Lemma init_dclrs_convert_to_connect_stmts_eq ss cncts valmap tmap : (forall s, Qin s cncts -> is_connection s) ->
-  Sem_HiFP.init_dclrs (Qcat ss cncts) valmap tmap  = Sem_HiFP.init_dclrs ss valmap tmap.
+  Sem_HiFP.init_dclrs (Qcat ss cncts) valmap tmap = Sem_HiFP.init_dclrs ss valmap tmap.
 Proof.
   intro. move : ss valmap. elim. simpl. intro; move : cncts H. elim. simpl; done.
   simpl; intros. assert (is_connection h). apply H0. simpl. specialize (hfstmt_eqn_refl h) as Heq. move/eqP : Heq => Heq. 
@@ -1699,14 +1776,14 @@ Proof.
   simpl; intros. destruct (Sem_HiFP.init_dclr h valmap tmap); try done.
 Qed.
 
-Lemma component_stmts_of_init_dclrs_eq ss valmap tmap init_s : Sem_HiFP.init_dclrs ss valmap tmap = Some init_s ->
-  forall conn_map, Sem_HiFP.init_dclrs (Qcat (component_stmts_of ss) (convert_to_connect_stmts conn_map)) valmap tmap = Some init_s.
+Lemma component_stmts_of_init_dclrs_eq ss valmap tmap : 
+  forall conn_map, Sem_HiFP.init_dclrs (Qcat (component_stmts_of ss) (convert_to_connect_stmts conn_map)) valmap tmap = Sem_HiFP.init_dclrs ss valmap tmap.
 Proof.
   intros. specialize convert_to_connect_stmts_is_connection as Hcncts. specialize (Hcncts conn_map).
   rewrite init_dclrs_convert_to_connect_stmts_eq; try done. rewrite -init_dclrs_component_stmts_of_eq //.
 Qed.
 
-Lemma PVM_equal_iff_find_eq (m1 m2 : PVM.t bits) : PVM.equal (fun val1 val2 : bitseq => val1 == val2) m1 m2 <-> (forall v, PVM.find v m1 = PVM.find v m2).
+(*Lemma PVM_equal_iff_find_eq (m1 m2 : PVM.t bits) : PVM.equal (fun val1 val2 : bitseq => val1 == val2) m1 m2 <-> (forall v, PVM.find v m1 = PVM.find v m2).
 Proof.
 Admitted.
 
@@ -1730,82 +1807,101 @@ Lemma update_values_equal : forall ns1 ns2 s,
   PVM.equal (fun v1 v2 : bitseq => v1 == v2) ns1 ns2 ->
   PVM.equal (fun v1 v2 : bitseq => v1 == v2) (Sem_HiFP.update_values ns1 s) (Sem_HiFP.update_values ns2 s).
 Proof.
-Admitted.
+Admitted.*)
 
-Lemma update_values_equal' : forall ns s1 s2,
-  PVM.equal (fun v1 v2 : bitseq => v1 == v2) s1 s2 ->
-  PVM.equal (fun v1 v2 : bitseq => v1 == v2) (Sem_HiFP.update_values ns s1) (Sem_HiFP.update_values ns s2).
-Proof.
+Definition pvm_included (m1 m2 : PVM.t bits) : Prop :=
+  forall k v1, 
+    PVM.find k m1 = Some v1 -> 
+    PVM.find k m2 = Some v1.
+
+Lemma included_update_values_included : forall s1 s2 ns1 ns2,
+  (*forall v, PVM.mem v s1 -> ~ PVM.mem v ns1 -> ~ PVM.mem v ns2) ->*)
+  pvm_included s1 s2 -> pvm_included ns1 ns2 ->
+  pvm_included (Sem_HiFP.update_values ns1 s1) (Sem_HiFP.update_values ns2 s2).
+Proof. (* TBD *)
+  unfold pvm_included, Sem_HiFP.update_values in *; intros s1 s2 ns1 ns2 (*Hypo*) Hinclude_s Hinclude_ns v bs Hfind. 
+  assert (Hfind' : PVM.find v ns1 = Some bs \/ (PVM.find v ns1 = None /\ PVM.find v s1 = Some bs)). admit.
+  destruct Hfind' as [Hfind'|Hfind'].
+  - (* in ns *)
+    apply Hinclude_ns in Hfind'. admit.
+  - (* not in ns *)
+    (* 不在ns1,但在s1的，是input或未被连接的reg，那么ns2也没有 *)
 Admitted.
 
 Definition func_type : Type := PVM.t bits -> PVM.t bits -> PVM.t bits -> PVM.t (fgtyp * fcomponent) -> option (PVM.t bits * PVM.t bits).
-Definition func_type_eq (fun1 fun2 : func_type) (tmap : PVM.t (fgtyp * fcomponent)) : Prop := forall (init_s1 init_s2 : PVM.t bits) (s1 s2 rs1 rs2 : PVM.t bits),
-  PVM.equal (fun val1 val2 : bitseq => val1 == val2) init_s1 init_s2 -> fun1 (PVM.empty bits) (PVM.empty bits) init_s1 tmap = Some (rs1, s1) -> fun2 (PVM.empty bits) (PVM.empty bits) init_s2 tmap = Some (rs2, s2) -> 
-  (forall v, PVM.find v s1 = PVM.find v s2) /\ (forall v, PVM.find v rs1 = PVM.find v rs2).
+Definition func_type_included (fun1 fun2 : func_type) (tmap : PVM.t (fgtyp * fcomponent)) : Prop := forall (init_s1 init_s2 : PVM.t bits) (s1 s2 rs1 rs2 : PVM.t bits),
+  pvm_included init_s1 init_s2 -> fun1 (PVM.empty bits) (PVM.empty bits) init_s1 tmap = Some (rs1, s1) -> fun2 (PVM.empty bits) (PVM.empty bits) init_s2 tmap = Some (rs2, s2) -> 
+  (pvm_included s1 s2) /\ (pvm_included rs1 rs2).
 
-Lemma iterate_func_eq n fun1 fun2 init_s1 init_s2 tmap sem sem_new : 
-  func_type_eq fun1 fun2 tmap -> PVM.equal (fun val1 val2 : bitseq => val1 == val2) init_s1 init_s2 -> Sem_HiFP.iterate n fun1 init_s1 tmap = Some sem -> Sem_HiFP.iterate n fun2 init_s2 tmap = Some sem_new -> 
-  (forall v, PVM.find v sem = PVM.find v sem_new).
+Lemma iterate_func_included n fun1 fun2 init_s1 init_s2 tmap sem sem_new : 
+  func_type_included fun1 fun2 tmap -> pvm_included init_s1 init_s2 -> Sem_HiFP.iterate n fun1 init_s1 tmap = Some sem -> Sem_HiFP.iterate n fun2 init_s2 tmap = Some sem_new -> 
+  pvm_included sem sem_new.
 Proof.
-  intros Hfun_eq. revert init_s1 init_s2 sem sem_new. 
+  intros Hfun_included. move : init_s1 init_s2 sem sem_new. 
   induction n as [|n IH]; intros init_s1 init_s2 sem sem_new Hinit_eq Hiter1 Hiter2.
   - (* Case n = 0 *)
     simpl in Hiter1, Hiter2.
-    inversion Hiter1; inversion Hiter2. subst sem sem_new. apply PVM_equal_iff_find_eq. done.
+    inversion Hiter1; inversion Hiter2. subst sem sem_new; done.
   - (* Case n = S n' *)
     simpl in Hiter1, Hiter2.
     destruct (fun1 (PVM.empty bits) (PVM.empty bits) init_s1 tmap) as [[rs1 ns1]|] eqn:Hcall1;
       [|discriminate].
     destruct (fun2 (PVM.empty bits) (PVM.empty bits) init_s2 tmap) as [[rs2 ns2]|] eqn:Hcall2;
       [|discriminate].
-    specialize (Hfun_eq init_s1 init_s2 ns1 ns2 rs1 rs2).
-    specialize (Hfun_eq Hinit_eq Hcall1 Hcall2). move : Hfun_eq => [Hfun_eq _]. 
-    simpl in Hfun_eq. 
-    apply PVM_equal_iff_find_eq in Hfun_eq. generalize Hfun_eq; intro Hns_eq. apply update_values_equal with (s := init_s1) in Hfun_eq.
-    destruct (PVM.equal (fun val1 val2 : bitseq => val1 == val2)
-             (Sem_HiFP.update_values ns1 init_s1) init_s1) eqn:Hfp1.
-    + (* 达到不动点 *)
-      apply PVM_equal_iff_find_eq. inversion Hiter1; subst sem; clear Hiter1.
-      specialize (update_values_equal' ns2 Hinit_eq) as Hhelper. apply (PVM_equal_trans Hfun_eq) in Hhelper.
-      apply PVM_equal_comm in Hfp1. apply (PVM_equal_trans Hfp1) in Hhelper. apply PVM_equal_comm in Hhelper. 
-      apply (PVM_equal_trans Hhelper) in Hinit_eq. rewrite Hinit_eq in Hiter2. inversion Hiter2; subst sem_new; clear Hiter2.
-      apply PVM_equal_comm. apply (PVM_equal_trans Hhelper Hfp1).
-    + (* 未达到不动点 *)
-      assert (Hfalse : ~ PVM.equal (fun val1 val2 : bitseq => val1 == val2) (Sem_HiFP.update_values ns2 init_s2) init_s2).
-        intro Hneg. specialize (update_values_equal' ns2 Hinit_eq) as Hhelper. apply (PVM_equal_trans Hfun_eq) in Hhelper.
-        apply (PVM_equal_trans Hhelper) in Hneg. apply not_true_iff_false in Hfp1. apply (PVM_non_equal_trans Hfp1) in Hinit_eq. 
-        done.
-      apply not_true_iff_false in Hfalse. rewrite Hfalse in Hiter2.
-      move : Hiter1 Hiter2; apply IH.
-      specialize (update_values_equal' ns2 Hinit_eq) as Hhelper. apply (PVM_equal_trans Hfun_eq) in Hhelper. 
-      done.
+    unfold func_type_included in Hfun_included. specialize (Hfun_included init_s1 init_s2 ns1 ns2 rs1 rs2).
+    specialize (Hfun_included Hinit_eq Hcall1 Hcall2). move : Hfun_included => [Hfun_included _]. 
+    move : Hiter1 Hiter2; apply IH.
+    move : Hinit_eq Hfun_included; apply included_update_values_included.
 Qed.
 
 Definition unique_node_dclr (ss : HiFP.hfstmt_seq) : Prop :=
-  forall v e, Qin (Snode v e) ss -> (forall v' e', Qin (Snode v' e') ss -> v <> v') /\ (forall e', ~ Qin (Sfcnct (Eid v) e') ss) /\ (forall v', Qin (Sinvalid (Eid v')) ss -> v <> v').
+  forall v e, Qin (Snode v e) ss -> (forall v' e', Qin (Snode v' e') (Qremove (Snode v e) ss) -> v <> v') /\ (forall e', ~ Qin (Sfcnct (Eid v) e') ss) /\ (forall v', Qin (Sinvalid (Eid v')) ss -> v <> v').
+
+Definition unique_node_dclr_when (ss : HiFP.hfstmt_seq) : Prop :=
+  forall v e, Qin_when (Snode v e) ss -> 
+  (forall v' e', Qin_when (Snode v' e') (Qremove_when (Snode v e) ss) -> v <> v') /\ (forall e', ~ Qin_when (Sfcnct (Eid v) e') ss) /\ (forall v', Qin_when (Sinvalid (Eid v')) ss -> v <> v').
+
+Fixpoint Qin_with_cond (s : HiFP.hfstmt) (ss : HiFP.hfstmt_seq) init_s tmap : bool :=
+match ss with 
+| Qnil => false
+| Qcons (Swhen c s1 s2) tl => match Sem_HiFP.eval_hfexpr c init_s tmap with
+    | Some valc => if (~~ is_zero valc) then (Qin_with_cond s s1 init_s tmap) || (Qin_with_cond s tl init_s tmap)
+                   else (Qin_with_cond s s2 init_s tmap) || (Qin_with_cond s tl init_s tmap)
+    | _ => false
+    end
+| Qcons h tl => (hfstmt_eqn h s) || (Qin_with_cond s tl init_s tmap)
+end.
 
 Lemma eval_hfstmts_unique_ss_find_eq ss rs0 ns0 init_s tmap rs s v : 
   (forall v' e', Qin (Snode v' e') ss -> v <> v') -> (forall e', ~ Qin (Sfcnct (Eid v) e') ss) -> (forall v', Qin (Sinvalid (Eid v')) ss -> v <> v') ->
+  (forall c ss1 ss2, ~ Qin (Swhen c ss1 ss2) ss) ->
   Sem_HiFP.eval_hfstmts ss rs0 ns0 init_s tmap = Some (rs, s) -> PVM.find v s = PVM.find v ns0
 with eval_hfstmt_unique_ss_find_eq st rs0 ns0 init_s tmap rs s v : match st with
   | Snode v' _ => v <> v'
   | Sfcnct (Eid v') _ => v <> v'
   | Sinvalid (Eid v') => v <> v'
+  | Swhen _ _ _ => false
   | _ => True
   end ->
   Sem_HiFP.eval_hfstmt st rs0 ns0 init_s tmap = Some (rs, s) -> PVM.find v s = PVM.find v ns0.
 Proof.
-  clear eval_hfstmts_unique_ss_find_eq. move : ss rs0 ns0. elim. simpl; intros. inversion H2; subst s; done.
-  intros hd tl IH. simpl; intros rs0 ns0 Hnode Hcnct Hinvalid Hevals. destruct (Sem_HiFP.eval_hfstmt hd rs0 ns0 init_s tmap) as [[rs1 ns1]|] eqn : Heval; try discriminate.
+  clear eval_hfstmts_unique_ss_find_eq. move : ss rs0 ns0. elim. simpl; intros. inversion H3; subst s; done.
+  intros hd tl IH. simpl; intros rs0 ns0 Hnode Hcnct Hinvalid Hwhen Hevals. destruct (Sem_HiFP.eval_hfstmt hd rs0 ns0 init_s tmap) as [[rs1 ns1]|] eqn : Heval; try discriminate.
   apply IH in Hevals; clear IH. rewrite Hevals. move : Heval; apply eval_hfstmt_unique_ss_find_eq.
   case Hst : hd => [||var reg|||var node_e|ref e|ref|cond ss_true ss_false]; subst hd; try done.
   - (* node *) move : Hnode; clear. intro. apply (Hnode _ node_e). simpl. rewrite eq_refl. rewrite eq_refl //.
   - (* cnct *) move : Hcnct; clear. intros. specialize (Hcnct e). destruct ref; try done. move : Hcnct; apply contra_not. intro; subst v. 
     simpl. rewrite eq_refl. rewrite eq_refl //.
   - (* invalid *) move : Hinvalid; clear. intro. destruct ref; try done. apply Hinvalid. simpl. rewrite eq_refl orb_true_l //.
+  - (* when *) specialize (Hwhen cond ss_true ss_false); simpl in Hwhen. rewrite eq_refl in Hwhen; simpl in Hwhen. 
+    specialize (hfstmt_seq_eqn_refl ss_true) as Heq. move/eqP : Heq => Heq. specialize (hfstmt_seq_eqP ss_true ss_true) as Heq'. apply reflect_iff in Heq'.
+    apply Heq' in Heq. rewrite Heq in Hwhen; simpl in Hwhen. clear Heq Heq'.
+    specialize (hfstmt_seq_eqn_refl ss_false) as Heq. move/eqP : Heq => Heq. specialize (hfstmt_seq_eqP ss_false ss_false) as Heq'. apply reflect_iff in Heq'.
+    apply Heq' in Heq. rewrite Heq in Hwhen; simpl in Hwhen. done.
   - (* node *) move : Hnode; clear. intros. apply (Hnode _ e'). rewrite H orb_true_r //.
   - (* cnct *) move : Hcnct; clear. intros. specialize (Hcnct e'). move : Hcnct; apply contra_not. intro. rewrite H orb_true_r //. 
   - (* invalid *) move : Hinvalid; clear. intros. apply Hinvalid. rewrite H orb_true_r //.
+  - (* when *) intros. specialize (Hwhen c ss1 ss2). move : Hwhen; apply contra_not; intro. rewrite H orb_true_r //.
 
   clear eval_hfstmt_unique_ss_find_eq. case Hst : st => [||var reg|||var node_e|ref e|ref|cond ss_true ss_false]; subst st. 
   (* skip, wire *) 
@@ -1825,16 +1921,14 @@ Proof.
   destruct (PVM.find s0 tmap) as [[gt cmpnt]|]; try discriminate. 
   destruct cmpnt; destruct (sizeof_fgtyp gt < length indeterminate_val); try (inversion Heval; subst rs s; try done).
   1-14 : rewrite PVM.Lemmas.find_add_neq //. 1-14 : unfold PVM.M.SE.eq; move : Hneq; apply contra_not; intro; move /eqP : H => H; done.
-  (* when *)
-  (*simpl; intros _ Heval. destruct (Sem_HiFP.eval_hfexpr cond init_s tmap); try discriminate. destruct (~~ is_zero b).
-  move : Heval. apply eval_hfstmts_unique_ss_find_eq. admit.*) admit. (* when 的情况还未体现在unique_node_dclr TBD *)
-Admitted.
+  (* when *) intro; done.
+Qed.
 
-Lemma eval_hfstmts_for_unique_node ss v e : 
-  Qin (Snode v e) ss -> unique_node_dclr ss -> 
+Lemma eval_hfstmts_for_unique_node' ss v e : 
+  Qin (Snode v e) ss -> unique_node_dclr ss -> (forall c ss1 ss2, ~ Qin (Swhen c ss1 ss2) ss) ->
   forall init_s tmap rs s, Sem_HiFP.eval_hfstmts ss (PVM.empty bits) (PVM.empty bits) init_s tmap = Some (rs, s) -> PVM.find v s = Sem_HiFP.eval_hfexpr e init_s tmap.
 Proof.
-  intros Hin Hunique init_s tmap.
+  intros Hin Hunique Hwhen init_s tmap.
   assert (Hhelper : forall rs0 ns0, PVM.find v ns0 = None -> forall rs s : PVM.t bits,
     Sem_HiFP.eval_hfstmts ss rs0 ns0 init_s tmap = Some (rs, s) ->
     PVM.find v s = Sem_HiFP.eval_hfexpr e init_s tmap). {
@@ -1849,23 +1943,28 @@ Proof.
         unfold unique_node_dclr in Hunique. assert (Hin : Qin (Snode v e) (Qcons (Snode v e) ss)) by (simpl; rewrite eq_refl; rewrite eq_refl //).
         apply Hunique in Hin; clear Hunique. move : Hin => [Hnode [Hcnct Hinvalid]]. 
         apply eval_hfstmts_unique_ss_find_eq with (v := v) in Heval. rewrite PVM.Lemmas.find_add_eq in Heval. done. apply PVM.M.SE.eq_refl.
-        (* node *) intros; apply (Hnode _ e'). simpl. rewrite H orb_true_r //.
+        (* node *) simpl in Hnode. intros; apply (Hnode _ e'). rewrite eq_refl; simpl. rewrite eq_refl; simpl; done.
         (* cnct *) intro. specialize (Hcnct e'). move : Hcnct; apply contra_not. intro. simpl; rewrite H //.
         (* invalid *) intros; apply Hinvalid. simpl. done.
+        (* when *) intros. specialize (Hwhen c ss1 ss2). move : Hwhen; apply contra_not; intro. simpl; done.
       + rewrite orb_false_l in Hin. 
         destruct (Sem_HiFP.eval_hfstmt s rs0 ns0 init_s tmap) as [[rs1 ns1]|] eqn : Hevals; try discriminate.
-        move : Heval. apply (IH Hin). move : Hunique Hs; clear.
+        move : Heval. apply (IH Hin). 
+        move : Hunique Hs; clear.
         { unfold unique_node_dclr in *; intros.
           assert (Qin (Snode v0 e0) (Qcons s ss)). simpl. rewrite H orb_true_r //.
           specialize (Hunique _ _ H0). move : Hunique => [Hunique0 [Hunique1 Hunique2]]. split.
-          intros. apply (Hunique0 _ e'). simpl. rewrite H1 orb_true_r //. split.
+          intros. apply (Hunique0 _ e'). simpl. destruct (hfstmt_eqn s (Snode v0 e0)). move : H1; apply in_qremove. simpl; rewrite H1 orb_true_r //. split.
           intros. specialize (Hunique1 e'). move : Hunique1; apply contra_not.
           simpl; intros. rewrite H1 orb_true_r //.
           intros. apply Hunique2. simpl. rewrite H1 orb_true_r //. }
+        { intros. specialize (Hwhen c ss1 ss2). move : Hwhen; apply contra_not; intro. simpl. rewrite H orb_true_r //. }
         { unfold unique_node_dclr in Hunique. 
           assert (Qin (Snode v e) (Qcons s ss)). simpl. rewrite Hin orb_true_r //.
           specialize (Hunique v e H).
-          move : Hevals Hnone Hs Hunique; clear; intros. destruct s as [|v0 t|v0 r|v0 m|v0 v1|v0 e0|v0 e0|v0|c s1 s2] eqn : Hstmt; subst s; simpl in Hevals.
+          assert (Hwhen' : forall c ss1 ss2, ~ hfstmt_eqn s (Swhen c ss1 ss2)).
+          intros. specialize (Hwhen c ss1 ss2). move : Hwhen; apply contra_not; intro. simpl. rewrite H0 orb_true_l //.
+          move : Hevals Hnone Hs Hunique Hwhen'; clear; intros. destruct s as [|v0 t|v0 r|v0 m|v0 v1|v0 e0|v0 e0|v0|c ss1 ss2] eqn : Hstmt; subst s; simpl in Hevals.
           * (* skip, wire, mem, inst *)
             1,2,4,5 : inversion Hevals; subst rs1 ns1; done.
           * (* reg *)
@@ -1875,7 +1974,7 @@ Proof.
             move : Hunique => [Hunique _].
             destruct (Sem_HiFP.eval_hfexpr e0 init_s tmap); try discriminate.
             inversion Hevals; subst rs1 ns1; rewrite PVM.Lemmas.find_add_neq //.
-            assert (Qin (Snode v0 e0) (Qcons (Snode v0 e0) ss)). simpl. rewrite eq_refl. rewrite eq_refl. simpl; done.
+            assert (Qin (Snode v0 e0) (Qremove (Snode v e) (Qcons (Snode v0 e0) ss))). simpl; simpl in Hs; rewrite Hs. simpl. rewrite eq_refl. rewrite eq_refl. simpl; done.
             specialize (Hunique _ _ H).
             unfold PVM.M.SE.eq. move : Hunique; apply contra_not. intro. move /eqP : H0 => H0; done.
           * (* cnct *)
@@ -1896,10 +1995,377 @@ Proof.
             assert (Hnoteq : v <> ref). apply Hunique. simpl. rewrite eq_refl orb_true_l //.
             destruct cmpnt; destruct (sizeof_fgtyp gt < length indeterminate_val); inversion Hevals; subst rs1 ns1; try done.
             1-14 : rewrite PVM.Lemmas.find_add_neq //. 1-14 : unfold PVM.M.SE.eq; move : Hnoteq; apply contra_not; intro; move /eqP : H => H; done.
-          * (* when *) admit. }
+          * (* when *) specialize (Hwhen' c ss1 ss2); simpl in Hwhen'. rewrite eq_refl in Hwhen'; simpl in Hwhen'. 
+            specialize (hfstmt_seq_eqn_refl ss1) as Heq. move/eqP : Heq => Heq. specialize (hfstmt_seq_eqP ss1 ss1) as Heq'. apply reflect_iff in Heq'.
+            apply Heq' in Heq. rewrite Heq in Hwhen'; simpl in Hwhen'. clear Heq Heq'.
+            specialize (hfstmt_seq_eqn_refl ss2) as Heq. move/eqP : Heq => Heq. specialize (hfstmt_seq_eqP ss2 ss2) as Heq'. apply reflect_iff in Heq'.
+            apply Heq' in Heq. rewrite Heq in Hwhen'; simpl in Hwhen'. done. }
   }
   apply Hhelper. done.
+Qed.
+
+Lemma eval_hfstmts_unique_when_ss_find_eq ss rs0 ns0 init_s tmap rs s v : 
+  (forall v' e', Qin_when (Snode v' e') ss -> v <> v') -> (forall e', ~ Qin_when (Sfcnct (Eid v) e') ss) -> (forall v', Qin_when (Sinvalid (Eid v')) ss -> v <> v') ->
+  Sem_HiFP.eval_hfstmts ss rs0 ns0 init_s tmap = Some (rs, s) -> PVM.find v s = PVM.find v ns0
+with eval_hfstmt_unique_when_ss_find_eq st rs0 ns0 init_s tmap rs s v : match st with
+  | Snode v' _ => v <> v'
+  | Sfcnct (Eid v') _ => v <> v'
+  | Sinvalid (Eid v') => v <> v'
+  | Swhen _ ss1 ss2 => 
+    (forall v' e', Qin_when (Snode v' e') ss1 -> v <> v') /\ (forall e', ~ Qin_when (Sfcnct (Eid v) e') ss1) /\ (forall v', Qin_when (Sinvalid (Eid v')) ss1 -> v <> v') /\
+    (forall v' e', Qin_when (Snode v' e') ss2 -> v <> v') /\ (forall e', ~ Qin_when (Sfcnct (Eid v) e') ss2) /\ (forall v', Qin_when (Sinvalid (Eid v')) ss2 -> v <> v') 
+  | _ => True
+  end ->
+  Sem_HiFP.eval_hfstmt st rs0 ns0 init_s tmap = Some (rs, s) -> PVM.find v s = PVM.find v ns0.
+Proof.
+  clear eval_hfstmts_unique_when_ss_find_eq. move : ss rs0 ns0. elim. simpl; intros. inversion H2; subst s; done.
+  intros hd tl IH. simpl; intros rs0 ns0 Hnode Hcnct Hinvalid Hevals. destruct (Sem_HiFP.eval_hfstmt hd rs0 ns0 init_s tmap) as [[rs1 ns1]|] eqn : Heval; try discriminate.
+  apply IH in Hevals; clear IH. rewrite Hevals. move : Heval; apply eval_hfstmt_unique_when_ss_find_eq.
+  case Hst : hd => [||var reg|||var node_e|ref e|ref|cond ss_true ss_false]; subst hd; try done.
+  - (* node *) move : Hnode; clear. intro. apply (Hnode _ node_e). simpl. rewrite eq_refl. rewrite eq_refl //.
+  - (* cnct *) move : Hcnct; clear. intros. specialize (Hcnct e). destruct ref; try done. move : Hcnct; apply contra_not. intro; subst v. 
+    simpl. rewrite eq_refl. rewrite eq_refl //.
+  - (* invalid *) move : Hinvalid; clear. intro. destruct ref; try done. apply Hinvalid. simpl. rewrite eq_refl orb_true_l //.
+  - (* when *) split. intros; apply (Hnode _ e'). rewrite H //. split.
+    intro. specialize (Hcnct e'). move : Hcnct; apply contra_not; intro. rewrite H //. split.
+    intros; apply Hinvalid. rewrite H //. split.
+    intros; apply (Hnode v' e'). rewrite H orb_true_r orb_true_l //. split.
+    intro. specialize (Hcnct e'). move : Hcnct; apply contra_not; intro. rewrite H orb_true_r orb_true_l //.
+    intros; apply Hinvalid. rewrite H orb_true_r orb_true_l //. 
+    intros. apply (Hnode v' e'). rewrite H; destruct hd; try (rewrite orb_true_r; done); try (rewrite orb_true_r orb_true_l; done).
+    intros. specialize (Hcnct e'). move : Hcnct; apply contra_not; intro. 
+      rewrite H; destruct hd; try (rewrite orb_true_r; done); try (rewrite orb_true_r orb_true_l; done).
+    intros; apply Hinvalid. rewrite H; destruct hd; try (rewrite orb_true_r; done); try (rewrite orb_true_r orb_true_l; done).
+
+  clear eval_hfstmt_unique_when_ss_find_eq. case Hst : st => [||var reg|||var node_e|ref e|ref|cond ss_true ss_false]; subst st. 
+  (* skip, wire *) 
+  1,2,4,5 : simpl; intros _ Heval; inversion Heval; subst rs s; done.
+  (* reg *)
+  simpl; intros _ Heval. destruct (PVM.find var init_s); try discriminate. inversion Heval; subst rs s; done.
+  (* node *)
+  simpl; intros Hneq Heval. destruct (Sem_HiFP.eval_hfexpr node_e init_s tmap); try discriminate. inversion Heval; subst rs s.
+  rewrite PVM.Lemmas.find_add_neq //. unfold PVM.M.SE.eq. move : Hneq; apply contra_not. intro. move /eqP : H => H. done.
+  (* cnct *)
+  simpl; intros Hneq Heval. destruct ref; try (inversion Heval; subst rs s; done).
+  destruct (PVM.find s0 tmap) as [[gt cmpnt]|]; try discriminate. 
+  destruct cmpnt; destruct (Sem_HiFP.eval_hfexpr e init_s tmap); try discriminate; try (inversion Heval; subst rs s; try done).
+  1-7 : rewrite PVM.Lemmas.find_add_neq //. 1-7 : unfold PVM.M.SE.eq; move : Hneq; apply contra_not; intro; move /eqP : H => H; done.
+  (* invalid *)
+  simpl; intros Hneq Heval. destruct ref; try (inversion Heval; subst rs s; done).
+  destruct (PVM.find s0 tmap) as [[gt cmpnt]|]; try discriminate. 
+  destruct cmpnt; destruct (sizeof_fgtyp gt < length indeterminate_val); try (inversion Heval; subst rs s; try done).
+  1-14 : rewrite PVM.Lemmas.find_add_neq //. 1-14 : unfold PVM.M.SE.eq; move : Hneq; apply contra_not; intro; move /eqP : H => H; done.
+  (* when *) intros [Hnode_true [Hcnct_true [Hinvalid_true [Hnode_false [Hcnct_false Hinvalid_false]]]]] Heval. simpl in Heval.
+  destruct (Sem_HiFP.eval_hfexpr cond init_s tmap) as [valc|]; try discriminate. destruct (~~ is_zero valc).
+  1,2 :move : Heval; apply eval_hfstmts_unique_when_ss_find_eq; try done.
+Qed.
+
+Lemma unique_node_dclr_when_subseq s ss : unique_node_dclr_when (Qcons s ss) -> unique_node_dclr_when ss.
+Proof.
+  unfold unique_node_dclr_when; intros. assert (Hin : Qin_when (Snode v e) (Qcons s ss)). simpl. rewrite H0.
+  destruct s; try (rewrite orb_true_r; done); try (rewrite orb_true_r orb_true_l; done).
+  apply H in Hin. move : Hin => [Hnode [Hcnct Hinvalid]]. split.
+  intros; apply (Hnode v' e'). simpl. destruct s; simpl; try done. destruct ((s == v) && (h == e)); try done.
+  move : H1; apply Qremove_when_Qin_when. simpl; rewrite H1 orb_true_r //.
+  destruct (Qin_when (Snode v e) h0). apply Qremove_when_Qin_when in H1. move : H1; apply Qin_when_Qcons.
+  destruct (Qin_when (Snode v e) h1). apply Qremove_when_Qin_when in H1. move : H1; apply Qin_when_Qcons.
+  move : H1; apply Qin_when_Qcons.
+  split. intros. specialize (Hcnct e'). move : Hcnct; apply contra_not; intro; simpl. rewrite H1.
+  destruct s; try (rewrite orb_true_r; done); try (rewrite orb_true_r orb_true_l; done).
+  intros. apply Hinvalid. simpl. rewrite H1.
+  destruct s; try (rewrite orb_true_r; done); try (rewrite orb_true_r orb_true_l; done).
+Qed.
+
+Lemma unique_node_dclr_when_branches c ss1 ss2 ss : unique_node_dclr_when (Qcons (Swhen c ss1 ss2) ss) -> unique_node_dclr_when ss1 /\ unique_node_dclr_when ss2.
+Proof. 
+  unfold unique_node_dclr_when; intros. split.
+  intros. assert (Hin : Qin_when (Snode v e) (Qcons (Swhen c ss1 ss2) ss)). simpl. rewrite H0 //.
+  apply H in Hin; clear H. move : Hin => [Hnode [Hcnct Hinvalid]]. split.
+  intros; apply (Hnode v' e'). simpl.
+  destruct (Qin_when (Snode v e) ss1). simpl. rewrite H //.
+  destruct (Qin_when (Snode v e) ss2). simpl. apply Qremove_when_Qin_when in H. rewrite H //.
+  simpl. apply Qremove_when_Qin_when in H. rewrite H //. split.
+  intros. specialize (Hcnct e'). move : Hcnct; apply contra_not; intro; simpl. rewrite H //.
+  intros. apply Hinvalid. simpl. rewrite H //.
+
+  intros. assert (Hin : Qin_when (Snode v e) (Qcons (Swhen c ss1 ss2) ss)). simpl. rewrite H0 orb_true_r //.
+  apply H in Hin; clear H. move : Hin => [Hnode [Hcnct Hinvalid]]. split.
+  intros; apply (Hnode v' e'). simpl.
+  destruct (Qin_when (Snode v e) ss1). simpl. apply Qremove_when_Qin_when in H. rewrite H orb_true_r //.
+  destruct (Qin_when (Snode v e) ss2). simpl. rewrite H orb_true_r //.
+  simpl. apply Qremove_when_Qin_when in H. rewrite H orb_true_r //. split.
+  intros. specialize (Hcnct e'). move : Hcnct; apply contra_not; intro; simpl. rewrite H orb_true_r //.
+  intros. apply Hinvalid. simpl. rewrite H orb_true_r //.
+Qed.
+
+Lemma Qin_with_cond2Qin_when s ss init_s tmap : Qin_with_cond s ss init_s tmap -> Qin_when s ss.
+Proof.
+  move : ss; elim. simpl; done.
+  intros hd tl IH Hin. unfold Qin_with_cond in Hin. unfold Qin_when. 
+  case Hhd : hd => [||var reg|||var node_e|ref e|ref|cond ss_true ss_false]; try rewrite -Hhd.
+  1-8 : destruct (hfstmt_eqn hd s) eqn : Heq; try (rewrite orb_true_l; done). 
+  1-8 : rewrite orb_false_l; subst hd; rewrite orb_false_l in Hin.
 Admitted.
+
+Lemma Qin_when_uniqie_False v e ss e' cond ss_true ss_false : (forall (v' : ProdVarOrder.T) (e' : hfexpr ProdVarOrder.T),
+  Qin_when (Snode v' e')
+    (Qremove_when (Snode v e) (Qcons (Swhen cond ss_true ss_false) ss)) ->
+  v <> v') -> Qin_when (Snode v e) ss -> Qin_when (Snode v e') ss_true \/ Qin_when (Snode v e') ss_false -> False.
+Proof.
+Admitted.
+
+Lemma eval_hfstmts_for_unique_node_helper ss v e init_s tmap : 
+  Qin_with_cond (Snode v e) ss init_s tmap -> unique_node_dclr_when ss -> 
+  forall rs0 ns0, PVM.find v ns0 = None -> forall rs s,
+  Sem_HiFP.eval_hfstmts ss rs0 ns0 init_s tmap = Some (rs, s) ->
+  PVM.find v s = Sem_HiFP.eval_hfexpr e init_s tmap
+with eval_hfstmt_for_unique_node s v e init_s tmap : 
+  forall rs0 ns0, PVM.find v ns0 = None -> forall rs ns,
+  Sem_HiFP.eval_hfstmt s rs0 ns0 init_s tmap = Some (rs, ns) ->
+  match s with
+  | Swhen c ss1 ss2 => match Sem_HiFP.eval_hfexpr c init_s tmap with
+    | Some valc => unique_node_dclr_when ss1 /\ unique_node_dclr_when ss2 /\
+      if (~~ is_zero valc) then Qin_with_cond (Snode v e) ss1 init_s tmap
+      else Qin_with_cond (Snode v e) ss2 init_s tmap 
+    | _ => True
+    end
+  | Snode v0 e0 => (v == v0) && (e == e0)
+  | _ => False
+  end -> PVM.find v ns = Sem_HiFP.eval_hfexpr e init_s tmap.
+Proof.
+  clear eval_hfstmts_for_unique_node_helper. move : ss; elim. simpl; intros; done.
+  intros s ss IH Hin Hunique rs0 ns0 Hfind rs ns Hevals.
+  simpl in Hevals. destruct (Sem_HiFP.eval_hfstmt s rs0 ns0 init_s tmap) as [[rs1 ns1]|] eqn : Heval; try discriminate. 
+  simpl in Hin.
+  case Hst : s => [||var reg|||var node_e|var cnct_e|var|cond ss_true ss_false]; subst s.
+  + (* skip *) simpl in Heval; inversion Heval; subst rs0 ns0. move : Hevals; apply (IH Hin); try (move : Hunique; apply unique_node_dclr_when_subseq); try done.
+  + (* wire *) simpl in Heval; inversion Heval; subst rs0 ns0. move : Hevals; apply (IH Hin); try (move : Hunique; apply unique_node_dclr_when_subseq); try done.
+  + (* reg *) simpl in Heval. destruct (PVM.find var init_s); try discriminate.
+    inversion Heval; subst rs1 ns1. move : Hevals; apply (IH Hin); try (move : Hunique; apply unique_node_dclr_when_subseq); try done.
+  + (* mem *) simpl in Heval; inversion Heval; subst rs0 ns0. move : Hevals; apply (IH Hin); try (move : Hunique; apply unique_node_dclr_when_subseq); try done.
+  + (* inst *) simpl in Heval; inversion Heval; subst rs0 ns0. move : Hevals; apply (IH Hin); try (move : Hunique; apply unique_node_dclr_when_subseq); try done.
+  + (* node *) destruct (hfstmt_eqn (Snode var node_e) (Snode v e)) eqn : Hs. 
+    - (* s is node *) clear Hin IH eval_hfstmt_for_unique_node. simpl in Hs. 
+      move /andP : Hs => [Hvar Hnode_e]; move /eqP : Hvar => Hvar; move /eqP : Hnode_e => Hnode_e. subst var node_e.
+      unfold unique_node_dclr_when in Hunique. assert (Hin : Qin_when (Snode v e) (Qcons (Snode v e) ss)) by (simpl; rewrite eq_refl; rewrite eq_refl //).
+      apply Hunique in Hin; clear Hunique. move : Hin => [Hnode [Hcnct Hinvalid]]. 
+      simpl in Hcnct. simpl in Hinvalid. simpl in Hnode; rewrite eq_refl in Hnode; simpl in Hnode. rewrite eq_refl in Hnode; simpl in Hnode.
+      apply (eval_hfstmts_unique_when_ss_find_eq Hnode Hcnct Hinvalid) in Hevals.
+      rewrite Hevals. simpl in Heval. destruct (Sem_HiFP.eval_hfexpr e init_s tmap); try discriminate.
+      inversion Heval; subst rs1 ns1. apply PVM.Lemmas.find_add_eq; apply PVM.M.SE.eq_refl.
+    - (* s is in ss *) rewrite orb_false_l in Hin.
+      move : Hevals. apply (IH Hin); try (move : Hunique; apply unique_node_dclr_when_subseq). move : Hunique Hs Hin Heval Hfind; clear; intros.
+      unfold unique_node_dclr_when in Hunique. apply Qin_with_cond2Qin_when in Hin. assert (Qin_when (Snode v e) (Qcons (Snode var node_e) ss)) by (simpl; rewrite Hin orb_true_r //).
+      specialize (Hunique v e H).
+      move : Hunique => [Hunique _]. specialize (Hunique var node_e). simpl in Heval.
+      destruct (Sem_HiFP.eval_hfexpr node_e init_s tmap); try discriminate.
+      inversion Heval; subst rs1 ns1; rewrite PVM.Lemmas.find_add_neq //.
+      simpl in Hunique; simpl in Hs; rewrite Hs in Hunique. simpl in Hunique. 
+      rewrite eq_refl in Hunique; simpl in Hunique. rewrite eq_refl in Hunique; simpl in Hunique.
+      assert (true) by done. apply Hunique in H0.
+      unfold PVM.M.SE.eq. move : H0; apply contra_not. intro. move /eqP : H0 => H0; done.
+  + (* cnct *) simpl in Hin.
+      move : Hevals. apply (IH Hin); try (move : Hunique; apply unique_node_dclr_when_subseq). 
+      move : Hunique Hin Heval Hfind; clear; intros.
+      unfold unique_node_dclr_when in Hunique. apply Qin_with_cond2Qin_when in Hin. assert (Qin_when (Snode v e) (Qcons (Sfcnct var cnct_e) ss)) by (simpl; done).
+      specialize (Hunique v e H). simpl in Heval. destruct var as [ref|a|a|a] eqn : Href; try (inversion Heval; subst rs1 ns1; done).
+      destruct (PVM.find ref tmap) as [[gt cmpnt]|] eqn : Hgt; try discriminate.
+      move : Hunique => [_ [Hunique _]]. specialize (Hunique cnct_e). simpl in Hunique. rewrite eq_refl in Hunique; simpl in Hunique.
+      destruct cmpnt; destruct (Sem_HiFP.eval_hfexpr cnct_e init_s tmap); try discriminate; 
+      inversion Heval; subst rs1 ns1; try done. 1-7 : rewrite PVM.Lemmas.find_add_neq //.
+      1-7 : unfold PVM.M.SE.eq; move : Hunique; apply contra_not; intro; move /eqP : H0 => H0; subst v; rewrite eq_refl; simpl; done.
+  + (* invalid *) simpl in Hin.
+      move : Hevals. apply (IH Hin); try (move : Hunique; apply unique_node_dclr_when_subseq). 
+      move : Hunique Hin Heval Hfind; clear; intros.
+      unfold unique_node_dclr_when in Hunique. apply Qin_with_cond2Qin_when in Hin. assert (Qin_when (Snode v e) (Qcons (Sinvalid var) ss)) by (simpl; done).
+      specialize (Hunique v e H). simpl in Heval. destruct var as [ref|a|a|a] eqn : Href; try (inversion Heval; subst rs1 ns1; done).
+      destruct (PVM.find ref tmap) as [[gt cmpnt]|] eqn : Hgt; try discriminate.
+      move : Hunique => [_ [_ Hunique]]. specialize (Hunique ref). simpl in Hunique. rewrite eq_refl in Hunique; simpl in Hunique.
+      destruct cmpnt; destruct (sizeof_fgtyp gt < length indeterminate_val); 
+      try (inversion Heval; subst rs1 ns1; try done). 1-14 : rewrite PVM.Lemmas.find_add_neq //. 
+      1-14 : assert (true) by done; apply Hunique in H0.
+      1-14 : unfold PVM.M.SE.eq; move : H0; apply contra_not; intro; move /eqP : H0 => H0; subst v; done.
+  + (* when *) specialize (eval_hfstmt_for_unique_node _ _ e _ _ _ _ Hfind _ _ Heval); simpl in eval_hfstmt_for_unique_node.
+    simpl in Heval; destruct (Sem_HiFP.eval_hfexpr cond init_s tmap) as [valc|] eqn : Hc; try discriminate. 
+    destruct (~~ is_zero valc) eqn : Hcond. 
+    - (* go to true *)
+      destruct (Qin_with_cond (Snode v e) ss_true init_s tmap) eqn : Hin_true.
+      * (* node in true, not in ss *)
+        clear IH Hin. rewrite -eval_hfstmt_for_unique_node; try done.
+        unfold unique_node_dclr_when in Hunique. assert (Qin_when (Snode v e) (Qcons (Swhen cond ss_true ss_false) ss)). 
+        apply Qin_with_cond2Qin_when in Hin_true. simpl; rewrite Hin_true orb_true_l //. apply Hunique in H. move : H => [Hnode [Hcnct Hinvalid]].
+        move : Hevals; apply eval_hfstmts_unique_when_ss_find_eq.
+        move : Hnode Hin_true; clear; intros. apply (Hnode v' e'). simpl. apply Qin_with_cond2Qin_when in Hin_true. rewrite Hin_true. apply Qin_when_Qcons; done.
+        intros. move : (Hcnct e'); clear. apply contra_not. apply Qin_when_Qcons; done.
+        intros. apply (Hinvalid v'). move : H; apply Qin_when_Qcons; done.
+        apply unique_node_dclr_when_branches in Hunique. move : Hunique => [Hunique0 Hunique1]. split; try done.
+      * (* in ss *) rewrite orb_false_l in Hin. move : Hevals; apply (IH Hin).
+        move : Hunique; apply unique_node_dclr_when_subseq.
+        unfold unique_node_dclr_when in Hunique. assert (Qin_when (Snode v e) (Qcons (Swhen cond ss_true ss_false) ss)). 
+        apply Qin_with_cond2Qin_when in Hin. apply Qin_when_Qcons; done. apply Hunique in H. move : H => [Hnode [Hcnct Hinvalid]].
+        rewrite -Hfind. move : Heval; apply eval_hfstmts_unique_when_ss_find_eq.
+        move : Hnode Hin; clear; intros. intro; subst v'. apply Qin_with_cond2Qin_when in Hin. 
+        assert (Qin_when (Snode v e') ss_true \/ Qin_when (Snode v e') ss_false) by (left; done).
+        apply (Qin_when_uniqie_False Hnode Hin H0).
+        intros. move : (Hcnct e'); clear. apply contra_not. intro; simpl. rewrite H //.
+        intros. apply (Hinvalid v'). simpl. rewrite H //.
+    - (* go to false *)
+      destruct (Qin_with_cond (Snode v e) ss_false init_s tmap) eqn : Hin_false.
+      * (* node in false, not in ss *)
+        clear IH Hin. rewrite -eval_hfstmt_for_unique_node; try done.
+        unfold unique_node_dclr_when in Hunique. assert (Qin_when (Snode v e) (Qcons (Swhen cond ss_true ss_false) ss)). 
+        apply Qin_with_cond2Qin_when in Hin_false. simpl; rewrite Hin_false orb_true_r //. apply Hunique in H. move : H => [Hnode [Hcnct Hinvalid]].
+        move : Hevals; apply eval_hfstmts_unique_when_ss_find_eq.
+        move : Hnode Hin_false; clear; intros. apply (Hnode v' e'). simpl. apply Qin_with_cond2Qin_when in Hin_false. rewrite Hin_false. 
+        destruct (Qin_when (Snode v e) ss_true); apply Qin_when_Qcons; done.
+        intros. move : (Hcnct e'); clear. apply contra_not. apply Qin_when_Qcons; done.
+        intros. apply (Hinvalid v'). move : H; apply Qin_when_Qcons; done.
+        apply unique_node_dclr_when_branches in Hunique. move : Hunique => [Hunique0 Hunique1]. split; try done.
+        * (* in ss *) rewrite orb_false_l in Hin. move : Hevals; apply (IH Hin).
+        move : Hunique; apply unique_node_dclr_when_subseq.
+        unfold unique_node_dclr_when in Hunique. assert (Qin_when (Snode v e) (Qcons (Swhen cond ss_true ss_false) ss)). 
+        apply Qin_with_cond2Qin_when in Hin. apply Qin_when_Qcons; done. apply Hunique in H. move : H => [Hnode [Hcnct Hinvalid]].
+        rewrite -Hfind. move : Heval; apply eval_hfstmts_unique_when_ss_find_eq.
+        move : Hnode Hin; clear; intros. intro; subst v'. apply Qin_with_cond2Qin_when in Hin. 
+        assert (Qin_when (Snode v e') ss_true \/ Qin_when (Snode v e') ss_false) by (right; done).
+        apply (Qin_when_uniqie_False Hnode Hin H0).
+        intros. move : (Hcnct e'); clear. apply contra_not. intro; simpl. rewrite H orb_true_r //.
+        intros. apply (Hinvalid v'). simpl. rewrite H orb_true_r //.
+  clear eval_hfstmt_for_unique_node.
+  intros rs0 ns0 Hfind rs ns Heval. induction s as [|v0 t|v0 r|v0 m|v0 v1|v0 e0|v0 e0|v0|cond ss_true ss_false]; intros; simpl in Heval; try done.
+  move /andP : H => [Hv He]; move /eqP : Hv => Hv; move /eqP : He => He; subst v; subst e. destruct (Sem_HiFP.eval_hfexpr e0 init_s tmap); try discriminate.
+    inversion Heval; subst rs ns. rewrite PVM.Lemmas.find_add_eq //. apply PVM.M.SE.eq_refl.
+  destruct (Sem_HiFP.eval_hfexpr cond init_s tmap) as [valc|] eqn : Hcond; try discriminate. move : H => [Hunique_true [Hunique_false Hin]].
+  destruct (~~ is_zero valc). 
+  1,2 : move : Heval; apply (eval_hfstmts_for_unique_node_helper _ _ _ _ _ Hin); try done.
+Admitted.
+
+(* old bad version
+Lemma eval_hfstmts_for_unique_node_helper ss v e init_s tmap : 
+  Qin_with_cond (Snode v e) ss init_s tmap -> unique_node_dclr_when ss -> 
+  forall rs0 ns0, PVM.find v ns0 = None -> forall rs s,
+  Sem_HiFP.eval_hfstmts ss rs0 ns0 init_s tmap = Some (rs, s) ->
+  PVM.find v s = Sem_HiFP.eval_hfexpr e init_s tmap
+with eval_hfstmt_for_unique_node s v e init_s tmap : 
+  forall rs0 ns0, PVM.find v ns0 = None -> forall rs ns,
+  Sem_HiFP.eval_hfstmt s rs0 ns0 init_s tmap = Some (rs, ns) ->
+  match s with
+  | Swhen c ss1 ss2 => forall valc, Sem_HiFP.eval_hfexpr c init_s tmap = Some valc -> unique_node_dclr_when ss1 -> unique_node_dclr_when ss2 -> 
+    if (~~ is_zero valc) then Qin_with_cond (Snode v e) ss1 init_s tmap -> PVM.find v ns = Sem_HiFP.eval_hfexpr e init_s tmap
+    else Qin_with_cond (Snode v e) ss2 init_s tmap -> PVM.find v ns = Sem_HiFP.eval_hfexpr e init_s tmap
+  | _ => True
+  end.
+Proof.
+  clear eval_hfstmts_for_unique_node_helper. move : ss; elim. simpl; intros; done.
+  intros s ss IH Hin Hunique rs0 ns0 Hfind rs ns Hevals.
+  simpl in Hevals. destruct (Sem_HiFP.eval_hfstmt s rs0 ns0 init_s tmap) as [[rs1 ns1]|] eqn : Heval; try discriminate. simpl in Hin.
+  case Hst : s => [||var reg|||var node_e|var cnct_e|var|cond ss_true ss_false]; subst s.
+  + (* skip *) simpl in Heval; inversion Heval; subst rs0 ns0. move : Hevals; apply (IH Hin); try (move : Hunique; apply unique_node_dclr_when_subseq); try done.
+  + (* wire *) simpl in Heval; inversion Heval; subst rs0 ns0. move : Hevals; apply (IH Hin); try (move : Hunique; apply unique_node_dclr_when_subseq); try done.
+  + (* reg *) simpl in Heval. destruct (PVM.find var init_s); try discriminate.
+    inversion Heval; subst rs1 ns1. move : Hevals; apply (IH Hin); try (move : Hunique; apply unique_node_dclr_when_subseq); try done.
+  + (* mem *) simpl in Heval; inversion Heval; subst rs0 ns0. move : Hevals; apply (IH Hin); try (move : Hunique; apply unique_node_dclr_when_subseq); try done.
+  + (* inst *) simpl in Heval; inversion Heval; subst rs0 ns0. move : Hevals; apply (IH Hin); try (move : Hunique; apply unique_node_dclr_when_subseq); try done.
+  + (* node *) destruct (hfstmt_eqn (Snode var node_e) (Snode v e)) eqn : Hs. 
+    - (* s is node *) clear Hin IH eval_hfstmt_for_unique_node. simpl in Hs. 
+      move /andP : Hs => [Hvar Hnode_e]; move /eqP : Hvar => Hvar; move /eqP : Hnode_e => Hnode_e. subst var node_e.
+      unfold unique_node_dclr_when in Hunique. assert (Hin : Qin_when (Snode v e) (Qcons (Snode v e) ss)) by (simpl; rewrite eq_refl; rewrite eq_refl //).
+      apply Hunique in Hin; clear Hunique. move : Hin => [Hnode [Hcnct Hinvalid]]. 
+      simpl in Hcnct. simpl in Hinvalid. simpl in Hnode; rewrite eq_refl in Hnode; simpl in Hnode. rewrite eq_refl in Hnode; simpl in Hnode.
+      apply (eval_hfstmts_unique_when_ss_find_eq Hnode Hcnct Hinvalid) in Hevals.
+      rewrite Hevals. simpl in Heval. destruct (Sem_HiFP.eval_hfexpr e init_s tmap); try discriminate.
+      inversion Heval; subst rs1 ns1. apply PVM.Lemmas.find_add_eq; apply PVM.M.SE.eq_refl.
+    - (* s is in ss *) rewrite orb_false_l in Hin.
+      move : Hevals. apply (IH Hin); try (move : Hunique; apply unique_node_dclr_when_subseq). move : Hunique Hs Hin Heval Hfind; clear; intros.
+      unfold unique_node_dclr_when in Hunique. apply Qin_with_cond2Qin_when in Hin. assert (Qin_when (Snode v e) (Qcons (Snode var node_e) ss)) by (simpl; rewrite Hin orb_true_r //).
+      specialize (Hunique v e H).
+      move : Hunique => [Hunique _]. specialize (Hunique var node_e). simpl in Heval.
+      destruct (Sem_HiFP.eval_hfexpr node_e init_s tmap); try discriminate.
+      inversion Heval; subst rs1 ns1; rewrite PVM.Lemmas.find_add_neq //.
+      simpl in Hunique; simpl in Hs; rewrite Hs in Hunique. simpl in Hunique. 
+      rewrite eq_refl in Hunique; simpl in Hunique. rewrite eq_refl in Hunique; simpl in Hunique.
+      assert (true) by done. apply Hunique in H0.
+      unfold PVM.M.SE.eq. move : H0; apply contra_not. intro. move /eqP : H0 => H0; done.
+  + (* cnct *) simpl in Hin.
+      move : Hevals. apply (IH Hin); try (move : Hunique; apply unique_node_dclr_when_subseq). 
+      move : Hunique Hin Heval Hfind; clear; intros.
+      unfold unique_node_dclr_when in Hunique. apply Qin_with_cond2Qin_when in Hin. assert (Qin_when (Snode v e) (Qcons (Sfcnct var cnct_e) ss)) by (simpl; done).
+      specialize (Hunique v e H). simpl in Heval. destruct var as [ref|a|a|a] eqn : Href; try (inversion Heval; subst rs1 ns1; done).
+      destruct (PVM.find ref tmap) as [[gt cmpnt]|] eqn : Hgt; try discriminate.
+      move : Hunique => [_ [Hunique _]]. specialize (Hunique cnct_e). simpl in Hunique. rewrite eq_refl in Hunique; simpl in Hunique.
+      destruct cmpnt; destruct (Sem_HiFP.eval_hfexpr cnct_e init_s tmap); try discriminate; 
+      inversion Heval; subst rs1 ns1; try done. 1-7 : rewrite PVM.Lemmas.find_add_neq //.
+      1-7 : unfold PVM.M.SE.eq; move : Hunique; apply contra_not; intro; move /eqP : H0 => H0; subst v; rewrite eq_refl; simpl; done.
+  + (* invalid *) simpl in Hin.
+      move : Hevals. apply (IH Hin); try (move : Hunique; apply unique_node_dclr_when_subseq). 
+      move : Hunique Hin Heval Hfind; clear; intros.
+      unfold unique_node_dclr_when in Hunique. apply Qin_with_cond2Qin_when in Hin. assert (Qin_when (Snode v e) (Qcons (Sinvalid var) ss)) by (simpl; done).
+      specialize (Hunique v e H). simpl in Heval. destruct var as [ref|a|a|a] eqn : Href; try (inversion Heval; subst rs1 ns1; done).
+      destruct (PVM.find ref tmap) as [[gt cmpnt]|] eqn : Hgt; try discriminate.
+      move : Hunique => [_ [_ Hunique]]. specialize (Hunique ref). simpl in Hunique. rewrite eq_refl in Hunique; simpl in Hunique.
+      destruct cmpnt; destruct (sizeof_fgtyp gt < length indeterminate_val); 
+      try (inversion Heval; subst rs1 ns1; try done). 1-14 : rewrite PVM.Lemmas.find_add_neq //. 
+      1-14 : assert (true) by done; apply Hunique in H0.
+      1-14 : unfold PVM.M.SE.eq; move : H0; apply contra_not; intro; move /eqP : H0 => H0; subst v; done.
+  + (* when *) specialize (eval_hfstmt_for_unique_node _ _ e _ _ _ _ Hfind _ _ Heval); simpl in eval_hfstmt_for_unique_node.
+    simpl in Heval; destruct (Sem_HiFP.eval_hfexpr cond init_s tmap) as [valc|] eqn : Hc; try discriminate. specialize (eval_hfstmt_for_unique_node valc).
+    destruct (~~ is_zero valc). 
+    - (* go to true *)
+      destruct (Qin_with_cond (Snode v e) ss_true init_s tmap) eqn : Hin_true.
+      * (* node in true, not in ss *)
+        clear IH Hin. rewrite -eval_hfstmt_for_unique_node; try done.
+        unfold unique_node_dclr_when in Hunique. assert (Qin_when (Snode v e) (Qcons (Swhen cond ss_true ss_false) ss)). 
+        apply Qin_with_cond2Qin_when in Hin_true. simpl; rewrite Hin_true orb_true_l //. apply Hunique in H. move : H => [Hnode [Hcnct Hinvalid]].
+        move : Hevals; apply eval_hfstmts_unique_when_ss_find_eq.
+        move : Hnode Hin_true; clear; intros. apply (Hnode v' e'). simpl. apply Qin_with_cond2Qin_when in Hin_true. rewrite Hin_true. apply Qin_when_Qcons; done.
+        intros. move : (Hcnct e'); clear. apply contra_not. apply Qin_when_Qcons; done.
+        intros. apply (Hinvalid v'). move : H; apply Qin_when_Qcons; done.
+        1,2 : apply unique_node_dclr_when_branches in Hunique; move : Hunique => [Hunique1 Hunique2]; done.
+      * (* in ss *) rewrite orb_false_l in Hin. move : Hevals; apply (IH Hin).
+        move : Hunique; apply unique_node_dclr_when_subseq.
+        unfold unique_node_dclr_when in Hunique. assert (Qin_when (Snode v e) (Qcons (Swhen cond ss_true ss_false) ss)). 
+        apply Qin_with_cond2Qin_when in Hin. apply Qin_when_Qcons; done. apply Hunique in H. move : H => [Hnode [Hcnct Hinvalid]].
+        rewrite -Hfind. move : Heval; apply eval_hfstmts_unique_when_ss_find_eq.
+        move : Hnode Hin; clear; intros. intro; subst v'. apply Qin_with_cond2Qin_when in Hin. 
+        assert (Qin_when (Snode v e') ss_true \/ Qin_when (Snode v e') ss_false) by (left; done).
+        apply (Qin_when_uniqie_False Hnode Hin H0).
+        intros. move : (Hcnct e'); clear. apply contra_not. intro; simpl. rewrite H //.
+        intros. apply (Hinvalid v'). simpl. rewrite H //.
+    - (* go to false *)
+      destruct (Qin_with_cond (Snode v e) ss_false init_s tmap) eqn : Hin_false.
+      * (* node in false, not in ss *)
+        clear IH Hin. rewrite -eval_hfstmt_for_unique_node; try done.
+        unfold unique_node_dclr_when in Hunique. assert (Qin_when (Snode v e) (Qcons (Swhen cond ss_true ss_false) ss)). 
+        apply Qin_with_cond2Qin_when in Hin_false. simpl; rewrite Hin_false orb_true_r //. apply Hunique in H. move : H => [Hnode [Hcnct Hinvalid]].
+        move : Hevals; apply eval_hfstmts_unique_when_ss_find_eq.
+        move : Hnode Hin_false; clear; intros. apply (Hnode v' e'). simpl. apply Qin_with_cond2Qin_when in Hin_false. rewrite Hin_false. 
+        destruct (Qin_when (Snode v e) ss_true); apply Qin_when_Qcons; done.
+        intros. move : (Hcnct e'); clear. apply contra_not. apply Qin_when_Qcons; done.
+        intros. apply (Hinvalid v'). move : H; apply Qin_when_Qcons; done.
+        1,2 : apply unique_node_dclr_when_branches in Hunique; move : Hunique => [Hunique1 Hunique2]; done.
+      * (* in ss *) rewrite orb_false_l in Hin. move : Hevals; apply (IH Hin).
+        move : Hunique; apply unique_node_dclr_when_subseq.
+        unfold unique_node_dclr_when in Hunique. assert (Qin_when (Snode v e) (Qcons (Swhen cond ss_true ss_false) ss)). 
+        apply Qin_with_cond2Qin_when in Hin. apply Qin_when_Qcons; done. apply Hunique in H. move : H => [Hnode [Hcnct Hinvalid]].
+        rewrite -Hfind. move : Heval; apply eval_hfstmts_unique_when_ss_find_eq.
+        move : Hnode Hin; clear; intros. intro; subst v'. apply Qin_with_cond2Qin_when in Hin. 
+        assert (Qin_when (Snode v e') ss_true \/ Qin_when (Snode v e') ss_false) by (right; done).
+        apply (Qin_when_uniqie_False Hnode Hin H0).
+        intros. move : (Hcnct e'); clear. apply contra_not. intro; simpl. rewrite H orb_true_r //.
+        intros. apply (Hinvalid v'). simpl. rewrite H orb_true_r //.
+
+  clear eval_hfstmt_for_unique_node.
+  intros rs0 ns0 Hfind rs ns Heval. induction s as [|v0 t|v0 r|v0 m|v0 v1|v0 e0|v0 e0|v0|cond ss_true ss_false]; intros; try done.
+  simpl in Heval. rewrite H in Heval. destruct (~~ is_zero valc). 
+  1, 2 : intro; move : Heval; apply (eval_hfstmts_for_unique_node_helper _ _ _ _ _ H2); try done.
+Admitted.*)
+
+Lemma eval_hfstmts_for_unique_node ss v e init_s tmap : Qin_with_cond (Snode v e) ss init_s tmap -> unique_node_dclr_when ss -> 
+  forall rs s, Sem_HiFP.eval_hfstmts ss (PVM.empty bits) (PVM.empty bits) init_s tmap = Some (rs, s) ->
+  PVM.find v s = Sem_HiFP.eval_hfexpr e init_s tmap.
+Proof.
+  intro. intro. apply eval_hfstmts_for_unique_node_helper; try done.
+Qed.
 
 Lemma eval_hfstmt_find_eq2find_eq temp_rs temp_s temp_rs' temp_s' init_s tmap rs' s' rs s stmt v : 
   Sem_HiFP.eval_hfstmt stmt temp_rs temp_s init_s tmap = Some (rs, s) ->
@@ -1961,9 +2427,13 @@ Qed.
 Lemma eval_hfstmts_for_comb_only_cnct init_s tmap v component_stmts connect_stmts:
   (forall s, Qin s component_stmts -> is_declaration s) ->
   match PVM.find v tmap with
-  | Some (gt, Out_port) => (forall v' e', Qin (Snode v' e') component_stmts -> v <> v') -> forall rs s, Sem_HiFP.eval_hfstmts (Qcat component_stmts connect_stmts) (PVM.empty bits) (PVM.empty bits) init_s tmap = Some (rs, s) ->
+  | Some (gt, Out_port) => (forall v' e', Qin (Snode v' e') component_stmts -> v <> v') -> 
+      (forall c ss1 ss2, ~ Qin (Swhen c ss1 ss2) (Qcat component_stmts connect_stmts)) ->
+      forall rs s, Sem_HiFP.eval_hfstmts (Qcat component_stmts connect_stmts) (PVM.empty bits) (PVM.empty bits) init_s tmap = Some (rs, s) ->
       forall rs' s', Sem_HiFP.eval_hfstmts connect_stmts (PVM.empty bits) (PVM.empty bits) init_s tmap = Some (rs', s') -> PVM.find v s' = PVM.find v s
-  | Some (gt, Wire) => (forall v' e', Qin (Snode v' e') component_stmts -> v <> v') -> forall rs s, Sem_HiFP.eval_hfstmts (Qcat component_stmts connect_stmts) (PVM.empty bits) (PVM.empty bits) init_s tmap = Some (rs, s) ->
+  | Some (gt, Wire) => (forall v' e', Qin (Snode v' e') component_stmts -> v <> v') -> 
+      (forall c ss1 ss2, ~ Qin (Swhen c ss1 ss2) (Qcat component_stmts connect_stmts)) ->
+      forall rs s, Sem_HiFP.eval_hfstmts (Qcat component_stmts connect_stmts) (PVM.empty bits) (PVM.empty bits) init_s tmap = Some (rs, s) ->
       forall rs' s', Sem_HiFP.eval_hfstmts connect_stmts (PVM.empty bits) (PVM.empty bits) init_s tmap = Some (rs', s') -> PVM.find v s' = PVM.find v s
   | _ => True
   end.
@@ -1972,6 +2442,7 @@ Proof.
   (* outport *) 
   assert (Hhelper : forall temp_rs temp_s rs s : PVM.t bits,
     (forall v' e', Qin (Snode v' e') component_stmts -> v <> v') ->
+    (forall c ss1 ss2, ~ Qin (Swhen c ss1 ss2) (Qcat component_stmts connect_stmts)) ->
     Sem_HiFP.eval_hfstmts (Qcat component_stmts connect_stmts)
     temp_rs temp_s init_s tmap = 
     Some (rs, s) ->
@@ -1980,17 +2451,19 @@ Proof.
     Sem_HiFP.eval_hfstmts connect_stmts temp_rs' temp_s' init_s tmap = Some (rs', s') ->
     PVM.find v s' = PVM.find v s). {
     move : component_stmts Hdclr. elim.
-    intros Hdclr temp_rs temp_s rs s Hneq Heval temp_rs' temp_s' rs' s' Htemp Heval'. simpl in Heval. apply (eval_hfstmts_find_eq2find_eq v Heval) in Heval'.
+    intros Hdclr temp_rs temp_s rs s Hneq Hwhen Heval temp_rs' temp_s' rs' s' Htemp Heval'. simpl in Heval. apply (eval_hfstmts_find_eq2find_eq v Heval) in Heval'.
       move : Heval' => [_ Heval']. apply Heval'; done.
-    intros st ss IH Hdclr temp_rs temp_s rs s Hneq Heval temp_rs' temp_s' rs' s' Htemp Heval'. simpl in Heval.
+    intros st ss IH Hdclr temp_rs temp_s rs s Hneq Hwhen Heval temp_rs' temp_s' rs' s' Htemp Heval'. simpl in Heval.
     case Hst : st => [||var reg|||var node_e|ref e|ref|cond ss_true ss_false]; subst st; simpl in Heval.
     1,2,4,5 : move : Heval temp_rs' temp_s' rs' s' Htemp Heval'; apply IH. 
-    1,3,5,7 : intros; apply Hdclr; simpl; rewrite H orb_true_r //.
-    1-4 : intros; apply (Hneq v' e'); simpl; done.
+    1,4,7,10 : intros; apply Hdclr; simpl; rewrite H orb_true_r //.
+    1,3,5,7 : intros; apply (Hneq v' e'); simpl; done.
+    1-4 : intros; specialize (Hwhen c ss1 ss2); move : Hwhen; apply contra_not; intro; try done.
     (* reg *)
     destruct (PVM.find var init_s); try discriminate.
     move : Heval temp_rs' temp_s' rs' s' Htemp Heval'; apply IH. intros; apply Hdclr; simpl; rewrite H orb_true_r //.
     intros; apply (Hneq v' e'); simpl; done.
+    intros; specialize (Hwhen c ss1 ss2); move : Hwhen; apply contra_not; intro; try done.
     (* node *)
     destruct (Sem_HiFP.eval_hfexpr node_e init_s tmap); try discriminate.
     move : Heval'; apply IH with (temp_rs := temp_rs) (temp_s := PVM.add var b temp_s) (rs := rs); try done. intros; apply Hdclr; simpl; rewrite H orb_true_r //.
@@ -2002,12 +2475,17 @@ Proof.
     (* invalid *)
     assert (Qin (Sinvalid ref) (Qcons (Sinvalid ref) ss)). simpl. rewrite eq_refl //. apply Hdclr in H. simpl in H. done.
     (* when *)
-    admit.
+    specialize (Hwhen cond ss_true ss_false). simpl in Hwhen. rewrite eq_refl in Hwhen; simpl in Hwhen. 
+    specialize (hfstmt_seq_eqn_refl ss_true) as Heq. move/eqP : Heq => Heq. specialize (hfstmt_seq_eqP ss_true ss_true) as Heq'. apply reflect_iff in Heq'.
+    apply Heq' in Heq. rewrite Heq in Hwhen; simpl in Hwhen. clear Heq Heq'.
+    specialize (hfstmt_seq_eqn_refl ss_false) as Heq. move/eqP : Heq => Heq. specialize (hfstmt_seq_eqP ss_false ss_false) as Heq'. apply reflect_iff in Heq'.
+    apply Heq' in Heq. rewrite Heq in Hwhen; simpl in Hwhen. done.
     }
-  intros. move : H1. apply (Hhelper _ _ _ _ H H0). done.
+  intros. move : H2. apply (Hhelper _ _ _ _ H H0 H1). done.
   (* wire *)
   assert (Hhelper : forall temp_rs temp_s rs s : PVM.t bits,
     (forall v' e', Qin (Snode v' e') component_stmts -> v <> v') ->
+    (forall c ss1 ss2, ~ Qin (Swhen c ss1 ss2) (Qcat component_stmts connect_stmts)) ->
     Sem_HiFP.eval_hfstmts (Qcat component_stmts connect_stmts)
     temp_rs temp_s init_s tmap = 
     Some (rs, s) ->
@@ -2016,17 +2494,19 @@ Proof.
     Sem_HiFP.eval_hfstmts connect_stmts temp_rs' temp_s' init_s tmap = Some (rs', s') ->
     PVM.find v s' = PVM.find v s). {
     move : component_stmts Hdclr. elim.
-    intros Hdclr temp_rs temp_s rs s Hneq Heval temp_rs' temp_s' rs' s' Htemp Heval'. simpl in Heval. apply (eval_hfstmts_find_eq2find_eq v Heval) in Heval'.
+    intros Hdclr temp_rs temp_s rs s Hneq Hwhen Heval temp_rs' temp_s' rs' s' Htemp Heval'. simpl in Heval. apply (eval_hfstmts_find_eq2find_eq v Heval) in Heval'.
       move : Heval' => [_ Heval']. apply Heval'; done.
-    intros st ss IH Hdclr temp_rs temp_s rs s Hneq Heval temp_rs' temp_s' rs' s' Htemp Heval'. simpl in Heval.
+    intros st ss IH Hdclr temp_rs temp_s rs s Hneq Hwhen Heval temp_rs' temp_s' rs' s' Htemp Heval'. simpl in Heval.
     case Hst : st => [||var reg|||var node_e|ref e|ref|cond ss_true ss_false]; subst st; simpl in Heval.
     1,2,4,5 : move : Heval temp_rs' temp_s' rs' s' Htemp Heval'; apply IH. 
-    1,3,5,7 : intros; apply Hdclr; simpl; rewrite H orb_true_r //.
-    1-4 : intros; apply (Hneq v' e'); simpl; done.
+    1,4,7,10 : intros; apply Hdclr; simpl; rewrite H orb_true_r //.
+    1,3,5,7 : intros; apply (Hneq v' e'); simpl; done.
+    1-4 : intros; specialize (Hwhen c ss1 ss2); move : Hwhen; apply contra_not; intro; try done.
     (* reg *)
     destruct (PVM.find var init_s); try discriminate.
     move : Heval temp_rs' temp_s' rs' s' Htemp Heval'; apply IH. intros; apply Hdclr; simpl; rewrite H orb_true_r //.
     intros; apply (Hneq v' e'); simpl; done.
+    intros; specialize (Hwhen c ss1 ss2); move : Hwhen; apply contra_not; intro; try done.
     (* node *)
     destruct (Sem_HiFP.eval_hfexpr node_e init_s tmap); try discriminate.
     move : Heval'; apply IH with (temp_rs := temp_rs) (temp_s := PVM.add var b temp_s) (rs := rs); try done. intros; apply Hdclr; simpl; rewrite H orb_true_r //.
@@ -2038,15 +2518,14 @@ Proof.
     (* invalid *)
     assert (Qin (Sinvalid ref) (Qcons (Sinvalid ref) ss)). simpl. rewrite eq_refl //. apply Hdclr in H. simpl in H. done.
     (* when *)
-    admit.
+    specialize (Hwhen cond ss_true ss_false). simpl in Hwhen. rewrite eq_refl in Hwhen; simpl in Hwhen. 
+    specialize (hfstmt_seq_eqn_refl ss_true) as Heq. move/eqP : Heq => Heq. specialize (hfstmt_seq_eqP ss_true ss_true) as Heq'. apply reflect_iff in Heq'.
+    apply Heq' in Heq. rewrite Heq in Hwhen; simpl in Hwhen. clear Heq Heq'.
+    specialize (hfstmt_seq_eqn_refl ss_false) as Heq. move/eqP : Heq => Heq. specialize (hfstmt_seq_eqP ss_false ss_false) as Heq'. apply reflect_iff in Heq'.
+    apply Heq' in Heq. rewrite Heq in Hwhen; simpl in Hwhen. done.
     }
-  intros. move : H1. apply (Hhelper _ _ _ _ H H0). done.
-Admitted.
-
-(*Lemma eval_hfstmts_Qcat_some s1 s2 rs ns s tmap res : Sem_HiFP.eval_hfstmts (Qcat s1 s2) rs ns s tmap = Some res ->
-  exists res', Sem_HiFP.eval_hfstmts s1 rs ns s tmap = Some res'.
-Proof.
-Admitted.*)
+  intros. move : H2. apply (Hhelper _ _ _ _ H H0 H1). done.
+Qed.
 
 Lemma eval_hfstmts_Qcat_exists s0 rs0 init_s tmap rs s l1 l2 : Sem_HiFP.eval_hfstmts (Qcat l1 l2) rs0 s0 init_s tmap = Some (rs, s)
   -> exists temp_s temp_rs, Sem_HiFP.eval_hfstmts l1 rs0 s0 init_s tmap = Some (temp_rs, temp_s) /\  Sem_HiFP.eval_hfstmts l2 temp_rs temp_s init_s tmap = Some (rs, s).
@@ -2307,8 +2786,7 @@ Lemma unique_connect_stmts_convert_to_connect_stmt ss (v : ProdVarOrder.t) d_exp
 Proof.
   intros [Hnot_invalid Hnot_cnct] Hss; unfold unique_connect_stmts in *. move : Hss => [Hcnct Hinvalid]. split.
   - (* cnct in *)
-    intros v0 e0 Hin. destruct d_expr as [|gt|de]; simpl in *. 
-    * apply Hcnct; done.
+    intros v0 e0 Hin. destruct d_expr as [gt|de]; simpl in *. 
     * specialize (Hnot_cnct e0). destruct (Eid v == v0) eqn : Hneq. move /eqP : Hneq => Hneq; subst v0; done.
       apply Hcnct in Hin as Hcnct'; clear Hcnct. move : Hcnct' => [Hcnct' Hinvalid']; split; try done.
     * destruct (Eid v == v0) eqn : Hneq. move /eqP : Hneq => Hneq; subst v0. simpl in *. destruct (de == e0) eqn : Heqe.
@@ -2319,8 +2797,7 @@ Proof.
       + (* neqv *)
         simpl in *. rewrite Hneq. simpl. apply Hcnct; done.
   - (* invalid in *) 
-    intros v0 Hin. destruct d_expr as [|gt|de]; simpl in *. 
-    * apply Hinvalid; done.
+    intros v0 Hin. destruct d_expr as [gt|de]; simpl in *. 
     * destruct (Eid v == v0) eqn : Hneq. move /eqP : Hneq => Hneq; subst v0; done.
       rewrite orb_false_l in Hin. simpl. rewrite Hneq; simpl.
       apply Hinvalid in Hin as Hinvalid'; clear Hinvalid. move : Hinvalid' => [Hcnct' Hinvalid']; split; try done.
@@ -2453,21 +2930,21 @@ Proof.
     (* invalid *)
     assert (Qin (Sinvalid ref) (Qcons (Sinvalid ref) ss)). simpl. rewrite eq_refl; simpl; done. apply Hdclr in H. simpl in H. done.
     (* when *)
-    admit.
+    assert (Qin (Swhen cond ss_true ss_false) (Qcons (Swhen cond ss_true ss_false) ss)). simpl. rewrite eq_refl; simpl.
+    specialize (hfstmt_seq_eqn_refl ss_true) as Heq. move/eqP : Heq => Heq. specialize (hfstmt_seq_eqP ss_true ss_true) as Heq'. apply reflect_iff in Heq'.
+    apply Heq' in Heq. rewrite Heq; simpl. clear Heq Heq'.
+    specialize (hfstmt_seq_eqn_refl ss_false) as Heq. move/eqP : Heq => Heq. specialize (hfstmt_seq_eqP ss_false ss_false) as Heq'. apply reflect_iff in Heq'.
+    apply Heq' in Heq. rewrite Heq //.
+    apply Hdclr in H. simpl in H. done.
     }
   intros H Hr_cnct rs s H0 rs' s' H1. move : H1; apply (Hhelper _ _ Hdclr) with (temp_rs := PVM.empty bits) (temp_s := PVM.empty bits) (s := s); try done.
   apply convert_to_connect_stmts_is_connection. 
   apply convert_to_connect_stmts_unique_connect_stmts.
-Admitted.
-
-Lemma func_type_eq_eval_hfstmts ss conn_map tmap : ExpandBranches_funs ss (PVM.empty def_expr) tmap = Some conn_map ->
-func_type_eq (Sem_HiFP.eval_hfstmts ss) (Sem_HiFP.eval_hfstmts (Qcat (component_stmts_of ss) (convert_to_connect_stmts conn_map))) tmap.
-Proof.
-Admitted.
+Qed.
 
 Lemma eval_hfstmts_Qcat_some' s1 s2 rs0 ns0 rs1 ns1 s tmap res : Sem_HiFP.eval_hfstmts (Qcat s1 s2) rs0 ns0 s tmap = Some res ->
   exists res', Sem_HiFP.eval_hfstmts s2 rs1 ns1 s tmap = Some res'.
-  Proof.
+Proof.
   move : s1 rs0 ns0 rs1 ns1. elim; simpl; intros.
   - (* s1 = Qnil *) destruct res as [rs ns].
     apply eval_hfstmts_exists with (rs1 := rs1) (ns1 := ns1) in H. destruct H as [rs' [ns' H]].
@@ -2523,7 +3000,7 @@ Proof.
   (* comb *) intro Hnone.
   assert (Hnone_hd : PVM.find v ns' = None). {
     move : Hneq Hss Hnone Heval_hd; clear.
-    destruct de_hd; simpl in *; intros. rewrite Hss in Heval_hd. inversion Heval_hd; subst ns'; done.
+    destruct de_hd; simpl in *; intros.
     - (* invalid *)
     destruct (PVM.find v_hd tmap) as [[gt cmpnt]|]; try discriminate. rewrite -Hnone.
     destruct cmpnt; destruct (sizeof_fgtyp gt < length indeterminate_val). 
@@ -2540,7 +3017,7 @@ Proof.
   (* sequ *) intro Hnone.
   assert (Hnone_hd : PVM.find v rs' = None). {
     move : Hneq Hss Hnone Heval_hd; clear.
-    destruct de_hd; simpl in *; intros. rewrite Hss in Heval_hd. inversion Heval_hd; subst rs'; done.
+    destruct de_hd; simpl in *; intros. 
     - (* invalid *)
     destruct (PVM.find v_hd tmap) as [[gt cmpnt]|]; try discriminate. rewrite -Hnone.
     destruct cmpnt; destruct (sizeof_fgtyp gt < length indeterminate_val). 
@@ -2559,7 +3036,8 @@ Qed.
 Lemma eval_hfstmts_notinss_findeq tmap init_s ss temp_rs temp_s rs s v : (forall st, Qin st ss ->
   match st with 
   | Snode _ _ 
-  | Sreg _ _ => False
+  | Sreg _ _ 
+  | Swhen _ _ _ => False
   | Sfcnct v0 _ 
   | Sinvalid v0 => v0 <> Eid v
   | _ => True
@@ -2569,7 +3047,8 @@ Lemma eval_hfstmts_notinss_findeq tmap init_s ss temp_rs temp_s rs s v : (forall
 with eval_hfstmt_notinss_findeq tmap init_s st temp_rs temp_s rs s v : 
   match st with 
   | Snode _ _ 
-  | Sreg _ _ => False
+  | Sreg _ _ 
+  | Swhen _ _ _ => False
   | Sfcnct v0 _ 
   | Sinvalid v0 => v0 <> Eid v
   | _ => True
@@ -2583,14 +3062,16 @@ Proof.
     Qin st tl ->
     match st with
     | Snode _ _ 
-    | Sreg _ _ => False
+    | Sreg _ _ 
+    | Swhen _ _ _ => False
     | Sfcnct v0 _ | Sinvalid v0 => v0 <> Eid v
     | _ => True
     end). intros; apply Hnotin. rewrite H orb_true_r //.
   apply (IH _ _ _ _ H) in Hevals as [Hevals0 Hevals1]. rewrite Hevals0 Hevals1. clear H. 
   assert (match hd with
   | Snode _ _
-  | Sreg _ _ => False
+  | Sreg _ _ 
+  | Swhen _ _ _ => False
   | Sfcnct v0 _ | Sinvalid v0 => v0 <> Eid v
   | _ => True
   end). apply Hnotin. specialize (hfstmt_eqn_refl hd) as Heq. move/eqP : Heq => Heq. 
@@ -2605,14 +3086,51 @@ Proof.
   (* invalid *) destruct v0; try (inversion Heval; subst s rs; done). destruct (PVM.find s0 tmap) as [[gt cmpnt]|]; try discriminate.
   destruct cmpnt; destruct (sizeof_fgtyp gt < length indeterminate_val); try (inversion Heval; subst s rs; split); try done.
   1-16 : rewrite PVM.Lemmas.find_add_neq //. 1-16 : unfold PVM.M.SE.eq; intro; move /eqP : H => H; subst v; done.
-  (* when *) destruct (Sem_HiFP.eval_hfexpr c init_s tmap); try discriminate. destruct (~~ is_zero b).
-  1,2 : move : Heval; apply eval_hfstmts_notinss_findeq. (* TBD *)
-Admitted.
+Qed.
 
 Lemma convert_to_connect_stmt_qcat k d l tl : convert_to_connect_stmt k d (Qcat l tl) =
   Qcat (convert_to_connect_stmt k d l) tl.
 Proof. 
   destruct d; simpl; done.
+Qed.
+
+Lemma eval_hfstmts_convert_to_connect_stmts_for_comb_helper v l1: 
+  (~ In v (fst (List.split l1))) -> forall ss, (forall st : hfstmt ProdVarOrder.T,
+      Qin st ss ->
+      match st with
+      | Snode _ _ 
+      | Sreg _ _ 
+      | Swhen _ _ _ => False
+      | Sfcnct v0 _ | Sinvalid v0 => v0 <> Eid v
+      | _ => True
+      end) ->
+      forall st : hfstmt ProdVarOrder.T,
+        Qin st
+          (fold_left
+            (fun (a : HiFP.hfstmt_seq) (p : PVM.key * def_expr) =>
+              convert_to_connect_stmt (fst p) (snd p) a) l1 
+            ss) ->
+        match st with
+        | Snode _ _ 
+        | Sreg _ _ 
+        | Swhen _ _ _ => False
+        | Sfcnct v0 _ | Sinvalid v0 => v0 <> Eid v
+        | _ => True
+        end.
+Proof.
+  move : l1. elim; simpl. intros _ ss Hss st Hin. apply Hss; done.
+  intros [hd_key hd_de] tl IH Hnotin ss Hss st. apply IH. move : Hnotin; apply contra_not; clear; intro.
+    destruct (List.split tl) as [left right]; simpl in *. right; done.
+  simpl; clear IH. rewrite -(qcat0s ss).
+  rewrite convert_to_connect_stmt_qcat. destruct hd_de; simpl; try done.
+  (* invalid *)
+  intros. destruct (Qin st0 ss) eqn : Hin. apply Hss; done. clear Hin. rewrite orb_false_r in H.
+  destruct st0; try done. move : Hnotin; apply contra_not; intro. subst h. move /eqP : H => H; inversion H; subst v.
+  destruct (List.split tl); simpl. left; done.
+  (* cnct *)
+  intros. destruct (Qin st0 ss) eqn : Hin. apply Hss; done. clear Hin. rewrite orb_false_r in H.
+  destruct st0; try done. move : Hnotin; apply contra_not; intro. subst h0. move /andP : H => [H _]. 
+  move /eqP : H => H; inversion H; subst v. destruct (List.split tl); simpl. left; done.
 Qed.
 
 Lemma eval_hfstmts_convert_to_connect_stmts_for_comb conn_map init_s tmap rs s v : 
@@ -2621,9 +3139,9 @@ Lemma eval_hfstmts_convert_to_connect_stmts_for_comb conn_map init_s tmap rs s v
   | Some (gt, Wire) => Sem_HiFP.eval_hfstmts (convert_to_connect_stmts conn_map) (PVM.empty bits) (PVM.empty bits) init_s tmap = Some (rs, s) -> 
       match PVM.find v conn_map with
       | Some (D_fexpr e) => Sem_HiFP.eval_hfexpr e init_s tmap = PVM.find v s
-      | Some (D_invalidated gt_e) => 
-          if (length indeterminate_val > sizeof_fgtyp gt_e) then Some (take (sizeof_fgtyp gt_e) indeterminate_val) = PVM.find v s
-          else Some (zext ((sizeof_fgtyp gt_e) - (length indeterminate_val)) indeterminate_val) = PVM.find v s
+      | Some (D_invalidated _) => 
+          if (length indeterminate_val > sizeof_fgtyp gt) then Some (take (sizeof_fgtyp gt) indeterminate_val) = PVM.find v s
+          else Some (zext ((sizeof_fgtyp gt) - (length indeterminate_val)) indeterminate_val) = PVM.find v s
       | _ => True
       end
   | _ => True
@@ -2631,8 +3149,69 @@ Lemma eval_hfstmts_convert_to_connect_stmts_for_comb conn_map init_s tmap rs s v
 Proof. 
   case Hcmpnt : (PVM.find v tmap) => [[gt cmpnt]|]; try done. destruct cmpnt; try done.
   - (* outport *)
-    intros Heval. destruct (PVM.find v conn_map) as [de|] eqn : Hcm; try done. destruct de as [|gt_e|e]; try done.
-    + (* invalid *) admit.
+    intros Heval. destruct (PVM.find v conn_map) as [de|] eqn : Hcm; try done. destruct de as [gt_e|e].
+    + (* invalid *) 
+    remember (convert_to_connect_stmts conn_map) as cmlist.
+    rewrite /convert_to_connect_stmts PVM.fold_1 in Heqcmlist. 
+    apply CEP.Lemmas.find_some_mapsto in Hcm. apply CEP.Lemmas.F.elements_mapsto_iff in Hcm.
+    remember (PVM.elements conn_map) as elements. apply InA_alt in Hcm. destruct Hcm as [[v' e'] [Heq Hin]].
+    destruct Heq as [Heq0 Heq1]. simpl in Heq0; simpl in Heq1. move /eqP : Heq0 => Heq0; subst v' e'.
+    destruct (in_split _ _ Hin) as [l1 [l2 Helements]]. subst elements.
+    rewrite Helements in Heqcmlist. rewrite fold_left_app in Heqcmlist. simpl in Heqcmlist.
+    remember (fold_left (fun (a : HiFP.hfstmt_seq) (p : PVM.key * def_expr) => convert_to_connect_stmt (fst p) (snd p) a) l1 (Qnil _)) as ss_prefix.
+    remember (fold_left (fun (a : HiFP.hfstmt_seq) (p : PVM.key * def_expr) => convert_to_connect_stmt (fst p) (snd p) a) l2 (Qcons (Sinvalid (Eid v)) ss_prefix)) as ss_suffix.
+    subst cmlist.
+    assert (Heqss_suffix' : ss_suffix = Qcat (fold_left
+                 (fun (a : HiFP.hfstmt_seq) (p : PVM.key * def_expr) =>
+                  convert_to_connect_stmt (fst p) (snd p) a) l2 (Qnil ProdVarOrder.T)) (Qcons (Sinvalid (Eid v)) ss_prefix)). {
+      move : Heqss_suffix; clear; intro. remember (Qcons (Sinvalid (Eid v)) ss_prefix) as res. clear Heqres. subst ss_suffix; clear.
+      rewrite -fold_left_qcat. simpl. done. }
+    clear Heqss_suffix.
+    rewrite Heqss_suffix' in Heval. apply eval_hfstmts_Qcat_exists in Heval. destruct Heval as [temp_s [temp_rs [Heval2 Heval1]]].
+    assert (Htemp : PVM.find v temp_s = None). { 
+      assert (Hnodup : ~ In v (fst (List.split l2))). {
+        specialize (PVM.elements_3w conn_map) as Hnodup. rewrite Helements in Hnodup. move : Hnodup; clear; intro.
+        specialize (NoDupA_notin Hnodup) as [_ Hnotin]; done. }
+      clear Heval1. assert (Sem_HiFP.eval_hfstmts (Qnil ProdVarOrder.T) (PVM.empty bits) (PVM.empty bits) init_s tmap = Some (PVM.empty bits, PVM.empty bits)) by (simpl; done).
+      specialize (eval_hfstmts_notin_none H Hnodup Heval2) as [Hhelper _]. apply Hhelper; done.
+    }
+    clear Heval2 Heqss_suffix'. simpl in Heval1. rewrite Hcmpnt in Heval1. destruct (sizeof_fgtyp gt < length indeterminate_val).
+    (* take *)
+    remember (take (sizeof_fgtyp gt) indeterminate_val) as val; clear Heqval.
+    assert (Hprefix : PVM.find v s = PVM.find v (PVM.add v val temp_s)).
+      assert (Hnotin : ~ In v (fst (List.split l1))). 
+      { specialize (PVM.elements_3w conn_map) as Hnodup. rewrite Helements in Hnodup. move : Hnodup; clear; intro. specialize (NoDupA_notin Hnodup) as [Hnotin _]; done. }
+      assert (Hhypo : forall st, Qin st ss_prefix ->
+      match st with 
+      | Snode _ _ 
+      | Sreg _ _
+      | Swhen _ _ _ => False
+      | Sfcnct v0 _ 
+      | Sinvalid v0 => v0 <> Eid v
+      | _ => True
+      end).
+      rewrite Heqss_prefix; move : Hnotin Hin; clear.
+    intros Hnotin Hin. apply eval_hfstmts_convert_to_connect_stmts_for_comb_helper; intros; try done.
+    specialize (eval_hfstmts_notinss_findeq Hhypo Heval1) as [Hhelper _]; done.
+    rewrite Hprefix HiFP.PCELemmas.find_add_eq //. apply CEP.SE.eq_refl.
+    (* ext *)
+    remember (zext (sizeof_fgtyp gt - length indeterminate_val) indeterminate_val) as val; clear Heqval.
+    assert (Hprefix : PVM.find v s = PVM.find v (PVM.add v val temp_s)).
+      assert (Hnotin : ~ In v (fst (List.split l1))). 
+      { specialize (PVM.elements_3w conn_map) as Hnodup. rewrite Helements in Hnodup. move : Hnodup; clear; intro. specialize (NoDupA_notin Hnodup) as [Hnotin _]; done. }
+      assert (Hhypo : forall st, Qin st ss_prefix ->
+      match st with 
+      | Snode _ _ 
+      | Sreg _ _
+      | Swhen _ _ _ => False
+      | Sfcnct v0 _ 
+      | Sinvalid v0 => v0 <> Eid v
+      | _ => True
+      end).
+      rewrite Heqss_prefix; move : Hnotin Hin; clear.
+    intros Hnotin Hin. apply eval_hfstmts_convert_to_connect_stmts_for_comb_helper; intros; try done.
+    specialize (eval_hfstmts_notinss_findeq Hhypo Heval1) as [Hhelper _]; done.
+    rewrite Hprefix HiFP.PCELemmas.find_add_eq //. apply CEP.SE.eq_refl.
     + (* cnct *)
     remember (convert_to_connect_stmts conn_map) as cmlist.
     rewrite /convert_to_connect_stmts PVM.fold_1 in Heqcmlist. 
@@ -2665,65 +3244,200 @@ Proof.
       assert (Hhypo : forall st, Qin st ss_prefix ->
       match st with 
       | Snode _ _ 
-      | Sreg _ _ => False
+      | Sreg _ _
+      | Swhen _ _ _ => False
       | Sfcnct v0 _ 
       | Sinvalid v0 => v0 <> Eid v
       | _ => True
       end).
       rewrite Heqss_prefix; move : Hnotin Hin; clear.
-      assert ((~ In v (fst (List.split l1))) -> forall ss, (forall st : hfstmt ProdVarOrder.T,
-      Qin st ss ->
-      match st with
-      | Snode _ _ 
-      | Sreg _ _ => False
-      | Sfcnct v0 _ | Sinvalid v0 => v0 <> Eid v
-      | _ => True
-      end) ->
-      forall st : hfstmt ProdVarOrder.T,
-        Qin st
-          (fold_left
-            (fun (a : HiFP.hfstmt_seq) (p : PVM.key * def_expr) =>
-              convert_to_connect_stmt (fst p) (snd p) a) l1 
-            ss) ->
-        match st with
-        | Snode _ _ 
-        | Sreg _ _ => False
-        | Sfcnct v0 _ | Sinvalid v0 => v0 <> Eid v
-        | _ => True
-        end). { move : l1. elim; simpl. intros _ ss Hss st Hin. apply Hss; done.
-      intros [hd_key hd_de] tl IH Hnotin ss Hss st. apply IH. move : Hnotin; apply contra_not; clear; intro.
-        destruct (List.split tl) as [left right]; simpl in *. right; done.
-      simpl; clear IH. rewrite -(qcat0s ss).
-      rewrite convert_to_connect_stmt_qcat. destruct hd_de; simpl; try done.
-      (* invalid *)
-      intros. destruct (Qin st0 ss) eqn : Hin. apply Hss; done. clear Hin. rewrite orb_false_r in H.
-      destruct st0; try done. move : Hnotin; apply contra_not; intro. subst h. move /eqP : H => H; inversion H; subst v.
-      destruct (List.split tl); simpl. left; done.
-      (* cnct *)
-      intros. destruct (Qin st0 ss) eqn : Hin. apply Hss; done. clear Hin. rewrite orb_false_r in H.
-      destruct st0; try done. move : Hnotin; apply contra_not; intro. subst h0. move /andP : H => [H _]. 
-      move /eqP : H => H; inversion H; subst v. destruct (List.split tl); simpl. left; done. }
-    intros Hnotin Hin. apply H; intros; try done. 
+    intros Hnotin Hin. apply eval_hfstmts_convert_to_connect_stmts_for_comb_helper; intros; try done.
     specialize (eval_hfstmts_notinss_findeq Hhypo Heval1) as [Hhelper _]; done.
-    rewrite Hprefix HiFP.PCELemmas.find_add_eq //. apply CEP.SE.eq_refl. 
+    rewrite Hprefix HiFP.PCELemmas.find_add_eq //. apply CEP.SE.eq_refl.
   - (* wire 同上 *)
-Admitted. 
+    intros Heval. destruct (PVM.find v conn_map) as [de|] eqn : Hcm; try done. destruct de as [gt_e|e].
+    + (* invalid *) 
+    remember (convert_to_connect_stmts conn_map) as cmlist.
+    rewrite /convert_to_connect_stmts PVM.fold_1 in Heqcmlist. 
+    apply CEP.Lemmas.find_some_mapsto in Hcm. apply CEP.Lemmas.F.elements_mapsto_iff in Hcm.
+    remember (PVM.elements conn_map) as elements. apply InA_alt in Hcm. destruct Hcm as [[v' e'] [Heq Hin]].
+    destruct Heq as [Heq0 Heq1]. simpl in Heq0; simpl in Heq1. move /eqP : Heq0 => Heq0; subst v' e'.
+    destruct (in_split _ _ Hin) as [l1 [l2 Helements]]. subst elements.
+    rewrite Helements in Heqcmlist. rewrite fold_left_app in Heqcmlist. simpl in Heqcmlist.
+    remember (fold_left (fun (a : HiFP.hfstmt_seq) (p : PVM.key * def_expr) => convert_to_connect_stmt (fst p) (snd p) a) l1 (Qnil _)) as ss_prefix.
+    remember (fold_left (fun (a : HiFP.hfstmt_seq) (p : PVM.key * def_expr) => convert_to_connect_stmt (fst p) (snd p) a) l2 (Qcons (Sinvalid (Eid v)) ss_prefix)) as ss_suffix.
+    subst cmlist.
+    assert (Heqss_suffix' : ss_suffix = Qcat (fold_left
+                 (fun (a : HiFP.hfstmt_seq) (p : PVM.key * def_expr) =>
+                  convert_to_connect_stmt (fst p) (snd p) a) l2 (Qnil ProdVarOrder.T)) (Qcons (Sinvalid (Eid v)) ss_prefix)). {
+      move : Heqss_suffix; clear; intro. remember (Qcons (Sinvalid (Eid v)) ss_prefix) as res. clear Heqres. subst ss_suffix; clear.
+      rewrite -fold_left_qcat. simpl. done. }
+    clear Heqss_suffix.
+    rewrite Heqss_suffix' in Heval. apply eval_hfstmts_Qcat_exists in Heval. destruct Heval as [temp_s [temp_rs [Heval2 Heval1]]].
+    assert (Htemp : PVM.find v temp_s = None). { 
+      assert (Hnodup : ~ In v (fst (List.split l2))). {
+        specialize (PVM.elements_3w conn_map) as Hnodup. rewrite Helements in Hnodup. move : Hnodup; clear; intro.
+        specialize (NoDupA_notin Hnodup) as [_ Hnotin]; done. }
+      clear Heval1. assert (Sem_HiFP.eval_hfstmts (Qnil ProdVarOrder.T) (PVM.empty bits) (PVM.empty bits) init_s tmap = Some (PVM.empty bits, PVM.empty bits)) by (simpl; done).
+      specialize (eval_hfstmts_notin_none H Hnodup Heval2) as [Hhelper _]. apply Hhelper; done.
+    }
+    clear Heval2 Heqss_suffix'. simpl in Heval1. rewrite Hcmpnt in Heval1. destruct (sizeof_fgtyp gt < length indeterminate_val).
+    (* take *)
+    remember (take (sizeof_fgtyp gt) indeterminate_val) as val; clear Heqval.
+    assert (Hprefix : PVM.find v s = PVM.find v (PVM.add v val temp_s)).
+      assert (Hnotin : ~ In v (fst (List.split l1))). 
+      { specialize (PVM.elements_3w conn_map) as Hnodup. rewrite Helements in Hnodup. move : Hnodup; clear; intro. specialize (NoDupA_notin Hnodup) as [Hnotin _]; done. }
+      assert (Hhypo : forall st, Qin st ss_prefix ->
+      match st with 
+      | Snode _ _ 
+      | Sreg _ _
+      | Swhen _ _ _ => False
+      | Sfcnct v0 _ 
+      | Sinvalid v0 => v0 <> Eid v
+      | _ => True
+      end).
+      rewrite Heqss_prefix; move : Hnotin Hin; clear.
+    intros Hnotin Hin. apply eval_hfstmts_convert_to_connect_stmts_for_comb_helper; intros; try done.
+    specialize (eval_hfstmts_notinss_findeq Hhypo Heval1) as [Hhelper _]; done.
+    rewrite Hprefix HiFP.PCELemmas.find_add_eq //. apply CEP.SE.eq_refl.
+    (* ext *)
+    remember (zext (sizeof_fgtyp gt - length indeterminate_val) indeterminate_val) as val; clear Heqval.
+    assert (Hprefix : PVM.find v s = PVM.find v (PVM.add v val temp_s)).
+      assert (Hnotin : ~ In v (fst (List.split l1))). 
+      { specialize (PVM.elements_3w conn_map) as Hnodup. rewrite Helements in Hnodup. move : Hnodup; clear; intro. specialize (NoDupA_notin Hnodup) as [Hnotin _]; done. }
+      assert (Hhypo : forall st, Qin st ss_prefix ->
+      match st with 
+      | Snode _ _ 
+      | Sreg _ _
+      | Swhen _ _ _ => False
+      | Sfcnct v0 _ 
+      | Sinvalid v0 => v0 <> Eid v
+      | _ => True
+      end).
+      rewrite Heqss_prefix; move : Hnotin Hin; clear.
+    intros Hnotin Hin. apply eval_hfstmts_convert_to_connect_stmts_for_comb_helper; intros; try done.
+    specialize (eval_hfstmts_notinss_findeq Hhypo Heval1) as [Hhelper _]; done.
+    rewrite Hprefix HiFP.PCELemmas.find_add_eq //. apply CEP.SE.eq_refl.
+    + (* cnct *)
+    remember (convert_to_connect_stmts conn_map) as cmlist.
+    rewrite /convert_to_connect_stmts PVM.fold_1 in Heqcmlist. 
+    apply CEP.Lemmas.find_some_mapsto in Hcm. apply CEP.Lemmas.F.elements_mapsto_iff in Hcm.
+    remember (PVM.elements conn_map) as elements. apply InA_alt in Hcm. destruct Hcm as [[v' e'] [Heq Hin]].
+    destruct Heq as [Heq0 Heq1]. simpl in Heq0; simpl in Heq1. move /eqP : Heq0 => Heq0; subst v' e'.
+    destruct (in_split _ _ Hin) as [l1 [l2 Helements]]. subst elements.
+    rewrite Helements in Heqcmlist. rewrite fold_left_app in Heqcmlist. simpl in Heqcmlist.
+    remember (fold_left (fun (a : HiFP.hfstmt_seq) (p : PVM.key * def_expr) => convert_to_connect_stmt (fst p) (snd p) a) l1 (Qnil _)) as ss_prefix.
+    remember (fold_left (fun (a : HiFP.hfstmt_seq) (p : PVM.key * def_expr) => convert_to_connect_stmt (fst p) (snd p) a) l2 (Qcons (Sfcnct (Eid v) e) ss_prefix)) as ss_suffix.
+    subst cmlist.
+    assert (Heqss_suffix' : ss_suffix = Qcat (fold_left
+                 (fun (a : HiFP.hfstmt_seq) (p : PVM.key * def_expr) =>
+                  convert_to_connect_stmt (fst p) (snd p) a) l2 (Qnil ProdVarOrder.T)) (Qcons (Sfcnct (Eid v) e) ss_prefix)). {
+      move : Heqss_suffix; clear; intro. remember (Qcons (Sfcnct (Eid v) e) ss_prefix) as res. clear Heqres. subst ss_suffix; clear.
+      rewrite -fold_left_qcat. simpl. done. }
+    clear Heqss_suffix.
+    rewrite Heqss_suffix' in Heval. apply eval_hfstmts_Qcat_exists in Heval. destruct Heval as [temp_s [temp_rs [Heval2 Heval1]]].
+    assert (Htemp : PVM.find v temp_s = None). { 
+      assert (Hnodup : ~ In v (fst (List.split l2))). {
+        specialize (PVM.elements_3w conn_map) as Hnodup. rewrite Helements in Hnodup. move : Hnodup; clear; intro.
+        specialize (NoDupA_notin Hnodup) as [_ Hnotin]; done. }
+      clear Heval1. assert (Sem_HiFP.eval_hfstmts (Qnil ProdVarOrder.T) (PVM.empty bits) (PVM.empty bits) init_s tmap = Some (PVM.empty bits, PVM.empty bits)) by (simpl; done).
+      specialize (eval_hfstmts_notin_none H Hnodup Heval2) as [Hhelper _]. apply Hhelper; done.
+    }
+    clear Heval2 Heqss_suffix'. simpl in Heval1. rewrite Hcmpnt in Heval1. destruct (Sem_HiFP.eval_hfexpr e init_s tmap) as [val|]; try discriminate.
+    assert (Hprefix : PVM.find v s = PVM.find v (PVM.add v val temp_s)).
+      assert (Hnotin : ~ In v (fst (List.split l1))). 
+      { specialize (PVM.elements_3w conn_map) as Hnodup. rewrite Helements in Hnodup. move : Hnodup; clear; intro. specialize (NoDupA_notin Hnodup) as [Hnotin _]; done. }
+      assert (Hhypo : forall st, Qin st ss_prefix ->
+      match st with 
+      | Snode _ _ 
+      | Sreg _ _
+      | Swhen _ _ _ => False
+      | Sfcnct v0 _ 
+      | Sinvalid v0 => v0 <> Eid v
+      | _ => True
+      end).
+      rewrite Heqss_prefix; move : Hnotin Hin; clear.
+    intros Hnotin Hin. apply eval_hfstmts_convert_to_connect_stmts_for_comb_helper; intros; try done.
+    specialize (eval_hfstmts_notinss_findeq Hhypo Heval1) as [Hhelper _]; done.
+    rewrite Hprefix HiFP.PCELemmas.find_add_eq //. apply CEP.SE.eq_refl.
+Qed. 
 
 Lemma eval_hfstmts_convert_to_connect_stmts_for_sequ conn_map init_s tmap rs s v : 
   match PVM.find v tmap with
   | Some (gt, Register) => Sem_HiFP.eval_hfstmts (convert_to_connect_stmts conn_map) (PVM.empty bits) (PVM.empty bits) init_s tmap = Some (rs, s) -> 
       match PVM.find v conn_map with
       | Some (D_fexpr e) => Sem_HiFP.eval_hfexpr e init_s tmap = PVM.find v rs
-      | Some (D_invalidated gt_e) => 
-          if (length indeterminate_val > sizeof_fgtyp gt_e) then Some (take (sizeof_fgtyp gt_e) indeterminate_val) = PVM.find v rs
-          else Some (zext ((sizeof_fgtyp gt_e) - (length indeterminate_val)) indeterminate_val) = PVM.find v rs
+      | Some (D_invalidated _) => 
+          if (length indeterminate_val > sizeof_fgtyp gt) then Some (take (sizeof_fgtyp gt) indeterminate_val) = PVM.find v rs
+          else Some (zext ((sizeof_fgtyp gt) - (length indeterminate_val)) indeterminate_val) = PVM.find v rs
       | _ => True
       end
   | _ => True
   end.
 Proof. 
-  (*destruct (PVM.find v tmap) as [[gt cmpnt]|] eqn : Hcmpnt; try done. destruct cmpnt; try done.
-  intros Heval Hcm. remember (convert_to_connect_stmts conn_map) as cmlist.
+  destruct (PVM.find v tmap) as [[gt cmpnt]|] eqn : Hcmpnt; try done. destruct cmpnt; try done.
+  intros Heval. destruct (PVM.find v conn_map) as [de|] eqn : Hcm; try done. destruct de as [gt_e|e].
+  + (* invalid *) 
+  remember (convert_to_connect_stmts conn_map) as cmlist.
+  rewrite /convert_to_connect_stmts PVM.fold_1 in Heqcmlist. 
+  apply CEP.Lemmas.find_some_mapsto in Hcm. apply CEP.Lemmas.F.elements_mapsto_iff in Hcm.
+  remember (PVM.elements conn_map) as elements. apply InA_alt in Hcm. destruct Hcm as [[v' e'] [Heq Hin]].
+  destruct Heq as [Heq0 Heq1]. simpl in Heq0; simpl in Heq1. move /eqP : Heq0 => Heq0; subst v' e'.
+  destruct (in_split _ _ Hin) as [l1 [l2 Helements]]. subst elements.
+  rewrite Helements in Heqcmlist. rewrite fold_left_app in Heqcmlist. simpl in Heqcmlist.
+  remember (fold_left (fun (a : HiFP.hfstmt_seq) (p : PVM.key * def_expr) => convert_to_connect_stmt (fst p) (snd p) a) l1 (Qnil _)) as ss_prefix.
+  remember (fold_left (fun (a : HiFP.hfstmt_seq) (p : PVM.key * def_expr) => convert_to_connect_stmt (fst p) (snd p) a) l2 (Qcons (Sinvalid (Eid v)) ss_prefix)) as ss_suffix.
+  subst cmlist.
+  assert (Heqss_suffix' : ss_suffix = Qcat (fold_left
+                 (fun (a : HiFP.hfstmt_seq) (p : PVM.key * def_expr) =>
+                  convert_to_connect_stmt (fst p) (snd p) a) l2 (Qnil ProdVarOrder.T)) (Qcons (Sinvalid (Eid v)) ss_prefix)). rewrite -fold_left_qcat qcat0s //. clear Heqss_suffix.
+  rewrite Heqss_suffix' in Heval. apply eval_hfstmts_Qcat_exists in Heval. destruct Heval as [temp_s [temp_rs [Heval2 Heval1]]].
+  assert (Htemp : PVM.find v temp_rs = None). { 
+    assert (Hnodup : ~ In v (fst (List.split l2))). {
+      specialize (PVM.elements_3w conn_map) as Hnodup. rewrite Helements in Hnodup. move : Hnodup; clear; intro.
+      specialize (NoDupA_notin Hnodup) as [_ Hnotin]; done. }
+    clear Heval1. assert (Sem_HiFP.eval_hfstmts (Qnil ProdVarOrder.T) (PVM.empty bits) (PVM.empty bits) init_s tmap = Some (PVM.empty bits, PVM.empty bits)) by (simpl; done).
+    specialize (eval_hfstmts_notin_none H Hnodup Heval2) as [_ Hhelper]. apply Hhelper; done.
+  }
+  clear Heval2 Heqss_suffix'. simpl in Heval1. rewrite Hcmpnt in Heval1. destruct (sizeof_fgtyp gt < length indeterminate_val).
+  (* take *)
+  remember (take (sizeof_fgtyp gt) indeterminate_val) as val; clear Heqval.
+  assert (Hprefix : PVM.find v rs = PVM.find v (PVM.add v val temp_rs)). 
+    assert (Hnotin : ~ In v (fst (List.split l1))). 
+      { specialize (PVM.elements_3w conn_map) as Hnodup. rewrite Helements in Hnodup. move : Hnodup; clear; intro. specialize (NoDupA_notin Hnodup) as [Hnotin _]; done. }
+      assert (Hhypo : forall st, Qin st ss_prefix ->
+      match st with 
+      | Snode _ _ 
+      | Sreg _ _ 
+      | Swhen _ _ _ => False
+      | Sfcnct v0 _ 
+      | Sinvalid v0 => v0 <> Eid v
+      | _ => True
+      end). 
+      rewrite Heqss_prefix; move : Hnotin Hin; clear.
+    intros Hnotin Hin. apply eval_hfstmts_convert_to_connect_stmts_for_comb_helper; intros; try done.
+    specialize (eval_hfstmts_notinss_findeq Hhypo Heval1) as [_ Hhelper]; done.
+  rewrite Hprefix HiFP.PCELemmas.find_add_eq //. apply CEP.SE.eq_refl.
+  (* ext *)
+  remember (zext (sizeof_fgtyp gt - length indeterminate_val) indeterminate_val) as val; clear Heqval.
+  assert (Hprefix : PVM.find v rs = PVM.find v (PVM.add v val temp_rs)). 
+    assert (Hnotin : ~ In v (fst (List.split l1))). 
+      { specialize (PVM.elements_3w conn_map) as Hnodup. rewrite Helements in Hnodup. move : Hnodup; clear; intro. specialize (NoDupA_notin Hnodup) as [Hnotin _]; done. }
+      assert (Hhypo : forall st, Qin st ss_prefix ->
+      match st with 
+      | Snode _ _ 
+      | Sreg _ _ 
+      | Swhen _ _ _ => False
+      | Sfcnct v0 _ 
+      | Sinvalid v0 => v0 <> Eid v
+      | _ => True
+      end). 
+      rewrite Heqss_prefix; move : Hnotin Hin; clear.
+    intros Hnotin Hin. apply eval_hfstmts_convert_to_connect_stmts_for_comb_helper; intros; try done.
+    specialize (eval_hfstmts_notinss_findeq Hhypo Heval1) as [_ Hhelper]; done.
+  rewrite Hprefix HiFP.PCELemmas.find_add_eq //. apply CEP.SE.eq_refl.
+  + (* cnct *) 
+  remember (convert_to_connect_stmts conn_map) as cmlist.
   rewrite /convert_to_connect_stmts PVM.fold_1 in Heqcmlist. 
   apply CEP.Lemmas.find_some_mapsto in Hcm. apply CEP.Lemmas.F.elements_mapsto_iff in Hcm.
   remember (PVM.elements conn_map) as elements. apply InA_alt in Hcm. destruct Hcm as [[v' e'] [Heq Hin]].
@@ -2751,90 +3465,118 @@ Proof.
       assert (Hhypo : forall st, Qin st ss_prefix ->
       match st with 
       | Snode _ _ 
-      | Sreg _ _ => False
+      | Sreg _ _ 
+      | Swhen _ _ _ => False
       | Sfcnct v0 _ 
       | Sinvalid v0 => v0 <> Eid v
       | _ => True
-      end).
+      end). 
       rewrite Heqss_prefix; move : Hnotin Hin; clear.
-      assert ((~ In v (fst (List.split l1))) -> forall ss, (forall st : hfstmt ProdVarOrder.T,
-      Qin st ss ->
-      match st with
-      | Snode _ _
-      | Sreg _ _ => False
-      | Sfcnct v0 _ | Sinvalid v0 => v0 <> Eid v
-      | _ => True
-      end) ->
-      forall st : hfstmt ProdVarOrder.T,
-        Qin st
-          (fold_left
-            (fun (a : HiFP.hfstmt_seq) (p : PVM.key * def_expr) =>
-              convert_to_connect_stmt (fst p) (snd p) a) l1 
-            ss) ->
-        match st with
-        | Snode _ _ 
-        | Sreg _ _ => False
-        | Sfcnct v0 _ | Sinvalid v0 => v0 <> Eid v
-        | _ => True
-        end). { move : l1. elim; simpl. intros _ ss Hss st Hin. apply Hss; done.
-      intros [hd_key hd_de] tl IH Hnotin ss Hss st. apply IH. move : Hnotin; apply contra_not; clear; intro.
-        destruct (List.split tl) as [left right]; simpl in *. right; done.
-      simpl; clear IH. rewrite -(qcat0s ss).
-      rewrite convert_to_connect_stmt_qcat. destruct hd_de; simpl; try done.
-      (* invalid *)
-      intros. destruct (Qin st0 ss) eqn : Hin. apply Hss; done. clear Hin. rewrite orb_false_r in H.
-      destruct st0; try done. move : Hnotin; apply contra_not; intro. subst h. move /eqP : H => H; inversion H; subst v.
-      destruct (List.split tl); simpl. left; done.
-      (* cnct *)
-      intros. destruct (Qin st0 ss) eqn : Hin. apply Hss; done. clear Hin. rewrite orb_false_r in H.
-      destruct st0; try done. move : Hnotin; apply contra_not; intro. subst h0. move /andP : H => [H _]. 
-      move /eqP : H => H; inversion H; subst v. destruct (List.split tl); simpl. left; done. }
-    intros Hnotin Hin. apply H; intros; try done.
+    intros Hnotin Hin. apply eval_hfstmts_convert_to_connect_stmts_for_comb_helper; intros; try done.
     specialize (eval_hfstmts_notinss_findeq Hhypo Heval1) as [_ Hhelper]; done.
   rewrite Hprefix HiFP.PCELemmas.find_add_eq //. apply CEP.SE.eq_refl.
-Qed.*) Admitted.
+Qed.
 
-Lemma eval_fexpr_PVM_equal_eq e init_s1 init_s2 tmap : PVM.equal (fun val1 val2 : bitseq => val1 == val2) init_s1 init_s2 -> Sem_HiFP.eval_hfexpr e init_s1 tmap = Sem_HiFP.eval_hfexpr e init_s2 tmap.
-Proof.
-Admitted.
+Lemma eval_fexpr_PVM_included_eq e init_s1 init_s2 tmap bs : pvm_included init_s1 init_s2 -> Sem_HiFP.eval_hfexpr e init_s1 tmap = Some bs ->
+  Sem_HiFP.eval_hfexpr e init_s2 tmap = Some bs.
+Proof. 
+  unfold pvm_included. intro Heq. move : e bs; elim.
+  simpl; done.
+  (* cast *)
+  simpl; intros. destruct u; try (apply H; done). 
+  1,2 : destruct (Sem_HiFP.eval_hfexpr h init_s1 tmap); try discriminate; inversion H0; subst bs; rewrite (H b) //.
+  (* unop *)
+  simpl; intros. destruct (Sem_HiFP.eval_hfexpr h init_s1 tmap); try discriminate.
+  destruct (Sem_HiFP.type_of_hfexpr h tmap); try discriminate. rewrite (H b) //.
+  (* binop *)
+  simpl; intros. destruct (Sem_HiFP.eval_hfexpr h init_s1 tmap); try discriminate.
+  destruct (Sem_HiFP.eval_hfexpr h0 init_s1 tmap); try discriminate.
+  destruct (Sem_HiFP.type_of_hfexpr h tmap); try discriminate. 
+  destruct (Sem_HiFP.type_of_hfexpr h0 tmap); try discriminate. rewrite (H b). rewrite (H0 b0) //. done.
+  (* mux *)
+  simpl; intros. destruct (Sem_HiFP.eval_hfexpr h init_s1 tmap); try discriminate.
+  destruct (Sem_HiFP.type_of_hfexpr h0 tmap); try discriminate. destruct f; try discriminate. 
+    destruct (Sem_HiFP.type_of_hfexpr h1 tmap); try discriminate. destruct f; try discriminate. 
+    destruct (Sem_HiFP.eval_hfexpr h0 init_s1 tmap); try discriminate.
+    destruct (Sem_HiFP.eval_hfexpr h1 init_s1 tmap); try discriminate.
+    rewrite (H b); try done. rewrite (H0 b0); try done. rewrite (H1 b1); try done.
+    (* same *)
+    destruct (Sem_HiFP.type_of_hfexpr h1 tmap); try discriminate. destruct f; try discriminate. 
+    destruct (Sem_HiFP.eval_hfexpr h0 init_s1 tmap); try discriminate.
+    destruct (Sem_HiFP.eval_hfexpr h1 init_s1 tmap); try discriminate.
+    rewrite (H b); try done. rewrite (H0 b0); try done. rewrite (H1 b1); try done.
+  (* ref *)
+  simpl; intros. destruct h; try discriminate. move : H; apply Heq.
+Qed.
 
-Lemma eval_hfstmts_ExpandBranches_funs_find_for_comb ss init_s tmap rs s v : 
-  match PVM.find v tmap with
-  | Some (gt, Out_port) 
-  | Some (gt, Wire) => (~ exists r, Qin (Sreg v r) ss) /\ (~ exists e, Qin (Snode v e) ss) ->
-  Sem_HiFP.eval_hfstmts ss (PVM.empty bits) (PVM.empty bits) init_s tmap = Some (rs, s) ->
-  forall conn_map, ExpandBranches_funs ss (PVM.empty def_expr) tmap = Some conn_map -> 
-      match PVM.find v conn_map with
-      | Some (D_fexpr e) => PVM.find v s = Sem_HiFP.eval_hfexpr e init_s tmap
-      | Some (D_invalidated gt_e) => 
-          if (length indeterminate_val > sizeof_fgtyp gt_e) then PVM.find v s = Some (take (sizeof_fgtyp gt_e) indeterminate_val)
-          else PVM.find v s = Some (zext ((sizeof_fgtyp gt_e) - (length indeterminate_val)) indeterminate_val)
-      | _ => True
-      end
+Lemma eval_hfexpr_Emux_eq_true_false cond init_s tmap: match Sem_HiFP.eval_hfexpr cond init_s tmap with
+  | Some valc => forall e1 e2, if (~~ is_zero valc) then Sem_HiFP.eval_hfexpr (Emux cond e1 e2) = Sem_HiFP.eval_hfexpr e1
+                 else Sem_HiFP.eval_hfexpr (Emux cond e1 e2) = Sem_HiFP.eval_hfexpr e2 
   | _ => True
   end.
-Proof. 
-  (*destruct (PVM.find v tmap) as [[gt cmpnt]|] eqn : Hcmpnt; try done. destruct cmpnt; try done.
-  assert (Hhelper : forall (ss : HiFP.hfstmt_seq) (rs s rs0 s0 : PVM.t bits),
+Proof. (* mux对长度有要求，但一般情况并不检查 *)
+  destruct (Sem_HiFP.eval_hfexpr cond init_s tmap) as [valc|] eqn : Hcond; try done. 
+Admitted.
+
+Lemma eval_hfstmts_ExpandBranches_funs_find_for_comb_helper v gt init_s tmap :
+  PVM.find v tmap = Some (gt, Out_port) \/ PVM.find v tmap = Some (gt, Wire) ->
+  forall (ss : HiFP.hfstmt_seq) (rs s rs0 s0 : PVM.t bits),
     (~ exists r, Qin (Sreg v r) ss) /\ (~ exists e, Qin (Snode v e) ss) -> 
     Sem_HiFP.eval_hfstmts ss rs0 s0 init_s tmap = Some (rs, s) ->
-    forall (old_conn_map : PVM.t def_expr),
+    forall val, PVM.find v s = Some val ->
+    forall (old_conn_map : PVM.t def_expr), (forall val0, PVM.find v s0 = Some val0 ->
     match PVM.find v old_conn_map with
-    | Some (D_fexpr e') => PVM.find v s0 = Sem_HiFP.eval_hfexpr e' init_s tmap
-    | _ => PVM.find v s0 = None
-    end ->
+    | Some (D_fexpr e') => Sem_HiFP.eval_hfexpr e' init_s tmap = Some val0
+    | Some (D_invalidated _) => 
+          if (length indeterminate_val > sizeof_fgtyp gt) then take (sizeof_fgtyp gt) indeterminate_val = val0
+          else zext ((sizeof_fgtyp gt) - (length indeterminate_val)) indeterminate_val = val0
+    | _ => False
+    end) ->
     forall conn_map : PVM.t def_expr,
     ExpandBranches_funs ss old_conn_map tmap = Some conn_map ->
-    forall (e : HiFP.hfexpr),
-    PVM.find v conn_map = Some (D_fexpr e) -> PVM.find v s = Sem_HiFP.eval_hfexpr e init_s tmap).
-  move : Hcmpnt; clear. intro. elim. 
-  - simpl; intros rs s rs0 s0 Hnotin Heval old_conn_map Hinit conn_map Hexpand_branches e Hfind.
-    inversion Heval; subst rs s; clear Heval. inversion Hexpand_branches; subst conn_map; clear Hexpand_branches.
-    rewrite Hfind in Hinit. done.
-  - intros st sts IH rs s rs0 s0 Hnotin Heval old_conn_map Hinit conn_map Hexpand_branches e Hfind.
+    match PVM.find v conn_map with
+    | Some (D_fexpr e) => Sem_HiFP.eval_hfexpr e init_s tmap = Some val 
+    | Some (D_invalidated _) => 
+          if (length indeterminate_val > sizeof_fgtyp gt) then take (sizeof_fgtyp gt) indeterminate_val = val
+          else zext ((sizeof_fgtyp gt) - (length indeterminate_val)) indeterminate_val = val
+    | _ => False
+    end
+with eval_hfstmt_ExpandBranches_funs_find_for_comb_helper st v gt init_s tmap :
+  PVM.find v tmap = Some (gt, Out_port) \/ PVM.find v tmap = Some (gt, Wire) ->
+  forall (rs_temp s_temp rs0 s0 : PVM.t bits),
+  Sem_HiFP.eval_hfstmt st rs0 s0 init_s tmap = Some (rs_temp, s_temp) ->
+  forall (old_conn_map : PVM.t def_expr), (forall val0, PVM.find v s0 = Some val0 ->
+    match PVM.find v old_conn_map with
+    | Some (D_fexpr e') => Sem_HiFP.eval_hfexpr e' init_s tmap = Some val0
+    | Some (D_invalidated _) => 
+          if (length indeterminate_val > sizeof_fgtyp gt) then take (sizeof_fgtyp gt) indeterminate_val = val0
+          else zext ((sizeof_fgtyp gt) - (length indeterminate_val)) indeterminate_val = val0
+    | _ => False
+    end) ->
+    match st with
+    | Swhen cond ss_true ss_false => forall true_conn_map false_conn_map,
+                        ExpandBranches_funs ss_true old_conn_map tmap = Some true_conn_map -> 
+                        ExpandBranches_funs ss_false old_conn_map tmap = Some false_conn_map ->
+                        forall val, PVM.find v s_temp = Some val ->
+                        match PVM.find v (combine_when_connections cond true_conn_map false_conn_map) with
+                        | Some (D_invalidated _) =>
+                                if sizeof_fgtyp gt < length indeterminate_val
+                                then take (sizeof_fgtyp gt) indeterminate_val = val
+                                else
+                                zext (sizeof_fgtyp gt - length indeterminate_val) indeterminate_val = val
+                        | Some (D_fexpr e') => Sem_HiFP.eval_hfexpr e' init_s tmap = Some val
+                        | None => False
+                        end
+    | _ => True
+    end. 
+Proof. clear eval_hfstmts_ExpandBranches_funs_find_for_comb_helper. intro Hcmpnt.
+  elim. 
+  - simpl; intros rs s rs0 s0 Hnotin Heval val Hval old_conn_map Hinit conn_map Hexpand_branches.
+    inversion Heval; subst rs s; clear Heval. inversion Hexpand_branches; subst conn_map; clear Hexpand_branches. apply Hinit; done.
+  - intros st sts IH rs s rs0 s0 Hnotin Heval val Hval old_conn_map Hinit conn_map Hexpand_branches.
     simpl in Heval. destruct (Sem_HiFP.eval_hfstmt st rs0 s0 init_s tmap) as [[rs_temp s_temp]|] eqn : Heval_temp; try discriminate.
     simpl in Hexpand_branches. destruct (ExpandBranch_fun st old_conn_map) as [temp_conn_map|] eqn : Hexpand_branches_temp; try discriminate.
-    move : conn_map Hexpand_branches e Hfind. apply IH with (rs := rs) (rs0 := rs_temp) (s0 := s_temp); try done. split; move : Hnotin => [Hnotin0 Hnotin1].
+    move : conn_map Hexpand_branches. apply IH with (rs := rs) (s := s) (rs0 := rs_temp) (s0 := s_temp); try done. split; move : Hnotin => [Hnotin0 Hnotin1].
     (* not in *)
     move : Hnotin0; apply contra_not; intro. destruct H as [r H]; exists r; simpl. rewrite H orb_true_r //.
     move : Hnotin1; apply contra_not; intro. destruct H as [e H]; exists e; simpl. rewrite H orb_true_r //.
@@ -2843,126 +3585,554 @@ Proof.
       split; move : Hnotin => [Hnotin0 Hnotin1].
       move : Hnotin0; apply contra_not; intro. destruct H as [r H]; exists r; simpl. rewrite H orb_true_l //.
       move : Hnotin1; apply contra_not; intro. destruct H as [e H]; exists e; simpl. rewrite H orb_true_l //. }
-    move : H; clear IH Hnotin Heval sts rs s. intro Hnotin.
+    move : H; clear IH Hnotin Heval sts rs. intros Hnotin val_temp Hval_temp.
     case Hst : st => [||var reg|||var node_e|ref e|ref|cond ss_true ss_false]; subst st.
-    + (* skip, wire *) 1,2,4,5 : 
-      simpl in Hexpand_branches_temp; inversion Hexpand_branches_temp; subst old_conn_map; clear Hexpand_branches_temp;
-      simpl in Heval_temp; inversion Heval_temp; subst rs0 s0; clear Heval_temp; done.
+    + (* skip, wire *)
+      1,2,4,5 : simpl in Hexpand_branches_temp; inversion Hexpand_branches_temp; subst old_conn_map; clear Hexpand_branches_temp;
+      simpl in Heval_temp; inversion Heval_temp; subst rs0 s0; clear Heval_temp; apply Hinit in Hval_temp; done.
     + (* reg *) 
       simpl in Hexpand_branches_temp. destruct (type reg); try discriminate. inversion Hexpand_branches_temp; subst temp_conn_map; clear Hexpand_branches_temp.
       rewrite HiFP.PCELemmas.find_add_neq.
-      simpl in Heval_temp. destruct (PVM.find var init_s); try discriminate. inversion Heval_temp; subst rs_temp s_temp; clear Heval_temp. done.
+      simpl in Heval_temp. destruct (PVM.find var init_s); try discriminate. inversion Heval_temp; subst rs_temp s_temp; clear Heval_temp. apply Hinit in Hval_temp; done.
       move : Hnotin => [Hnotin _]. move : Hnotin; apply contra_not; intro. exists reg; simpl. move /eqP : H => H; subst v. rewrite eq_refl; rewrite eq_refl; simpl; done.
     + (* node *) 
       simpl in Hexpand_branches_temp. inversion Hexpand_branches_temp; subst temp_conn_map; clear Hexpand_branches_temp.
       simpl in Heval_temp. destruct (Sem_HiFP.eval_hfexpr node_e init_s tmap); try discriminate. inversion Heval_temp; subst rs_temp s_temp; clear Heval_temp. 
-      rewrite HiFP.PCELemmas.find_add_neq. done.
+      rewrite HiFP.PCELemmas.find_add_neq in Hval_temp. apply Hinit in Hval_temp; done.
       move : Hnotin => [_ Hnotin]. move : Hnotin; apply contra_not; intro. exists node_e; simpl. move /eqP : H => H; subst v. rewrite eq_refl; rewrite eq_refl; simpl; done.
     + (* fcnct *) 
       simpl in Hexpand_branches_temp. case Href : ref => [var|||]; subst ref; try discriminate. inversion Hexpand_branches_temp; subst temp_conn_map; clear Hexpand_branches_temp.
       destruct (v == var) eqn : Heq.
-      * move /eqP : Heq => Heq; subst var. rewrite HiFP.PCELemmas.find_add_eq.
-        simpl in Heval_temp. rewrite Hcmpnt in Heval_temp. destruct (Sem_HiFP.eval_hfexpr e init_s tmap) as [val|]; try discriminate.
-        inversion Heval_temp; subst rs_temp s_temp; clear Heval_temp. rewrite HiFP.PCELemmas.find_add_eq //.
-        1,2 : apply CEP.SE.eq_refl.
+      * move /eqP : Heq => Heq; subst var. rewrite HiFP.PCELemmas.find_add_eq; try apply CEP.SE.eq_refl.
+        simpl in Heval_temp. destruct Hcmpnt as [Hcmpnt|Hcmpnt].
+        (* outport *)
+        rewrite Hcmpnt in Heval_temp. destruct (Sem_HiFP.eval_hfexpr e init_s tmap) as [val_e|]; try discriminate.
+        inversion Heval_temp; subst rs_temp s_temp; clear Heval_temp. rewrite HiFP.PCELemmas.find_add_eq in Hval_temp. done.
+        apply CEP.SE.eq_refl.
+        (* wire *)
+        rewrite Hcmpnt in Heval_temp. destruct (Sem_HiFP.eval_hfexpr e init_s tmap) as [val_e|]; try discriminate.
+        inversion Heval_temp; subst rs_temp s_temp; clear Heval_temp. rewrite HiFP.PCELemmas.find_add_eq in Hval_temp. done.
+        apply CEP.SE.eq_refl.
       * rewrite HiFP.PCELemmas.find_add_neq. 
         simpl in Heval_temp. destruct (PVM.find var tmap) as [[gt_var cmpnt_var]|]; try discriminate.
-        destruct cmpnt_var; destruct (Sem_HiFP.eval_hfexpr e init_s tmap) as [val|]; try discriminate; inversion Heval_temp; subst rs_temp s_temp; clear Heval_temp;
-        try rewrite HiFP.PCELemmas.find_add_neq; try done. 1-8 : move /eqP : Heq => Heq; move : Heq; apply contra_not; intro; unfold CEP.SE.eq in H; move /eqP : H => H; subst v; done.
+        destruct cmpnt_var; destruct (Sem_HiFP.eval_hfexpr e init_s tmap) as [val_e|]; try discriminate; inversion Heval_temp; subst rs_temp s_temp; clear Heval_temp;
+        try rewrite HiFP.PCELemmas.find_add_neq in Hval_temp; try (apply Hinit; done). 1-8 : move /eqP : Heq => Heq; move : Heq; apply contra_not; intro; unfold CEP.SE.eq in H; move /eqP : H => H; subst v; done.
     + (* invalid *) 
       simpl in Hexpand_branches_temp. case Href : ref => [var|||]; subst ref; try discriminate. destruct (PVM.find var tmap) as [[gt' cmpnt]|]; try discriminate.
       inversion Hexpand_branches_temp; subst temp_conn_map; clear Hexpand_branches_temp Hnotin. 
       destruct (v == var) eqn : Heq.
       * move /eqP : Heq => Heq; subst var. rewrite HiFP.PCELemmas.find_add_eq; try apply CEP.SE.eq_refl.
-        simpl in Heval_temp. rewrite Hcmpnt in Heval_temp. destruct (sizeof_fgtyp gt < length indeterminate_val).
-
-
-        1,2 : inversion Heval_temp; subst rs_temp s_temp; clear Heval_temp. rewrite HiFP.PCELemmas.find_add_eq //.
-        1,2 : apply CEP.SE.eq_refl.
+        simpl in Heval_temp. destruct Hcmpnt as [Hcmpnt|Hcmpnt].
+        (* outport *)
+        rewrite Hcmpnt in Heval_temp. destruct (sizeof_fgtyp gt < length indeterminate_val).
+        - (* take *)
+          inversion Heval_temp; subst rs_temp s_temp; clear Heval_temp; rewrite HiFP.PCELemmas.find_add_eq in Hval_temp.
+          inversion Hval_temp; done. apply CEP.SE.eq_refl.
+        - (* ext *)
+          inversion Heval_temp; subst rs_temp s_temp; clear Heval_temp. rewrite HiFP.PCELemmas.find_add_eq in Hval_temp.
+          inversion Hval_temp; done. apply CEP.SE.eq_refl.
+        (* wire *)
+        rewrite Hcmpnt in Heval_temp. destruct (sizeof_fgtyp gt < length indeterminate_val).
+        - (* take *)
+          inversion Heval_temp; subst rs_temp s_temp; clear Heval_temp; rewrite HiFP.PCELemmas.find_add_eq in Hval_temp.
+          inversion Hval_temp; done. apply CEP.SE.eq_refl.
+        - (* ext *)
+          inversion Heval_temp; subst rs_temp s_temp; clear Heval_temp. rewrite HiFP.PCELemmas.find_add_eq in Hval_temp.
+          inversion Hval_temp; done. apply CEP.SE.eq_refl.
       * rewrite HiFP.PCELemmas.find_add_neq. 
         simpl in Heval_temp. destruct (PVM.find var tmap) as [[gt_var cmpnt_var]|]; try discriminate.
-        destruct cmpnt_var; destruct (Sem_HiFP.eval_hfexpr e init_s tmap) as [val|]; try discriminate; inversion Heval_temp; subst rs_temp s_temp; clear Heval_temp;
-        try rewrite HiFP.PCELemmas.find_add_neq; try done. 1-8 : move /eqP : Heq => Heq; move : Heq; apply contra_not; intro; unfold CEP.SE.eq in H; move /eqP : H => H; subst v; done.
-      admit. (* dont know what to do *)
-    + (* when *) admit.
-  intros. move : conn_map H0 e H1. apply (Hhelper _ _ _ _ _ H). simpl. done.*)
+        destruct cmpnt_var; destruct (sizeof_fgtyp gt_var < length indeterminate_val); inversion Heval_temp; subst rs_temp s_temp; clear Heval_temp;
+        try rewrite HiFP.PCELemmas.find_add_neq in Hval_temp; try (apply Hinit; done). 1-15 : move /eqP : Heq => Heq; move : Heq; apply contra_not; intro; unfold CEP.SE.eq in H; move /eqP : H => H; subst v; done. 
+    + (* when *)
+      simpl in Hexpand_branches_temp. destruct (ExpandBranches_funs ss_true old_conn_map tmap) as [true_conn_map|] eqn : Hexpand_true; try discriminate.
+      destruct (ExpandBranches_funs ss_false old_conn_map tmap) as [false_conn_map|] eqn : Hexpand_false; try discriminate. 
+      inversion Hexpand_branches_temp; subst temp_conn_map; clear Hexpand_branches_temp.
+      specialize (eval_hfstmt_ExpandBranches_funs_find_for_comb_helper _ _ _ _ _ Hcmpnt _ _ _ _ Heval_temp _ Hinit) as Hwhen; simpl in Hwhen;
+        clear eval_hfstmt_ExpandBranches_funs_find_for_comb_helper. specialize (Hwhen _ _ Hexpand_true Hexpand_false _ Hval_temp). done.
+
+  clear eval_hfstmt_ExpandBranches_funs_find_for_comb_helper.
+  intros Hcmpnt rs_temp s_temp rs0 s0 Heval old_conn_map Hinit.
+  case Hst : st => [||var reg|||var node_e|ref e|ref|cond ss_true ss_false]; subst st; try done. intros true_conn_map false_conn_map Hexpand_true Hexpand_false val Hval.
+  simpl in Heval. destruct (Sem_HiFP.eval_hfexpr cond init_s tmap) as [valc|] eqn : Hvalc; try discriminate. destruct (~~ is_zero valc) eqn : Hcond.
+  - (* when go to true *)
+    clear Hexpand_false. 
+    assert ((~ exists r, Qin (Sreg v r) ss_true) /\ (~ exists e, Qin (Snode v e) ss_true)) by admit.
+    specialize (eval_hfstmts_ExpandBranches_funs_find_for_comb_helper _ _ _ _ Hcmpnt _ _ _ _ _ H Heval _ Hval _ Hinit _ Hexpand_true) as Htrue; 
+      clear eval_hfstmts_ExpandBranches_funs_find_for_comb_helper. unfold combine_when_connections. rewrite PVM.Lemmas.F.map2_1bis; try done.
+    destruct (PVM.find v true_conn_map) as [de_true|] eqn : Hde_true; try done. destruct de_true as [gt_e_true|e_true].
+    + (* true is invlid *) 
+      destruct (PVM.M.find v false_conn_map) as [de_false|]; try done. destruct de_false.
+      * (* false is invalid *) 
+        specialize (eval_hfexpr_Emux_eq_true_false cond init_s tmap) as Hmux. rewrite Hvalc Hcond in Hmux. rewrite Hmux.
+        unfold Sem_HiFP.indeterminate_cst. admit. (* eval_hfexpr const 稍微与invalid有些冲突*)
+      * (* false is cnct *) 
+        specialize (eval_hfexpr_Emux_eq_true_false cond init_s tmap) as Hmux. rewrite Hvalc Hcond in Hmux. rewrite Hmux.
+        unfold Sem_HiFP.indeterminate_cst. admit. (* eval_hfexpr const 稍微与invalid有些冲突*)
+    + (* true is cnct *) 
+      destruct (PVM.M.find v false_conn_map) as [de_false|]; try done. destruct de_false as [gt_e_false|e_false].
+      * (* false is invalid *) 
+        specialize (eval_hfexpr_Emux_eq_true_false cond init_s tmap) as Hmux. rewrite Hvalc Hcond in Hmux. rewrite Hmux //.
+      * (* false is cnct *) destruct (e_true == e_false) eqn : Heq; try done.
+        specialize (eval_hfexpr_Emux_eq_true_false cond init_s tmap) as Hmux. rewrite Hvalc Hcond in Hmux. rewrite Hmux //.
+  - (* when go to false *)
+    clear Hexpand_true. 
+    assert ((~ exists r, Qin (Sreg v r) ss_false) /\ (~ exists e, Qin (Snode v e) ss_false)) by admit.
+    specialize (eval_hfstmts_ExpandBranches_funs_find_for_comb_helper _ _ _ _ Hcmpnt _ _ _ _ _ H Heval _ Hval _ Hinit _ Hexpand_false) as Hfalse; 
+      clear eval_hfstmts_ExpandBranches_funs_find_for_comb_helper. unfold combine_when_connections. rewrite PVM.Lemmas.F.map2_1bis; try done.
+    destruct (PVM.find v true_conn_map) as [de_true|] eqn : Hde_true; try done. destruct de_true as [gt_e_true|e_true].
+    + (* true is invlid *) 
+      destruct (PVM.M.find v false_conn_map) as [de_false|]; try done. destruct de_false.
+      * (* false is invalid *) 
+        specialize (eval_hfexpr_Emux_eq_true_false cond init_s tmap) as Hmux. rewrite Hvalc Hcond in Hmux. rewrite Hmux.
+        unfold Sem_HiFP.indeterminate_cst. admit. (* eval_hfexpr const 稍微与invalid有些冲突*)
+      * (* false is cnct *) 
+        specialize (eval_hfexpr_Emux_eq_true_false cond init_s tmap) as Hmux. rewrite Hvalc Hcond in Hmux. rewrite Hmux //.
+    + (* true is cnct *) 
+      destruct (PVM.M.find v false_conn_map) as [de_false|]; try done. destruct de_false as [gt_e_false|e_false].
+      * (* false is invalid *) 
+        specialize (eval_hfexpr_Emux_eq_true_false cond init_s tmap) as Hmux. rewrite Hvalc Hcond in Hmux. rewrite Hmux.
+        unfold Sem_HiFP.indeterminate_cst. admit. (* eval_hfexpr const 稍微与invalid有些冲突*)
+      * (* false is cnct *) destruct (e_true == e_false) eqn : Heq. move /eqP : Heq => Heq; subst e_true. done.
+        specialize (eval_hfexpr_Emux_eq_true_false cond init_s tmap) as Hmux. rewrite Hvalc Hcond in Hmux. rewrite Hmux //.
 Admitted.
 
-Lemma eval_hfstmts_ExpandBranches_funs_find_for_sequ ss init_s tmap rs s v : 
+Lemma eval_hfstmts_ExpandBranches_funs_find_for_comb ss init_s tmap rs s v : 
   match PVM.find v tmap with
-  | Some (gt, Register) => Sem_HiFP.eval_hfstmts ss (PVM.empty bits) (PVM.empty bits) init_s tmap = Some (rs, s) ->
+  | Some (gt, Out_port) 
+  | Some (gt, Wire) => (~ exists r, Qin (Sreg v r) ss) /\ (~ exists e, Qin (Snode v e) ss) ->
+  Sem_HiFP.eval_hfstmts ss (PVM.empty bits) (PVM.empty bits) init_s tmap = Some (rs, s) ->
+  forall val, PVM.find v s = Some val ->
   forall conn_map, ExpandBranches_funs ss (PVM.empty def_expr) tmap = Some conn_map -> 
       match PVM.find v conn_map with
-      | Some (D_fexpr e) => PVM.find v rs = Sem_HiFP.eval_hfexpr e init_s tmap
-      | Some (D_invalidated gt_e) => 
-          if (length indeterminate_val > sizeof_fgtyp gt_e) then PVM.find v rs = Some (take (sizeof_fgtyp gt_e) indeterminate_val)
-          else PVM.find v rs = Some (zext ((sizeof_fgtyp gt_e) - (length indeterminate_val)) indeterminate_val)
-      | _ => True
+      | Some (D_fexpr e) => Sem_HiFP.eval_hfexpr e init_s tmap = Some val
+      | Some (D_invalidated _) => 
+          if (length indeterminate_val > sizeof_fgtyp gt) then take (sizeof_fgtyp gt) indeterminate_val = val
+          else zext ((sizeof_fgtyp gt) - (length indeterminate_val)) indeterminate_val = val
+      | _ => False
       end
   | _ => True
   end.
-Proof.
-  (*destruct (PVM.find v tmap) as [[gt cmpnt]|] eqn : Hcmpnt; try done. destruct cmpnt; try done.
-  assert (Hhelper : forall (ss : HiFP.hfstmt_seq) (rs s rs0 s0 : PVM.t bits),
+Proof. 
+  destruct (PVM.find v tmap) as [[gt cmpnt]|] eqn : Hcmpnt; try done. destruct cmpnt; try done.
+  assert (Hcmpnt' : PVM.find v tmap = Some (gt, Out_port) \/ PVM.find v tmap = Some (gt, Wire)) by (left; done).
+  intros; move : conn_map H2. apply (eval_hfstmts_ExpandBranches_funs_find_for_comb_helper Hcmpnt' H H0 H1); try done.
+  assert (Hcmpnt' : PVM.find v tmap = Some (gt, Out_port) \/ PVM.find v tmap = Some (gt, Wire)) by (right; done).
+  intros; move : conn_map H2. apply (eval_hfstmts_ExpandBranches_funs_find_for_comb_helper Hcmpnt' H H0 H1); try done.
+Qed. 
+
+Lemma ExpandBranch_fun_none st old_conn_map tmap temp_conn_map v : ExpandBranch_fun st old_conn_map tmap = Some temp_conn_map -> PVM.find v temp_conn_map = None
+  -> PVM.find v old_conn_map = None
+with ExpandBranches_fun_none ss old_conn_map tmap temp_conn_map v : ExpandBranches_funs ss old_conn_map tmap = Some temp_conn_map -> PVM.find v temp_conn_map = None
+  -> PVM.find v old_conn_map = None.
+Proof. 
+  destruct st; simpl.
+  1,2,4,5,6 : intros; inversion H; subst old_conn_map; done.
+  (* reg *)
+  intros. destruct (type h); try discriminate. inversion H; subst temp_conn_map; clear H.
+  apply CEP.Lemmas.not_in_find_none. apply CEP.Lemmas.find_none_not_in in H0. move : H0; apply contra_not.
+  intro. apply CEP.Lemmas.F.add_in_iff; right; done.
+  (* cnct *)
+  intros. destruct h; try discriminate. inversion H; subst temp_conn_map; clear H.
+  apply CEP.Lemmas.not_in_find_none. apply CEP.Lemmas.find_none_not_in in H0. move : H0; apply contra_not.
+  intro. apply CEP.Lemmas.F.add_in_iff; right; done.
+  (* invalid *)
+  intros. destruct h; try discriminate. destruct (PVM.find s tmap) as [[gt cmpnt]|]; try discriminate.
+  inversion H; subst temp_conn_map; clear H.
+  apply CEP.Lemmas.not_in_find_none. apply CEP.Lemmas.find_none_not_in in H0. move : H0; apply contra_not.
+  intro. apply CEP.Lemmas.F.add_in_iff; right; done.
+  (* when *)
+  intros. destruct (ExpandBranches_funs h0 old_conn_map tmap) as [true_conn_map|] eqn : Htrue; try discriminate.
+  destruct (ExpandBranches_funs h1 old_conn_map tmap) as [false_conn_map|] eqn : Hfalse; try discriminate.
+  inversion H; subst temp_conn_map; clear H. unfold combine_when_connections in H0. 
+  rewrite CEP.Lemmas.map2_1bis in H0; try done. destruct (PVM.find v true_conn_map) as [de_true|] eqn : Hfind_true.
+  destruct de_true; destruct (PVM.find v false_conn_map) as [de_false|]; try destruct de_false; try destruct (h2 == h3); try discriminate.
+  move : Hfalse H0; apply ExpandBranches_fun_none.
+
+  clear ExpandBranches_fun_none. move : ss old_conn_map temp_conn_map. elim. 
+  simpl; intros. inversion H; subst temp_conn_map; done.
+  simpl; intros hd tl IH; intros. destruct (ExpandBranch_fun hd old_conn_map tmap) eqn : Hexpand; try discriminate.
+  apply (IH _ _ H) in H0; clear IH. move : Hexpand H0; apply ExpandBranch_fun_none.
+Qed.
+
+Lemma eval_hfstmts_ExpandBranches_funs_find_for_sequ_helper v gt init_s tmap :
+  PVM.find v tmap = Some (gt, Register) -> 
+  forall (ss : HiFP.hfstmt_seq) (rs s rs0 s0 : PVM.t bits),
     Sem_HiFP.eval_hfstmts ss rs0 s0 init_s tmap = Some (rs, s) ->
-    forall (old_conn_map : PVM.t def_expr),
+    forall val, PVM.find v rs = Some val ->
+    forall (old_conn_map : PVM.t def_expr), (forall val0, PVM.find v rs0 = Some val0 ->
     match PVM.find v old_conn_map with
-    | Some (D_fexpr e') => PVM.find v rs0 = Sem_HiFP.eval_hfexpr e' init_s tmap
-    | _ => PVM.find v rs0 = None
-    end ->
+      | Some (D_fexpr e') => Sem_HiFP.eval_hfexpr e' init_s tmap = Some val0
+      | Some (D_invalidated _) => 
+            if (length indeterminate_val > sizeof_fgtyp gt) then take (sizeof_fgtyp gt) indeterminate_val = val0
+            else zext ((sizeof_fgtyp gt) - (length indeterminate_val)) indeterminate_val = val0
+      | _ => False
+      end) ->
     forall conn_map : PVM.t def_expr,
     ExpandBranches_funs ss old_conn_map tmap = Some conn_map ->
-    forall (e : HiFP.hfexpr),
-    PVM.find v conn_map = Some (D_fexpr e) -> PVM.find v rs = Sem_HiFP.eval_hfexpr e init_s tmap).
-  move : Hcmpnt; clear. intro. elim. 
-  - simpl; intros rs s rs0 s0 Heval old_conn_map Hinit conn_map Hexpand_branches e Hfind.
-    inversion Heval; subst rs s; clear Heval. inversion Hexpand_branches; subst conn_map; clear Hexpand_branches.
-    rewrite Hfind in Hinit. done.
-  - intros st sts IH rs s rs0 s0 Heval old_conn_map Hinit conn_map Hexpand_branches e Hfind.
+      match PVM.find v conn_map with
+      | Some (D_fexpr e) => Sem_HiFP.eval_hfexpr e init_s tmap = Some val 
+      | Some (D_invalidated _) => 
+            if (length indeterminate_val > sizeof_fgtyp gt) then take (sizeof_fgtyp gt) indeterminate_val = val
+            else zext ((sizeof_fgtyp gt) - (length indeterminate_val)) indeterminate_val = val
+      | _ => False
+      end
+with eval_hfstmt_ExpandBranches_funs_find_for_sequ_helper st v gt init_s tmap :
+  PVM.find v tmap = Some (gt, Register) -> 
+  forall (rs_temp s_temp rs0 s0 : PVM.t bits),
+  Sem_HiFP.eval_hfstmt st rs0 s0 init_s tmap = Some (rs_temp, s_temp) ->
+  forall (old_conn_map : PVM.t def_expr), (forall val0, PVM.find v rs0 = Some val0 ->
+  match PVM.find v old_conn_map with
+    | Some (D_fexpr e') => Sem_HiFP.eval_hfexpr e' init_s tmap = Some val0
+    | Some (D_invalidated _) => 
+          if (length indeterminate_val > sizeof_fgtyp gt) then take (sizeof_fgtyp gt) indeterminate_val = val0
+          else zext ((sizeof_fgtyp gt) - (length indeterminate_val)) indeterminate_val = val0
+    | _ => False
+    end) ->
+    match st with
+    | Swhen cond ss_true ss_false => forall true_conn_map false_conn_map,
+                        ExpandBranches_funs ss_true old_conn_map tmap = Some true_conn_map -> 
+                        ExpandBranches_funs ss_false old_conn_map tmap = Some false_conn_map ->
+                        forall val, PVM.find v rs_temp = Some val ->
+                        match PVM.find v (combine_when_connections cond true_conn_map false_conn_map) with
+                          | Some (D_invalidated _) =>
+                                  if sizeof_fgtyp gt < length indeterminate_val
+                                  then take (sizeof_fgtyp gt) indeterminate_val = val
+                                  else
+                                  zext (sizeof_fgtyp gt - length indeterminate_val) indeterminate_val = val
+                          | Some (D_fexpr e') => Sem_HiFP.eval_hfexpr e' init_s tmap = Some val
+                          | None => False
+                          end
+    | _ => True
+    end. 
+Proof. intro Hcmpnt.
+  elim. clear eval_hfstmts_ExpandBranches_funs_find_for_sequ_helper.
+  - simpl; intros rs s rs0 s0 Heval val Hval old_conn_map Hinit conn_map Hexpand_branches.
+    inversion Heval; subst rs s; clear Heval. inversion Hexpand_branches; subst conn_map; clear Hexpand_branches. apply Hinit; done.
+  - intros st sts IH rs s rs0 s0 Heval val Hval old_conn_map Hinit conn_map Hexpand_branches.
     simpl in Heval. destruct (Sem_HiFP.eval_hfstmt st rs0 s0 init_s tmap) as [[rs_temp s_temp]|] eqn : Heval_temp; try discriminate.
     simpl in Hexpand_branches. destruct (ExpandBranch_fun st old_conn_map) as [temp_conn_map|] eqn : Hexpand_branches_temp; try discriminate.
-    move : conn_map Hexpand_branches e Hfind. apply (IH _ _ _ _ Heval). clear IH Heval sts rs s.
+    move : Hexpand_branches; apply IH with (rs := rs) (s := s) (rs0 := rs_temp) (s0 := s_temp); try done.
+    (* find temp *)
+    clear IH Heval conn_map sts s. 
     case Hst : st => [||var reg|||var node_e|ref e|ref|cond ss_true ss_false]; subst st.
     + (* skip, wire *) 1,2,4,5 : 
       simpl in Hexpand_branches_temp; inversion Hexpand_branches_temp; subst old_conn_map; clear Hexpand_branches_temp;
-      simpl in Heval_temp; inversion Heval_temp; subst rs0 s0; clear Heval_temp; done.
+      simpl in Heval_temp; inversion Heval_temp; subst rs0 s0; clear Heval_temp; apply Hinit; done.
     + (* reg *) 
       simpl in Hexpand_branches_temp. destruct (type reg); try discriminate. inversion Hexpand_branches_temp; subst temp_conn_map; clear Hexpand_branches_temp.
+      simpl in Heval_temp. destruct (PVM.find var init_s) as [val_temp|] eqn : Hval_temp; try discriminate. inversion Heval_temp; subst rs_temp s_temp; clear Heval_temp. intros bs Hfind.
       destruct (v == var) eqn : Heq.
-      * move /eqP : Heq => Heq; subst var. rewrite HiFP.PCELemmas.find_add_eq.
-        simpl in Heval_temp; simpl. destruct (PVM.find v init_s) as [val|]; try discriminate. 
-        inversion Heval_temp; subst rs_temp s_temp; clear Heval_temp. rewrite HiFP.PCELemmas.find_add_eq //.
-        1,2 : apply CEP.SE.eq_refl.
-      * rewrite HiFP.PCELemmas.find_add_neq. 
-        simpl in Heval_temp. destruct (PVM.find var init_s) as [val|]; try discriminate. 
-        inversion Heval_temp; subst rs_temp s_temp; clear Heval_temp. rewrite HiFP.PCELemmas.find_add_neq //.
-        1,2 : admit.
+      move /eqP : Heq => Heq; subst v. rewrite PVM.Lemmas.find_add_eq. rewrite PVM.Lemmas.find_add_eq in Hfind. inversion Hfind; subst bs. simpl; done. 1,2 : apply PVM.M.SE.eq_refl.
+      rewrite PVM.Lemmas.find_add_neq. rewrite PVM.Lemmas.find_add_neq in Hfind. apply Hinit; done.
+      1,2 : move /eqP : Heq => Heq; move : Heq; apply contra_not; intro; unfold CEP.SE.eq in H; move /eqP : H => H; done.
     + (* node *) 
       simpl in Hexpand_branches_temp. inversion Hexpand_branches_temp; subst temp_conn_map; clear Hexpand_branches_temp.
-      simpl in Heval_temp. destruct (Sem_HiFP.eval_hfexpr node_e init_s tmap); try discriminate. inversion Heval_temp; subst rs_temp s_temp; clear Heval_temp. done.
+      simpl in Heval_temp. destruct (Sem_HiFP.eval_hfexpr node_e init_s tmap); try discriminate. inversion Heval_temp; subst rs_temp s_temp; clear Heval_temp. done. 
     + (* fcnct *) 
       simpl in Hexpand_branches_temp. case Href : ref => [var|||]; subst ref; try discriminate. inversion Hexpand_branches_temp; subst temp_conn_map; clear Hexpand_branches_temp.
       destruct (v == var) eqn : Heq.
       * move /eqP : Heq => Heq; subst var. rewrite HiFP.PCELemmas.find_add_eq.
-        simpl in Heval_temp. rewrite Hcmpnt in Heval_temp. destruct (Sem_HiFP.eval_hfexpr e init_s tmap) as [val|]; try discriminate.
+        simpl in Heval_temp. rewrite Hcmpnt in Heval_temp. destruct (Sem_HiFP.eval_hfexpr e init_s tmap) as [val_e|]; try discriminate.
         inversion Heval_temp; subst rs_temp s_temp; clear Heval_temp. rewrite HiFP.PCELemmas.find_add_eq //.
         1,2 : apply CEP.SE.eq_refl.
       * rewrite HiFP.PCELemmas.find_add_neq. 
         simpl in Heval_temp. destruct (PVM.find var tmap) as [[gt_var cmpnt_var]|]; try discriminate.
-        destruct cmpnt_var; destruct (Sem_HiFP.eval_hfexpr e init_s tmap) as [val|]; try discriminate; inversion Heval_temp; subst rs_temp s_temp; clear Heval_temp;
-        try rewrite HiFP.PCELemmas.find_add_neq; try done. 1-2 : admit.
+        destruct cmpnt_var; destruct (Sem_HiFP.eval_hfexpr e init_s tmap) as [val_e|]; try discriminate; inversion Heval_temp; subst rs_temp s_temp; clear Heval_temp;
+        try rewrite HiFP.PCELemmas.find_add_neq; try done. 1-2 : move /eqP : Heq => Heq; move : Heq; apply contra_not; intro; unfold CEP.SE.eq in H; move /eqP : H => H; subst v; done.
     + (* invalid *) 
-      (*simpl in Hexpand_branches_temp. case Href : ref => [var|||]; subst ref; try discriminate. inversion Hexpand_branches_temp; subst temp_conn_map; clear Hexpand_branches_temp.*)
-      admit. (* dont know what to do *)
-    + (* when *) admit.
-  intros. move : conn_map H0 e H1. apply (Hhelper _ _ _ _ _ H). simpl. done.*)
-Admitted. 
+      simpl in Hexpand_branches_temp. case Href : ref => [var|||]; subst ref; try discriminate. destruct (PVM.find var tmap) as [[gt' cmpnt]|]; try discriminate.
+      inversion Hexpand_branches_temp; subst temp_conn_map; clear Hexpand_branches_temp. 
+      destruct (v == var) eqn : Heq.
+      * move /eqP : Heq => Heq; subst var. rewrite HiFP.PCELemmas.find_add_eq; try apply CEP.SE.eq_refl.
+        simpl in Heval_temp. rewrite Hcmpnt in Heval_temp. destruct (sizeof_fgtyp gt < length indeterminate_val).
+        - (* take *)
+          inversion Heval_temp; subst rs_temp s_temp; clear Heval_temp. rewrite HiFP.PCELemmas.find_add_eq.
+          intros. inversion H; done. apply CEP.SE.eq_refl.
+        - (* ext *)
+          inversion Heval_temp; subst rs_temp s_temp; clear Heval_temp. rewrite HiFP.PCELemmas.find_add_eq.
+          intros. inversion H; done. apply CEP.SE.eq_refl.
+      * rewrite HiFP.PCELemmas.find_add_neq. 
+        simpl in Heval_temp. destruct (PVM.find var tmap) as [[gt_var cmpnt_var]|]; try discriminate.
+        destruct cmpnt_var; destruct (sizeof_fgtyp gt_var < length indeterminate_val); inversion Heval_temp; subst rs_temp s_temp; clear Heval_temp; try done.
+        1,2 : rewrite HiFP.PCELemmas.find_add_neq; try done.
+        1-3 : move /eqP : Heq => Heq; move : Heq; apply contra_not; intro; unfold CEP.SE.eq in H; move /eqP : H => H; subst v; done. 
+    + (* when *)
+      simpl in Hexpand_branches_temp. destruct (ExpandBranches_funs ss_true old_conn_map tmap) as [true_conn_map|] eqn : Hexpand_true; try discriminate.
+      destruct (ExpandBranches_funs ss_false old_conn_map tmap) as [false_conn_map|] eqn : Hexpand_false; try discriminate. 
+      inversion Hexpand_branches_temp; subst temp_conn_map; clear Hexpand_branches_temp. 
+      specialize (eval_hfstmt_ExpandBranches_funs_find_for_sequ_helper _ _ _ _ _ Hcmpnt _ _ _ _ Heval_temp _ Hinit) as Hwhen; simpl in Hwhen;
+        clear eval_hfstmt_ExpandBranches_funs_find_for_sequ_helper. specialize (Hwhen _ _ Hexpand_true Hexpand_false). done.
 
-Lemma eval_hfstmts_find_rs ss init_s tmap rs s : Sem_HiFP.eval_hfstmts ss (PVM.empty bits) (PVM.empty bits) init_s tmap = Some (rs, s) ->
-  forall v, match PVM.find v tmap with
-  | Some (_, Register) => True
+  clear eval_hfstmt_ExpandBranches_funs_find_for_sequ_helper. intro Hcmpnt.
+  intros rs_temp s_temp rs0 s0 Heval old_conn_map Hinit.
+  case Hst : st => [||var reg|||var node_e|ref e|ref|cond ss_true ss_false]; subst st; try done. intros true_conn_map false_conn_map Hexpand_true Hexpand_false val Hval.
+  simpl in Heval. destruct (Sem_HiFP.eval_hfexpr cond init_s tmap) as [valc|] eqn : Hvalc; try discriminate. destruct (~~ is_zero valc) eqn : Hcond.
+  - (* when go to true *)
+    clear Hexpand_false. 
+    specialize (eval_hfstmts_ExpandBranches_funs_find_for_sequ_helper _ _ _ _ Hcmpnt _ _ _ _ _ Heval _ Hval _ Hinit _ Hexpand_true) as Htrue; 
+      clear eval_hfstmts_ExpandBranches_funs_find_for_sequ_helper. unfold combine_when_connections. rewrite PVM.Lemmas.F.map2_1bis; try done.
+    destruct (PVM.find v true_conn_map) as [de_true|] eqn : Hde_true; try done. destruct de_true as [gt_e_true|e_true].
+    + (* true is invlid *) 
+      destruct (PVM.M.find v false_conn_map) as [de_false|]; try done. destruct de_false.
+      * (* false is invalid *) 
+        specialize (eval_hfexpr_Emux_eq_true_false cond init_s tmap) as Hmux. rewrite Hvalc Hcond in Hmux. rewrite Hmux.
+        unfold Sem_HiFP.indeterminate_cst. admit. (* eval_hfexpr const 稍微与invalid有些冲突*)
+      * (* false is cnct *) 
+        specialize (eval_hfexpr_Emux_eq_true_false cond init_s tmap) as Hmux. rewrite Hvalc Hcond in Hmux. rewrite Hmux.
+        unfold Sem_HiFP.indeterminate_cst. admit. (* eval_hfexpr const 稍微与invalid有些冲突*)
+    + (* true is cnct *) 
+      destruct (PVM.M.find v false_conn_map) as [de_false|]; try done. destruct de_false as [gt_e_false|e_false].
+      * (* false is invalid *) 
+        specialize (eval_hfexpr_Emux_eq_true_false cond init_s tmap) as Hmux. rewrite Hvalc Hcond in Hmux. rewrite Hmux //.
+      * (* false is cnct *) destruct (e_true == e_false) eqn : Heq; try done.
+        specialize (eval_hfexpr_Emux_eq_true_false cond init_s tmap) as Hmux. rewrite Hvalc Hcond in Hmux. rewrite Hmux //.
+  - (* when go to false *)
+    clear Hexpand_true. 
+    specialize (eval_hfstmts_ExpandBranches_funs_find_for_sequ_helper _ _ _ _ Hcmpnt _ _ _ _ _ Heval _ Hval _ Hinit _ Hexpand_false) as Hfalse; 
+      clear eval_hfstmts_ExpandBranches_funs_find_for_sequ_helper. unfold combine_when_connections. rewrite PVM.Lemmas.F.map2_1bis; try done.
+    destruct (PVM.find v true_conn_map) as [de_true|] eqn : Hde_true; try done. destruct de_true as [gt_e_true|e_true].
+    + (* true is invlid *) 
+      destruct (PVM.M.find v false_conn_map) as [de_false|]; try done. destruct de_false.
+      * (* false is invalid *) 
+        specialize (eval_hfexpr_Emux_eq_true_false cond init_s tmap) as Hmux. rewrite Hvalc Hcond in Hmux. rewrite Hmux.
+        unfold Sem_HiFP.indeterminate_cst. admit. (* eval_hfexpr const 稍微与invalid有些冲突*)
+      * (* false is cnct *) 
+        specialize (eval_hfexpr_Emux_eq_true_false cond init_s tmap) as Hmux. rewrite Hvalc Hcond in Hmux. rewrite Hmux //.
+    + (* true is cnct *) 
+      destruct (PVM.M.find v false_conn_map) as [de_false|]; try done. destruct de_false as [gt_e_false|e_false].
+      * (* false is invalid *) 
+        specialize (eval_hfexpr_Emux_eq_true_false cond init_s tmap) as Hmux. rewrite Hvalc Hcond in Hmux. rewrite Hmux.
+        unfold Sem_HiFP.indeterminate_cst. admit. (* eval_hfexpr const 稍微与invalid有些冲突*)
+      * (* false is cnct *) destruct (e_true == e_false) eqn : Heq. move /eqP : Heq => Heq; subst e_true. done.
+        specialize (eval_hfexpr_Emux_eq_true_false cond init_s tmap) as Hmux. rewrite Hvalc Hcond in Hmux. rewrite Hmux //.
+Admitted.
+
+Lemma eval_hfstmts_ExpandBranches_funs_find_for_sequ ss init_s tmap rs s v : 
+  match PVM.find v tmap with
+  | Some (gt, Register) => 
+  Sem_HiFP.eval_hfstmts ss (PVM.empty bits) (PVM.empty bits) init_s tmap = Some (rs, s) ->
+  forall val, PVM.find v rs = Some val ->
+  forall conn_map, ExpandBranches_funs ss (PVM.empty def_expr) tmap = Some conn_map -> 
+      match PVM.find v conn_map with
+      | Some (D_fexpr e) => Sem_HiFP.eval_hfexpr e init_s tmap = Some val
+      | Some (D_invalidated _) => 
+          if (length indeterminate_val > sizeof_fgtyp gt) then take (sizeof_fgtyp gt) indeterminate_val = val
+          else zext ((sizeof_fgtyp gt) - (length indeterminate_val)) indeterminate_val = val
+      | _ => False
+      end
+  | _ => True
+  end.
+Proof.
+  destruct (PVM.find v tmap) as [[gt cmpnt]|] eqn : Hcmpnt; try done. destruct cmpnt; try done.
+  intros. move : conn_map H1; apply (eval_hfstmts_ExpandBranches_funs_find_for_sequ_helper Hcmpnt H H0).
+  try done.
+Qed. 
+
+Lemma eval_hfstmts_find_none_cases_helper ss init_s tmap rs s temp_rs temp_s v : 
+  match PVM.find v tmap with
+  | Some (_, In_port) => PVM.find v temp_s = None /\ PVM.find v temp_rs = None
+  | Some (_, Instanceof) => PVM.find v temp_s = None /\ PVM.find v temp_rs = None
+  | Some (_, Memory) => PVM.find v temp_s = None /\ PVM.find v temp_rs = None
+  | Some (_, Fmodule) => PVM.find v temp_s = None /\ PVM.find v temp_rs = None
+  | Some (_, Register) => PVM.find v temp_s = None
+  | None => PVM.find v temp_s = None /\ PVM.find v temp_rs = None
+  | _ => PVM.find v temp_rs = None
+  end ->
+  Sem_HiFP.eval_hfstmts ss temp_rs temp_s init_s tmap = Some (rs, s) ->
+  match PVM.find v tmap with
+  | Some (_, In_port) => PVM.find v s = None /\ PVM.find v rs = None
+  | Some (_, Instanceof) => PVM.find v s = None /\ PVM.find v rs = None
+  | Some (_, Memory) => PVM.find v s = None /\ PVM.find v rs = None
+  | Some (_, Fmodule) => PVM.find v s = None /\ PVM.find v rs = None
+  | Some (_, Register) => PVM.find v s = None
+  | None => PVM.find v s = None /\ PVM.find v rs = None
+  | _ => PVM.find v rs = None
+  end
+with eval_hfstmt_find_rs_helper st init_s tmap rs s temp_rs temp_s v : 
+  match PVM.find v tmap with
+  | Some (_, In_port) => PVM.find v temp_s = None /\ PVM.find v temp_rs = None
+  | Some (_, Instanceof) => PVM.find v temp_s = None /\ PVM.find v temp_rs = None
+  | Some (_, Memory) => PVM.find v temp_s = None /\ PVM.find v temp_rs = None
+  | Some (_, Fmodule) => PVM.find v temp_s = None /\ PVM.find v temp_rs = None
+  | Some (_, Register) => PVM.find v temp_s = None
+  | None => PVM.find v temp_s = None /\ PVM.find v temp_rs = None
+  | _ => PVM.find v temp_rs = None
+  end ->
+  match PVM.find v tmap with
+  | Some (_, In_port) => (forall r, ~ hfstmt_eqn (Sreg v r) st) /\ (forall e, ~ hfstmt_eqn (Snode v e) st)
+      /\ (forall e, ~ hfstmt_eqn (Sfcnct (Eid v) e) st) /\ (~ hfstmt_eqn (Sinvalid (Eid v)) st)
+  | Some (_, Instanceof) => (forall r, ~ hfstmt_eqn (Sreg v r) st) /\ (forall e, ~ hfstmt_eqn (Snode v e) st)
+      /\ (forall e, ~ hfstmt_eqn (Sfcnct (Eid v) e) st) /\ (~ hfstmt_eqn (Sinvalid (Eid v)) st)
+  | Some (_, Memory) => (forall r, ~ hfstmt_eqn (Sreg v r) st) /\ (forall e, ~ hfstmt_eqn (Snode v e) st)
+      /\ (forall e, ~ hfstmt_eqn (Sfcnct (Eid v) e) st) /\ (~ hfstmt_eqn (Sinvalid (Eid v)) st)
+  | Some (_, Node) => forall r, ~ hfstmt_eqn (Sreg v r) st
+  | Some (_, Out_port) => forall r, ~ hfstmt_eqn (Sreg v r) st
+  | Some (_, Wire) => forall r, ~ hfstmt_eqn (Sreg v r) st
+  | Some (_, Fmodule) => (forall r, ~ hfstmt_eqn (Sreg v r) st) /\ (forall e, ~ hfstmt_eqn (Snode v e) st)
+      /\ (forall e, ~ hfstmt_eqn (Sfcnct (Eid v) e) st) /\ (~ hfstmt_eqn (Sinvalid (Eid v)) st)
+  | Some (_, Register) => (forall e, ~ hfstmt_eqn (Snode v e) st)
+  | None => (forall r, ~ hfstmt_eqn (Sreg v r) st) /\ (forall e, ~ hfstmt_eqn (Snode v e) st)
+  end ->
+  Sem_HiFP.eval_hfstmt st temp_rs temp_s init_s tmap = Some (rs, s) ->
+  match PVM.find v tmap with
+  | Some (_, In_port) => PVM.find v s = None /\ PVM.find v rs = None
+  | Some (_, Instanceof) => PVM.find v s = None /\ PVM.find v rs = None
+  | Some (_, Memory) => PVM.find v s = None /\ PVM.find v rs = None
+  | Some (_, Fmodule) => PVM.find v s = None /\ PVM.find v rs = None
+  | Some (_, Register) => PVM.find v s = None
+  | None => PVM.find v s = None /\ PVM.find v rs = None
   | _ => PVM.find v rs = None
   end.
+Proof. 
+  move : ss temp_rs temp_s rs s. elim. 
+  simpl; intros. inversion H0; subst rs s. apply H. 
+  simpl; intros hd tl IH; intros. clear eval_hfstmts_find_none_cases_helper.
+  destruct (Sem_HiFP.eval_hfstmt hd temp_rs temp_s init_s tmap) as [[rs0 ns0]|] eqn : Heval; try discriminate.
+  move : H0; apply IH; clear IH. move : Heval; apply (eval_hfstmt_find_rs_helper _ _ _ _ _ _ _ _ H). admit.
+
+  intros Hinit Hunique Heval. destruct st as [|v0 t|v0 r|v0 m|v0 v1|v0 e0|v0 e0|v0|c s1 s2] eqn : Hst; simpl in *.
+  (* skip, wire *) 1,2,4,5 : inversion Heval; subst rs s; apply Hinit.
+  (* reg *) destruct (PVM.find v0 init_s) as [val|]; try discriminate. inversion Heval; subst rs s; clear Heval.
+    destruct (PVM.find v tmap) as [[gt cmpnt]|] eqn : Hfind. destruct cmpnt; try done.
+    - (* inport *)
+      move : Hinit => [Htemp_s Htemp_rs]. split; try done. rewrite PVM.Lemmas.find_add_neq //. move : Hunique => [Hunique _].
+      specialize (Hunique r). move : Hunique; apply contra_not; intro. unfold PVM.M.SE.eq in H. 
+      rewrite H eq_refl //.
+    - (* inst *)
+      move : Hinit => [Htemp_s Htemp_rs]. split; try done. rewrite PVM.Lemmas.find_add_neq //. move : Hunique => [Hunique _].
+      specialize (Hunique r). move : Hunique; apply contra_not; intro. unfold PVM.M.SE.eq in H. 
+      rewrite H eq_refl //.
+    - (* memory *)
+      move : Hinit => [Htemp_s Htemp_rs]. split; try done. rewrite PVM.Lemmas.find_add_neq //. move : Hunique => [Hunique _].
+      specialize (Hunique r). move : Hunique; apply contra_not; intro. unfold PVM.M.SE.eq in H. 
+      rewrite H eq_refl //.
+    - (* node *)
+      rewrite PVM.Lemmas.find_add_neq //. 
+      specialize (Hunique r). move : Hunique; apply contra_not; intro. unfold PVM.M.SE.eq in H. 
+      rewrite H eq_refl //.
+    - (* outport *)
+      rewrite PVM.Lemmas.find_add_neq //. 
+      specialize (Hunique r). move : Hunique; apply contra_not; intro. unfold PVM.M.SE.eq in H. 
+      rewrite H eq_refl //.
+    - (* wire *)
+      rewrite PVM.Lemmas.find_add_neq //. 
+      specialize (Hunique r). move : Hunique; apply contra_not; intro. unfold PVM.M.SE.eq in H. 
+      rewrite H eq_refl //.
+    - (* module *)
+      move : Hinit => [Htemp_s Htemp_rs]. split; try done. rewrite PVM.Lemmas.find_add_neq //. move : Hunique => [Hunique _].
+      specialize (Hunique r). move : Hunique; apply contra_not; intro. unfold PVM.M.SE.eq in H. 
+      rewrite H eq_refl //.
+    - (* none *)
+      move : Hinit => [Htemp_s Htemp_rs]. split; try done. rewrite PVM.Lemmas.find_add_neq //. move : Hunique => [Hunique _].
+      specialize (Hunique r). move : Hunique; apply contra_not; intro. unfold PVM.M.SE.eq in H. 
+      rewrite H eq_refl //.
+  (* node *) destruct (Sem_HiFP.eval_hfexpr e0 init_s tmap) as [val|]; try discriminate. inversion Heval; subst rs s; clear Heval.
+    destruct (PVM.find v tmap) as [[gt cmpnt]|] eqn : Hfind. destruct cmpnt; try done.
+    - (* inport *)
+      move : Hinit => [Htemp_s Htemp_rs]. split; try done. rewrite PVM.Lemmas.find_add_neq //. move : Hunique => [_ [Hunique _]].
+      specialize (Hunique e0). move : Hunique; apply contra_not; intro. unfold PVM.M.SE.eq in H. 
+      rewrite H eq_refl //.
+    - (* inst *)
+      move : Hinit => [Htemp_s Htemp_rs]. split; try done. rewrite PVM.Lemmas.find_add_neq //. move : Hunique => [_ [Hunique _]].
+      specialize (Hunique e0). move : Hunique; apply contra_not; intro. unfold PVM.M.SE.eq in H. 
+      rewrite H eq_refl //.
+    - (* memory *)
+      move : Hinit => [Htemp_s Htemp_rs]. split; try done. rewrite PVM.Lemmas.find_add_neq //. move : Hunique => [_ [Hunique _]].
+      specialize (Hunique e0). move : Hunique; apply contra_not; intro. unfold PVM.M.SE.eq in H. 
+      rewrite H eq_refl //.
+    - (* reg *)
+      rewrite PVM.Lemmas.find_add_neq //. 
+      specialize (Hunique e0). move : Hunique; apply contra_not; intro. unfold PVM.M.SE.eq in H. 
+      rewrite H eq_refl //.
+    - (* module *)
+      move : Hinit => [Htemp_s Htemp_rs]. split; try done. rewrite PVM.Lemmas.find_add_neq //. move : Hunique => [_ [Hunique _]].
+      specialize (Hunique e0). move : Hunique; apply contra_not; intro. unfold PVM.M.SE.eq in H. 
+      rewrite H eq_refl //.
+    - (* none *)
+      move : Hinit => [Htemp_s Htemp_rs]. split; try done. rewrite PVM.Lemmas.find_add_neq //. move : Hunique => [_ Hunique].
+      specialize (Hunique e0). move : Hunique; apply contra_not; intro. unfold PVM.M.SE.eq in H. 
+      rewrite H eq_refl //.
+  (* cnct *) destruct v0 as [ref|a b|a b|a b]; try (inversion Heval; subst rs s; try done). 
+    destruct (PVM.find ref tmap) as [[gt_ref cmpnt_ref]|] eqn : Hgt; try discriminate. destruct (v == ref) eqn : Heq. 
+    (* v == ref *) move /eqP : Heq => Heq; subst ref. rewrite Hgt in Hunique Hinit; rewrite Hgt.
+      destruct cmpnt_ref; destruct (Sem_HiFP.eval_hfexpr e0 init_s tmap); try discriminate; inversion Heval; subst rs s; clear Heval; try done.
+      (* inport, inst, memory, module *)
+      1-4 : move : Hunique => [_ [_ [Hunique _]]]; specialize (Hunique e0); rewrite eq_refl in Hunique; simpl in Hunique;
+      rewrite eq_refl in Hunique; simpl in Hunique; done.
+    (* v <> ref *) destruct cmpnt_ref; destruct (Sem_HiFP.eval_hfexpr e0 init_s tmap); try discriminate; 
+      inversion Heval; subst rs s; clear Heval; try done; try rewrite PVM.Lemmas.find_add_neq; try done.
+      1-8 : unfold PVM.M.SE.eq; rewrite Heq //.
+  (* invalid *) destruct v0 as [ref|a b|a b|a b]; try (inversion Heval; subst rs s; try done). 
+    destruct (PVM.find ref tmap) as [[gt_ref cmpnt_ref]|] eqn : Hgt; try discriminate. destruct (v == ref) eqn : Heq. 
+    (* v == ref *) move /eqP : Heq => Heq; subst ref. rewrite Hgt in Hunique Hinit; rewrite Hgt.
+      destruct cmpnt_ref; destruct (sizeof_fgtyp gt_ref < length indeterminate_val); inversion Heval; subst rs s; clear Heval; try done.
+      (* inport, inst, memory, module *)
+      1-8 : move : Hunique => [_ [_ [_ Hunique]]]; rewrite eq_refl in Hunique; simpl in Hunique; done.
+    (* v <> ref *) destruct cmpnt_ref; destruct (sizeof_fgtyp gt_ref < length indeterminate_val); 
+      inversion Heval; subst rs s; clear Heval; try done; try rewrite PVM.Lemmas.find_add_neq; try done.
+      1-16 : unfold PVM.M.SE.eq; rewrite Heq //.
+  (* when *) destruct (Sem_HiFP.eval_hfexpr c init_s tmap) as [valc|]; try discriminate. destruct (~~ is_zero valc).
+    move : Heval; apply eval_hfstmts_find_none_cases_helper; try done.
+    move : Heval; apply eval_hfstmts_find_none_cases_helper; try done.
+Admitted.
+
+Lemma eval_hfstmts_find_none_cases ss init_s tmap rs s v : Sem_HiFP.eval_hfstmts ss (PVM.empty bits) (PVM.empty bits) init_s tmap = Some (rs, s) ->
+  match PVM.find v tmap with
+  | Some (_, In_port) => PVM.find v s = None /\ PVM.find v rs = None
+  | Some (_, Instanceof) => PVM.find v s = None /\ PVM.find v rs = None
+  | Some (_, Memory) => PVM.find v s = None /\ PVM.find v rs = None
+  | Some (_, Fmodule) => PVM.find v s = None /\ PVM.find v rs = None
+  | Some (_, Register) => PVM.find v s = None
+  | None => PVM.find v s = None /\ PVM.find v rs = None
+  | _ => PVM.find v rs = None
+  end.
+Proof. 
+  apply eval_hfstmts_find_none_cases_helper. intros; destruct (PVM.find v tmap) as [[gt cmpnt]|]; try done. destruct cmpnt; try done.
+Qed.
+
+(*Lemma find_node_qin_with_cond_helpers ss tmap init_s: 
+  forall v gt, PVM.find v tmap = Some (gt, Node) -> 
+  forall rs0 s0, PVM.find v s0 = None ->
+  forall rs1 s1, Sem_HiFP.eval_hfstmts ss rs0 s0 init_s tmap = Some (rs1, s1) ->
+  forall bs, PVM.find v s1 = Some bs ->
+  exists e, Qin_with_cond (Snode v e) ss init_s tmap.
+Proof. 
+  intros v gt Hcmpnt. move : ss; elim. simpl; intros. inversion H0; subst rs1 s1. rewrite H in H1. discriminate.
+  intros hd tl IH rs0 s0 Hinit rs1 s1 Hevals bs Hfind. simpl in Hevals. 
+  destruct (Sem_HiFP.eval_hfstmt hd rs0 s0 init_s tmap) as [[rs_temp s_temp]|] eqn : Heval; try discriminate.
+  simpl.
+
+with find_node_qin_with_cond_helper st tmap init_s: 
+  forall v gt, PVM.find v tmap = Some (gt, Node) -> 
+  forall rs0 s0, PVM.find v s0 = None ->
+  forall init_s rs1 s1, Sem_HiFP.eval_hfstmt st rs0 s0 init_s tmap = Some (rs1, s1) ->
+  forall bs, PVM.find v s1 = Some bs ->
+  exists e, Qin_with_cond (Snode v e) ss init_s tmap.*)
+
+Lemma find_node_qin_with_cond mv pp ss tmap: Sem_HiFP.module_tmap (PVM.empty (fgtyp * fcomponent)) (FInmod mv pp ss) = Some tmap ->
+  forall v gt, PVM.find v tmap = Some (gt, Node) -> 
+  forall init_s rs1 s1 bs, Sem_HiFP.eval_hfstmts ss (PVM.empty bits) (PVM.empty bits) init_s tmap = Some (rs1, s1) ->
+  PVM.find v s1 = Some bs ->
+  exists e, Qin_with_cond (Snode v e) ss init_s tmap.
+Proof.
+  simpl; intros. destruct (Sem_HiFP.ports_tmap' (PVM.empty (fgtyp * fcomponent)) pp) as[pmap|]; try discriminate.
+  (* td *)
+Admitted.
+
+Lemma qin_with_cond_node_qin_cmpnt v e ss init_s tmap: 
+  Qin_with_cond (Snode v e) ss init_s tmap -> 
+  Qin (Snode v e) (component_stmts_of ss).
+Proof.
+  (* td *)
+Admitted.
+
+Lemma pvm_included_refl valmap : pvm_included valmap valmap.
+Proof. 
+  unfold pvm_included. intros; done.
+Qed.
+
+Lemma func_type_included_eval_hfstmts ss conn_map tmap : ExpandBranches_funs ss (PVM.empty def_expr) tmap = Some conn_map ->
+  func_type_included (Sem_HiFP.eval_hfstmts ss) (Sem_HiFP.eval_hfstmts (Qcat (component_stmts_of ss) (convert_to_connect_stmts conn_map))) tmap.
 Proof.
 Admitted.
 
@@ -2974,8 +4144,8 @@ Theorem Sem_preservation_expandWhens :
       forall (newc : HiFP.hfcircuit),
       expandWhens c = Some newc ->
       match Sem_HiFP.compute_Sem newc inputs reg_init with
-      | Some (sem_new, regval_new) => PVM.equal (fun val1 val2 => val1 == val2) sem sem_new /\
-                                      PVM.equal (fun val1 val2 => val1 == val2) regval regval_new
+      | Some (sem_new, regval_new) => pvm_included sem sem_new /\
+                                      pvm_included regval regval_new
       | _ => true
       end
   | _ => true
@@ -2993,8 +4163,8 @@ Proof.
   unfold ExpandWhens_fun in *. destruct m as [mv pp ss|] eqn : Hm; try discriminate.
   destruct (ExpandBranches_funs ss (PVM.empty def_expr)) as [conn_map|] eqn : Hexpand_branches; try discriminate.
   inversion Hpass; subst fm. clear Hpass.
+  rewrite component_stmts_of_init_dclrs_eq in Hsem_new.
   destruct (Sem_HiFP.init_dclrs ss (Sem_HiFP.update_values reg_init inputs) tmap) as [init_s|] eqn : Hinit_s; try discriminate.
-  specialize (component_stmts_of_init_dclrs_eq Hinit_s) as Hinit_s_new. rewrite Hinit_s_new in Hsem_new; clear Hinit_s_new.
   destruct (Sem_HiFP.iterate Sem_HiFP.n (Sem_HiFP.eval_hfstmts ss) init_s tmap) as [s0|] eqn : Hiter; try discriminate.
   destruct (Sem_HiFP.eval_hfstmts ss (PVM.empty bits) (PVM.empty bits) s0 tmap) as [[rs ns]|] eqn : Hregval; try discriminate. inversion Hsem; subst s0 rs; clear Hsem.
   destruct (Sem_HiFP.iterate Sem_HiFP.n
@@ -3003,209 +4173,119 @@ Proof.
   destruct (Sem_HiFP.eval_hfstmts (Qcat (component_stmts_of ss) (convert_to_connect_stmts conn_map))
                (PVM.empty bits) (PVM.empty bits) s0 tmap) as [[rs ns_new]|] eqn : Hregval_new; try discriminate. inversion Hsem_new; subst s0 rs; clear Hsem_new.
 
-  assert (Hfst_do_this : PVM.equal (fun val1 val2 : bitseq_eqType => val1 == val2) sem sem_new). {
-    apply PVM_equal_iff_find_eq. move : Hiter Hiter_new; apply iterate_func_eq.  
-    (* apply func_type_eq_eval_hfstmts; try done. *)
+  assert (Hfst_do_this : pvm_included sem sem_new). { 
+    move : Hiter Hiter_new; apply iterate_func_included.
+    (*apply func_type_included_eval_hfstmts; try done. apply pvm_included_refl. } *)
 
-
-
-  unfold func_type_eq. intros init_s1 init_s2 s1 s2 rs1 rs2 Hinit_eq Hevalss1 Hevalss2; simpl. split.
+  unfold func_type_included. intros init_s1 init_s2 s1 s2 rs1 rs2 Hinit_eq Hevalss1 Hevalss2. split.
   - (* combinational part *)
     move : Hevalss1 Hevalss2 Hexpand_branches Htmap Hinit_eq; clear. intros Hevalss1 Hevalss2 Hexpand_branches Htmap Hinit_eq v.
     destruct (PVM.find v tmap) as [[gt cmpnt]|] eqn : Hcmpnt. destruct cmpnt.
-    * (* inport *) admit. (* PVM.find v s1 = PVM.find v s2 = None, inport不出现在连接左侧，不会被更新 *)
-    * (* instance of *) admit. (* 暂不考虑 *)
-    * (* memory *) admit. (* 暂不考虑 *)
-    * (* node : v的值在 component_stmts_of 中 *) 
-      assert (Hgt : exists gt, PVM.find v tmap = Some (gt, Node)) by (exists gt; done).
-      assert (He : exists e, Qin (Snode v e) ss). admit. (* 由Hgt *) destruct He as [e He].
-      assert (Hunique : unique_node_dclr ss) by admit. (* 前提 *)
-      rewrite (eval_hfstmts_for_unique_node He Hunique Hevalss1).
-      assert (He' : Qin (Snode v e) (Qcat (component_stmts_of ss) (convert_to_connect_stmts conn_map))). admit. 
+    * (* inport *) 
+      specialize (eval_hfstmts_find_none_cases v Hevalss1) as Hfind1; rewrite Hcmpnt in Hfind1; move : Hfind1 => [Hfind1 _].
+      intros; rewrite Hfind1 in H; discriminate.
+    * (* instance of *) 
+      specialize (eval_hfstmts_find_none_cases v Hevalss1) as Hfind1; rewrite Hcmpnt in Hfind1; move : Hfind1 => [Hfind1 _].
+      intros; rewrite Hfind1 in H; discriminate.
+    * (* memory *) 
+      specialize (eval_hfstmts_find_none_cases v Hevalss1) as Hfind1; rewrite Hcmpnt in Hfind1; move : Hfind1 => [Hfind1 _].
+      intros; rewrite Hfind1 in H; discriminate.
+    * (* node : v的值在 component_stmts_of 中 *) intros bs Hfind1.
+      specialize (find_node_qin_with_cond Htmap Hcmpnt Hevalss1 Hfind1) as He. destruct He as [e He].
+      assert (Hunique : unique_node_dclr_when ss). admit.
+      assert (He' : Qin (Snode v e) (Qcat (component_stmts_of ss) (convert_to_connect_stmts conn_map))). 
+      specialize (qin_with_cond_node_qin_cmpnt He) as Hin. apply Qin_Qcat; left; done.
       assert (Hunique' : unique_node_dclr (Qcat (component_stmts_of ss) (convert_to_connect_stmts conn_map))). admit.
-      rewrite (eval_hfstmts_for_unique_node He' Hunique' Hevalss2).
-      apply eval_fexpr_PVM_equal_eq. done.
+      rewrite (eval_hfstmts_for_unique_node He Hunique Hevalss1) in Hfind1.
+      assert (Hwhen : forall c ss1 ss2, ~ Qin (Swhen c ss1 ss2) (Qcat (component_stmts_of ss) (convert_to_connect_stmts conn_map))).
+        intros. intro. apply Qin_Qcat in H. destruct H. specialize (component_stmts_of_is_declaration H); simpl; done.
+        specialize (convert_to_connect_stmts_is_connection H); simpl; done.
+      rewrite (eval_hfstmts_for_unique_node' He' Hunique' Hwhen Hevalss2).
+      move : Hinit_eq Hfind1; apply eval_fexpr_PVM_included_eq.
     * (* outport *) 
-      assert (Hcm : exists dexpr, PVM.find v conn_map = Some dexpr). admit. (* 有dclr那么应该被连接 *)
-      destruct Hcm as [dexpr Hcm]. 
-      case Hdexpr : dexpr => [|gt_e|e]; subst dexpr.
-      admit. (* conn_map 中不允许未连接，实际上，我的ExpandBranches_funs并不产生D_undefined *)
+      specialize (eval_hfstmts_Qcat_some' (PVM.empty bits) (PVM.empty bits) Hevalss2) as Hexists. destruct Hexists as [[rs s] Hexists].
+      specialize eval_hfstmts_for_comb_only_cnct with (v := v) (tmap := tmap) as Hcnct. rewrite Hcmpnt in Hcnct.
+      assert (Hin : forall s, Qin s (component_stmts_of ss) -> is_declaration s) by (apply component_stmts_of_is_declaration).
+      assert (Hneq : forall v' e', Qin (Snode v' e') (component_stmts_of ss) -> v <> v'). admit. (* TBD *)
+      assert (Hwhen : forall c ss1 ss2, ~ Qin (Swhen c ss1 ss2) (Qcat (component_stmts_of ss) (convert_to_connect_stmts conn_map))). 
+        intros. intro. apply Qin_Qcat in H. destruct H. specialize (component_stmts_of_is_declaration H); simpl; done.
+        specialize (convert_to_connect_stmts_is_connection H); simpl; done.
+      specialize (Hcnct _ _ _ Hin Hneq Hwhen _ _ Hevalss2 _ _ Hexists). rewrite -Hcnct; clear Hcnct Hevalss2.
+      specialize eval_hfstmts_convert_to_connect_stmts_for_comb with (v := v) (tmap := tmap) as Hconvert. rewrite Hcmpnt in Hconvert.
+      specialize (Hconvert _ _ _ _ Hexists). clear Hexists.
+      specialize eval_hfstmts_ExpandBranches_funs_find_for_comb with (v := v) (tmap := tmap) as Hhelper.
+      rewrite Hcmpnt in Hhelper. 
+      assert (Hnotin : ~ (exists r : hfreg ProdVarOrder.T, Qin (Sreg v r) ss) /\ ~ (exists e : hfexpr ProdVarOrder.T, Qin (Snode v e) ss)). admit.
+      intros val Hval; specialize (Hhelper _ _ _ _ Hnotin Hevalss1 _ Hval _ Hexpand_branches). 
+      destruct (PVM.find v conn_map) as [dexpr|] eqn : Hcm; try done. destruct dexpr as [gt_e|e] eqn : Hde; subst dexpr.
       (* invalid *)
-      specialize (eval_hfstmts_Qcat_some' (PVM.empty bits) (PVM.empty bits) Hevalss2) as Hexists. destruct Hexists as [[rs s] Hexists].
-      specialize eval_hfstmts_for_comb_only_cnct with (v := v) (tmap := tmap) as Hcnct. rewrite Hcmpnt in Hcnct.
-      assert (Hin : forall s, Qin s (component_stmts_of ss) -> is_declaration s). admit. (* TBD *)
-      assert (Hneq : forall v' e', Qin (Snode v' e') (component_stmts_of ss) -> v <> v'). admit. (* TBD *)
-      specialize (Hcnct _ _ _ Hin Hneq _ _ Hevalss2 _ _ Hexists). rewrite -Hcnct; clear Hcnct Hevalss2.
-      specialize eval_hfstmts_convert_to_connect_stmts_for_comb with (v := v) (tmap := tmap) as Hconvert. rewrite Hcmpnt in Hconvert.
-      specialize (Hconvert _ _ _ _ Hexists). rewrite Hcm in Hconvert. clear Hexists.
-      specialize eval_hfstmts_ExpandBranches_funs_find_for_comb with (v := v) (tmap := tmap) as Hhelper.
-      rewrite Hcmpnt in Hhelper. 
-      assert (Hnotin : ~ (exists r : hfreg ProdVarOrder.T, Qin (Sreg v r) ss) /\ ~ (exists e : hfexpr ProdVarOrder.T, Qin (Snode v e) ss)). admit.
-      specialize (Hhelper _ _ _ _ Hnotin Hevalss1 _ Hexpand_branches). rewrite Hcm in Hhelper. 
-      destruct (sizeof_fgtyp gt_e < length indeterminate_val); rewrite -Hconvert Hhelper //.
+      destruct (sizeof_fgtyp gt < length indeterminate_val).
+      1,2 : rewrite -Hconvert Hhelper //.
       (* cnct *)
-      specialize (eval_hfstmts_Qcat_some' (PVM.empty bits) (PVM.empty bits) Hevalss2) as Hexists. destruct Hexists as [[rs s] Hexists].
-      specialize eval_hfstmts_for_comb_only_cnct with (v := v) (tmap := tmap) as Hcnct. rewrite Hcmpnt in Hcnct.
-      assert (Hin : forall s, Qin s (component_stmts_of ss) -> is_declaration s). admit. (* TBD *)
-      assert (Hneq : forall v' e', Qin (Snode v' e') (component_stmts_of ss) -> v <> v'). admit. (* TBD *)
-      specialize (Hcnct _ _ _ Hin Hneq _ _ Hevalss2 _ _ Hexists). rewrite -Hcnct; clear Hcnct Hevalss2.
-      specialize eval_hfstmts_convert_to_connect_stmts_for_comb with (v := v) (tmap := tmap) as Hconvert. rewrite Hcmpnt in Hconvert.
-      specialize (Hconvert _ _ _ _ Hexists). rewrite Hcm in Hconvert; rewrite -Hconvert. clear Hconvert Hexists.
-      specialize eval_hfstmts_ExpandBranches_funs_find_for_comb with (v := v) (tmap := tmap) as Hhelper.
-      rewrite Hcmpnt in Hhelper. 
-      assert (Hnotin : ~ (exists r : hfreg ProdVarOrder.T, Qin (Sreg v r) ss) /\ ~ (exists e : hfexpr ProdVarOrder.T, Qin (Snode v e) ss)). admit.
-      specialize (Hhelper _ _ _ _ Hnotin Hevalss1 _ Hexpand_branches). rewrite Hcm in Hhelper. rewrite Hhelper.
-      apply eval_fexpr_PVM_equal_eq; done.
-    * (* register *) admit. (* 均为 None *)
+      rewrite -Hconvert. move : Hhelper; apply eval_fexpr_PVM_included_eq; done.
+    * (* register *) 
+      specialize (eval_hfstmts_find_none_cases v Hevalss1) as Hfind1; rewrite Hcmpnt in Hfind1.
+      intros; rewrite Hfind1 in H; discriminate.
     * (* wire : 同 outport *) 
-      assert (Hcm : exists dexpr, PVM.find v conn_map = Some dexpr). admit. (* 有dclr那么应该被连接 *)
-      destruct Hcm as [dexpr Hcm]. 
-      case Hdexpr : dexpr => [|gt_e|e]; subst dexpr.
-      admit. (* conn_map 中不允许未连接，实际上，我的ExpandBranches_funs并不产生D_undefined *)
+      specialize (eval_hfstmts_Qcat_some' (PVM.empty bits) (PVM.empty bits) Hevalss2) as Hexists. destruct Hexists as [[rs s] Hexists].
+      specialize eval_hfstmts_for_comb_only_cnct with (v := v) (tmap := tmap) as Hcnct. rewrite Hcmpnt in Hcnct.
+      assert (Hin : forall s, Qin s (component_stmts_of ss) -> is_declaration s) by (apply component_stmts_of_is_declaration).
+      assert (Hneq : forall v' e', Qin (Snode v' e') (component_stmts_of ss) -> v <> v'). admit. (* TBD *)
+      assert (Hwhen : forall c ss1 ss2, ~ Qin (Swhen c ss1 ss2) (Qcat (component_stmts_of ss) (convert_to_connect_stmts conn_map))). 
+        intros. intro. apply Qin_Qcat in H. destruct H. specialize (component_stmts_of_is_declaration H); simpl; done.
+        specialize (convert_to_connect_stmts_is_connection H); simpl; done.
+      specialize (Hcnct _ _ _ Hin Hneq Hwhen _ _ Hevalss2 _ _ Hexists). rewrite -Hcnct; clear Hcnct Hevalss2.
+      specialize eval_hfstmts_convert_to_connect_stmts_for_comb with (v := v) (tmap := tmap) as Hconvert. rewrite Hcmpnt in Hconvert.
+      specialize (Hconvert _ _ _ _ Hexists). clear Hexists.
+      specialize eval_hfstmts_ExpandBranches_funs_find_for_comb with (v := v) (tmap := tmap) as Hhelper.
+      rewrite Hcmpnt in Hhelper. 
+      assert (Hnotin : ~ (exists r : hfreg ProdVarOrder.T, Qin (Sreg v r) ss) /\ ~ (exists e : hfexpr ProdVarOrder.T, Qin (Snode v e) ss)). admit.
+      intros val Hval; specialize (Hhelper _ _ _ _ Hnotin Hevalss1 _ Hval _ Hexpand_branches). 
+      destruct (PVM.find v conn_map) as [dexpr|] eqn : Hcm; try done. destruct dexpr as [gt_e|e] eqn : Hde; subst dexpr.
       (* invalid *)
-      specialize (eval_hfstmts_Qcat_some' (PVM.empty bits) (PVM.empty bits) Hevalss2) as Hexists. destruct Hexists as [[rs s] Hexists].
-      specialize eval_hfstmts_for_comb_only_cnct with (v := v) (tmap := tmap) as Hcnct. rewrite Hcmpnt in Hcnct.
-      assert (Hin : forall s, Qin s (component_stmts_of ss) -> is_declaration s). admit. (* TBD *)
-      assert (Hneq : forall v' e', Qin (Snode v' e') (component_stmts_of ss) -> v <> v'). admit. (* TBD *)
-      specialize (Hcnct _ _ _ Hin Hneq _ _ Hevalss2 _ _ Hexists). rewrite -Hcnct; clear Hcnct Hevalss2.
-      specialize eval_hfstmts_convert_to_connect_stmts_for_comb with (v := v) (tmap := tmap) as Hconvert. rewrite Hcmpnt in Hconvert.
-      specialize (Hconvert _ _ _ _ Hexists). rewrite Hcm in Hconvert. clear Hexists.
-      specialize eval_hfstmts_ExpandBranches_funs_find_for_comb with (v := v) (tmap := tmap) as Hhelper.
-      rewrite Hcmpnt in Hhelper. 
-      assert (Hnotin : ~ (exists r : hfreg ProdVarOrder.T, Qin (Sreg v r) ss) /\ ~ (exists e : hfexpr ProdVarOrder.T, Qin (Snode v e) ss)). admit.
-      specialize (Hhelper _ _ _ _ Hnotin Hevalss1 _ Hexpand_branches). rewrite Hcm in Hhelper. 
-      destruct (sizeof_fgtyp gt_e < length indeterminate_val); rewrite -Hconvert Hhelper //.
+      destruct (sizeof_fgtyp gt < length indeterminate_val).
+      1,2 : rewrite -Hconvert Hhelper //.
       (* cnct *)
-      specialize (eval_hfstmts_Qcat_some' (PVM.empty bits) (PVM.empty bits) Hevalss2) as Hexists. destruct Hexists as [[rs s] Hexists].
-      specialize eval_hfstmts_for_comb_only_cnct with (v := v) (tmap := tmap) as Hcnct. rewrite Hcmpnt in Hcnct.
-      assert (Hin : forall s, Qin s (component_stmts_of ss) -> is_declaration s). admit. (* TBD *)
-      assert (Hneq : forall v' e', Qin (Snode v' e') (component_stmts_of ss) -> v <> v'). admit. (* TBD *)
-      specialize (Hcnct _ _ _ Hin Hneq _ _ Hevalss2 _ _ Hexists). rewrite -Hcnct; clear Hcnct Hevalss2.
-      specialize eval_hfstmts_convert_to_connect_stmts_for_comb with (v := v) (tmap := tmap) as Hconvert. rewrite Hcmpnt in Hconvert.
-      specialize (Hconvert _ _ _ _ Hexists). rewrite Hcm in Hconvert; rewrite -Hconvert. clear Hconvert Hexists.
-      specialize eval_hfstmts_ExpandBranches_funs_find_for_comb with (v := v) (tmap := tmap) as Hhelper.
-      rewrite Hcmpnt in Hhelper. 
-      assert (Hnotin : ~ (exists r : hfreg ProdVarOrder.T, Qin (Sreg v r) ss) /\ ~ (exists e : hfexpr ProdVarOrder.T, Qin (Snode v e) ss)). admit.
-      specialize (Hhelper _ _ _ _ Hnotin Hevalss1 _ Hexpand_branches). rewrite Hcm in Hhelper. rewrite Hhelper.
-      apply eval_fexpr_PVM_equal_eq; done.
-    * (* module *) admit. (* 均为 None *)
-    * (* None *) admit. (* 均为 None *)
+      rewrite -Hconvert. move : Hhelper; apply eval_fexpr_PVM_included_eq; done.
+    * (* module *) 
+      specialize (eval_hfstmts_find_none_cases v Hevalss1) as Hfind1; rewrite Hcmpnt in Hfind1; move : Hfind1 => [Hfind1 _].
+      intros; rewrite Hfind1 in H; discriminate.
+    * (* None *) 
+      specialize (eval_hfstmts_find_none_cases v Hevalss1) as Hfind1; rewrite Hcmpnt in Hfind1; move : Hfind1 => [Hfind1 _].
+      intros; rewrite Hfind1 in H; discriminate.
 
-    (* old try *)
-    (*assert (Hbefore : forall v, PVM.find v s1 = eval_hfstmts_for_v ss init_s1 tmap v (PVM.find v init_s1)). admit.
-    assert (Hafter : forall v, eval_hfstmts_for_v ss init_s2 tmap v (PVM.find v init_s2) = PVM.find v s2). {
-      move : Hevalss2 Hexpand_branches Htmap; clear. intros Hevalss2 Hexpand_branches Htmap v.
-      destruct (PVM.find v tmap) as [[gt cmpnt]|] eqn : Hcmpnt. destruct cmpnt.
-      * (* inport *) admit. (* 此时 eval_hfstmts_for_v = PVM.find v init_s2(初始值), 原因是 inport 不出现在连接 lhs; 同时 s2 中input的值也不变 *)
-      * (* instance of *) admit. (* 暂不考虑 *)
-      * (* memory *) admit. (* 暂不考虑 *)
-      * (* node : v的值在 component_stmts_of 中 *) 
-        assert (Hgt : exists gt, PVM.find v tmap = Some (gt, Node)) by (exists gt; done).
-        assert (He : exists e, Qin (Snode v e) ss). admit. destruct He as [e He].
-        apply eval_hfstmts_Qcat_some in Hevalss2 as Hexists. destruct Hexists as [[rs s] Hexists].
-        apply (eval_hfstmts_for_node_no_cnct Hgt Hevalss2) in Hexists as Hevalss. rewrite -Hevalss; clear Hevalss Hevalss2.
-        rewrite (eval_hfstmts_for_v_node _ _ He). rewrite (eval_hfstmts_node He Hexists) //.
-      * (* outport *) 
-        assert (Hcm : exists dexpr, PVM.find v conn_map = Some dexpr). admit. destruct Hcm as [dexpr Hcm]. 
-        case Hdexpr : dexpr => [||e]; subst dexpr.
-        admit. (* conn_map 中不允许未连接 *)
-        admit. (* invalid 的信号不需证明相等？ *)
-        specialize (eval_hfstmts_Qcat_some' Hevalss2) as Hexists. destruct Hexists as [[rs s] Hexists].
-        specialize eval_hfstmts_for_others_only_cnct with (v := v) (tmap := tmap) as Hcnct. rewrite Hcmpnt in Hcnct.
-        specialize (Hcnct _ _ _ _ _ Hevalss2 _ _ Hexists). rewrite -Hcnct; clear Hcnct Hevalss2.
-        specialize (eval_hfstmts_for_v_others conn_map tmap v) as Heq. rewrite Hcmpnt in Heq.
-        rewrite (Heq _ Hcm); clear Heq. apply (eval_hfstmts_convert_to_connect_stmts Hexists Hcm).
-      * (* register *) admit. (* 均为 None *)
-      * (* wire : 同 outport *) 
-        assert (Hcm : exists dexpr, PVM.find v conn_map = Some dexpr). admit. destruct Hcm as [dexpr Hcm]. 
-        case Hdexpr : dexpr => [||e]; subst dexpr.
-        admit. (* conn_map 中不允许未连接 *)
-        admit. (* invalid 的信号不需证明相等？ *)
-        specialize (eval_hfstmts_Qcat_some' Hevalss2) as Hexists. destruct Hexists as [[rs s] Hexists].
-        specialize eval_hfstmts_for_others_only_cnct with (v := v) (tmap := tmap) as Hcnct. rewrite Hcmpnt in Hcnct.
-        specialize (Hcnct _ _ _ _ _ Hevalss2 _ _ Hexists). rewrite -Hcnct; clear Hcnct Hevalss2.
-        specialize (eval_hfstmts_for_v_others conn_map tmap v) as Heq. rewrite Hcmpnt in Heq.
-        rewrite (Heq _ Hcm); clear Heq. apply (eval_hfstmts_convert_to_connect_stmts Hexists Hcm).
-      * (* module *) admit. (* 均为 None *)
-      * (* None *) admit. (* 均为 None *)
-    }
-    intro. rewrite Hbefore -Hafter. 
-    assert (Hinit_eq' : forall v, PVM.find v init_s1 = PVM.find v init_s2) by (apply PVM_equal_iff_find_eq; done).
-    rewrite Hinit_eq'. apply (eval_hfstmts_for_v_init_eq _ _ _ _ Hinit_eq).*)
   - (* sequential part *)
     move : Hevalss1 Hevalss2 Hexpand_branches Htmap Hinit_eq; clear. intros Hevalss1 Hevalss2 Hexpand_branches Htmap Hinit_eq v.
     destruct (PVM.find v tmap) as [[gt cmpnt]|] eqn : Hcmpnt. destruct cmpnt.
     * (* inport, instance of, memory, node, output, wire, module, none *) 
-      1,2,3,4,5,7,8,9 : specialize (eval_hfstmts_find_rs Hevalss1 v) as Hfind1; rewrite Hcmpnt in Hfind1;
-      specialize (eval_hfstmts_find_rs Hevalss2 v) as Hfind2; rewrite Hcmpnt in Hfind2;
-      rewrite Hfind1 Hfind2 //.
+      1,2,3,8,9 : 
+      specialize (eval_hfstmts_find_none_cases v Hevalss1) as Hfind1; rewrite Hcmpnt in Hfind1; move : Hfind1 => [_ Hfind1];
+      intros; rewrite Hfind1 in H; discriminate.
+      1,2,4 : specialize (eval_hfstmts_find_none_cases v Hevalss1) as Hfind1; rewrite Hcmpnt in Hfind1;
+      intros; rewrite Hfind1 in H; discriminate.
     * (* register *) 
-      assert (Hcm : exists dexpr, PVM.find v conn_map = Some dexpr). admit. (* reg在dclr时就记录连接 *)
-      destruct Hcm as [dexpr Hcm]. 
-      case Hdexpr : dexpr => [|gt_e|e]; subst dexpr.
-      admit. (* 实际上，我的ExpandBranches_funs并不产生D_undefined *)
+      specialize (eval_hfstmts_Qcat_some' (PVM.empty bits) (PVM.empty bits) Hevalss2) as Hexists. destruct Hexists as [[rs s] Hexists].
+      specialize eval_hfstmts_for_sequ_only_cnct with (v := v) (tmap := tmap) as Hcnct. rewrite Hcmpnt in Hcnct.
+      assert (Hdclr : forall s, Qin s (component_stmts_of ss) -> is_declaration s) by (apply component_stmts_of_is_declaration).
+      assert (Hin : Qin (Sfcnct (Eid v) (Eref (Eid v))) (convert_to_connect_stmts conn_map) \/
+        (exists e : hfexpr ProdVarOrder.T, Qin (Sfcnct (Eid v) e) (convert_to_connect_stmts conn_map))). admit. (* TBD *)
+      specialize (Hcnct _ _ _ Hdclr Hexpand_branches Hin _ _ Hevalss2 _ _ Hexists). rewrite -Hcnct; clear Hcnct Hevalss2.
+      specialize eval_hfstmts_convert_to_connect_stmts_for_sequ with (v := v) (tmap := tmap) as Hconvert. rewrite Hcmpnt in Hconvert.
+      specialize (Hconvert _ _ _ _ Hexists). clear Hexists.
+      specialize eval_hfstmts_ExpandBranches_funs_find_for_sequ with (v := v) (tmap := tmap) as Hhelper.
+      rewrite Hcmpnt in Hhelper. 
+      intros val Hval; specialize (Hhelper _ _ _ _ Hevalss1 _ Hval _ Hexpand_branches). 
+      destruct (PVM.find v conn_map) as [dexpr|] eqn : Hcm; try done. destruct dexpr as [gt_e|e] eqn : Hde; subst dexpr.
       (* invalid *)
-      specialize (eval_hfstmts_Qcat_some' (PVM.empty bits) (PVM.empty bits) Hevalss2) as Hexists. destruct Hexists as [[rs s] Hexists].
-      specialize eval_hfstmts_for_sequ_only_cnct with (v := v) (tmap := tmap) as Hcnct. rewrite Hcmpnt in Hcnct.
-      assert (Hin : forall s, Qin s (component_stmts_of ss) -> is_declaration s). admit. (* TBD *)
-      assert (Hr_cnct : Qin (Sfcnct (Eid v) (Eref (Eid v))) (convert_to_connect_stmts conn_map) \/
-        (exists e : hfexpr ProdVarOrder.T, Qin (Sfcnct (Eid v) e) (convert_to_connect_stmts conn_map))). admit. (* TBD *)
-      specialize (Hcnct _ _ _ Hin Hexpand_branches Hr_cnct _ _ Hevalss2 _ _ Hexists). rewrite -Hcnct; clear Hcnct Hevalss2.
-      specialize eval_hfstmts_convert_to_connect_stmts_for_sequ with (v := v) (tmap := tmap) as Hconvert. rewrite Hcmpnt in Hconvert.
-      specialize (Hconvert _ _ _ _ Hexists). rewrite Hcm in Hconvert. clear Hexists.
-      specialize eval_hfstmts_ExpandBranches_funs_find_for_sequ with (v := v) (tmap := tmap) as Hhelper.
-      rewrite Hcmpnt in Hhelper. 
-      (*assert (Hnotin : ~ (exists r : hfreg ProdVarOrder.T, Qin (Sreg v r) ss) /\ ~ (exists e : hfexpr ProdVarOrder.T, Qin (Snode v e) ss)). admit.*)
-      specialize (Hhelper _ _ _ _ Hevalss1 _ Hexpand_branches). rewrite Hcm in Hhelper. 
-      destruct (sizeof_fgtyp gt_e < length indeterminate_val); rewrite -Hconvert Hhelper //.
+      destruct (sizeof_fgtyp gt < length indeterminate_val).
+      1,2 : rewrite -Hconvert Hhelper //.
       (* cnct *)
-      specialize (eval_hfstmts_Qcat_some' (PVM.empty bits) (PVM.empty bits) Hevalss2) as Hexists. destruct Hexists as [[rs s] Hexists].
-      specialize eval_hfstmts_for_sequ_only_cnct with (v := v) (tmap := tmap) as Hcnct. rewrite Hcmpnt in Hcnct.
-      assert (Hin : forall s, Qin s (component_stmts_of ss) -> is_declaration s). admit. (* TBD *)
-      assert (Hr_cnct : Qin (Sfcnct (Eid v) (Eref (Eid v))) (convert_to_connect_stmts conn_map) \/
-        (exists e : hfexpr ProdVarOrder.T, Qin (Sfcnct (Eid v) e) (convert_to_connect_stmts conn_map))). admit. (* TBD *)
-      specialize (Hcnct _ _ _ Hin Hexpand_branches Hr_cnct _ _ Hevalss2 _ _ Hexists). rewrite -Hcnct; clear Hcnct Hevalss2.
-      specialize eval_hfstmts_convert_to_connect_stmts_for_sequ with (v := v) (tmap := tmap) as Hconvert. rewrite Hcmpnt in Hconvert.
-      specialize (Hconvert _ _ _ _ Hexists). rewrite Hcm in Hconvert; rewrite -Hconvert. clear Hconvert Hexists.
-      specialize eval_hfstmts_ExpandBranches_funs_find_for_sequ with (v := v) (tmap := tmap) as Hhelper.
-      rewrite Hcmpnt in Hhelper. 
-      (*assert (Hnotin : ~ (exists r : hfreg ProdVarOrder.T, Qin (Sreg v r) ss) /\ ~ (exists e : hfexpr ProdVarOrder.T, Qin (Snode v e) ss)). admit.*)
-      specialize (Hhelper _ _ _ _ Hevalss1 _ Hexpand_branches). rewrite Hcm in Hhelper. rewrite Hhelper.
-      apply eval_fexpr_PVM_equal_eq; done.
-
-  (* old old try *)
-  (*apply find_eq_iff_mem_eq_and_1d (* maybe we do not need this one *). split.
-  + (* mem eq *) admit. (* 这里比较好说明的角度应该是: 说明 s1的定义域等于init_s1 和 s2的定义域等于init_s2 *)
-  + (* find some value eq *) 
-    assert (Hbefore : forall v val, PVM.find v s1 = Some val -> eval_hfstmts_for_v ss init_s1 tmap v None = Some val). admit.
-    assert (Hafter : forall v val, eval_hfstmts_for_v ss init_s2 tmap v None = Some val -> PVM.find v s2 = Some val). {
-      move : Hevalss2 Hexpand_branches; clear. intros Hevalss2 Hexpand_branches v val Heval_for_v.
-      destruct (PVM.find v tmap) as [[gt cmpnt]|] eqn : Hcmpnt. destruct cmpnt.
-      * (* inport *) admit. (* 此时 eval_hfstmts_for_v = None, inport 不出现在连接 lhs *)
-      * (* instance of *) admit. (* 暂不考虑 *)
-      * (* memory *) admit. (* 暂不考虑 *)
-      * (* node : v的值在 component_stmts_of 中 *) 
-        assert (Hgt : exists gt, PVM.find v tmap = Some (gt, Node)) by (exists gt; done).
-        apply eval_hfstmts_Qcat_some in Hevalss2 as Hexists. destruct Hexists as [[rs s] Hexists].
-        apply (eval_hfstmts_for_node_dclr1 Hgt Heval_for_v) in Hexists as Hs.
-        move : Hexists Hs; apply (eval_hfstmts_for_node_no_cnct Hgt Hevalss2).
-      * (* outport *) admit.
-
-      * (* register *) admit. (* 此时 eval_hfstmts_for_v = None, iteration中不考虑reg*)
-      * (* wire : 同 outport *) admit.
-      * (* module *) admit. (* tmap 中不含 *)
-      * (* None *) admit. (* 此时 eval_hfstmts_for_v = None *)
-    }
-    move : Hinit_eq Hbefore Hafter; clear; intros.
-    apply Hbefore in H. rewrite (eval_hfstmts_for_v_init_eq _ _ _ Hinit_eq) in H. apply Hafter in H; done.
-  *)
-  
-
-    apply PVM_equal_refl.
+      rewrite -Hconvert. move : Hhelper; apply eval_fexpr_PVM_included_eq; done.
+    apply pvm_included_refl.
   }
   (* proof the equivalence of registers' next state values *)
   split; try done.
-  specialize func_type_eq_eval_hfstmts as Hhelper. apply Hhelper with (tmap := tmap) in Hexpand_branches. clear Hhelper.
-  unfold func_type_eq in Hexpand_branches. apply (Hexpand_branches _ _ _ _ _ _ Hfst_do_this Hregval) in Hregval_new.
-  apply PVM_equal_iff_find_eq. move : Hregval_new => [_ Hregval_new]. done.
+  specialize func_type_included_eval_hfstmts as Hhelper. apply Hhelper with (tmap := tmap) in Hexpand_branches. clear Hhelper.
+  unfold func_type_included in Hexpand_branches. apply (Hexpand_branches _ _ _ _ _ _ Hfst_do_this Hregval) in Hregval_new.
+  move : Hregval_new => [_ Hregval_new]. done.
 Admitted.
